@prefix owl:    <http://www.w3.org/2002/07/owl#> .
@prefix rdf:    <http://www.w3.org/1999/02/22-rdf-syntax-ns#> .
@prefix rdfs:   <http://www.w3.org/2000/01/rdf-schema#> .
@prefix xsd:    <http://www.w3.org/2001/XMLSchema#> .
@prefix dct:    <http://purl.org/dc/terms/> .
@prefix skos:   <http://www.w3.org/2004/02/skos/core#> .
@prefix vann:   <http://purl.org/vocab/vann/> .
@prefix olo:    <http://purl.org/ontology/olo/core#> .
@prefix vs:     <http://www.w3.org/2003/06/sw-vocab-status/ns#> .
@prefix doap:   <http://usefulinc.com/ns/doap#> .
@prefix schema: <http://schema.org/> .
@prefix scor:   <http://purl.org/eis/vocab/scor#> .

scor:
    rdf:type owl:Ontology ;
    rdfs:comment "A vocabulary which represents the Supply Chain Operations Reference (SCOR) standard."@en ;
    rdfs:label "SCORVoc"@en;
    dct:creator <http://eis.iai.uni-bonn.de/Irlan>, <http://eis.iai.uni-bonn.de/NiklasPetersen>, <http://sebastian.tramp.name> ;
    dct:publisher <http://dbpedia.org/resource/University_of_Bonn>, <https://ns.eccenca.com/eccenca-GmbH> ;
    dct:license <http://www.opendatacommons.org/licenses/pddl/1.0/> ;
    dct:created "2015-03-01"^^xsd:date ;
    dct:modified "2015-11-05"^^xsd:date ;
    owl:imports <http://www.w3.org/2004/02/skos/core> , dct: ;
    owl:versionInfo "SNAPSHOT" ;
    vann:preferredNamespacePrefix "scor" ;
    vann:preferredNamespaceUri "http://purl.org/eis/vocab/scor#" ;
    doap:homepage <https://github.com/vocol/scor> ;
    doap:implements <http://www.apics.org/sites/apics-supply-chain-council/frameworks/scor> ;
    doap:bug-database <https://github.com/vocol/scor/issues> ;
    doap:download-page <https://github.com/vocol/scor/releases> ;
    doap:wiki <https://github.com/vocol/scor/wiki> ;
    doap:repository <https://github.com/vocol/scor.git> ;
    rdfs:isDefinedBy scor: ;
 .

<https://github.com/vocol/scor.git>
    rdf:type doap:GitRepository ;
    rdfs:label "SCORVoc GitHub Repository" ;
.

<http://eis.iai.uni-bonn.de/Irlan>
    rdf:type schema:Person;
    rdfs:label "Irlán Grangel-González";
    schema:affiliation <http://dbpedia.org/resource/University_of_Bonn>;
.

<http://eis.iai.uni-bonn.de/NiklasPetersen>
    rdf:type schema:Person;
    rdfs:label "Niklas Petersen";
    schema:affiliation <http://dbpedia.org/resource/University_of_Bonn>;
.

<http://sebastian.tramp.name>
    rdf:type schema:Person;
    rdfs:label "Sebastian Tramp";
    owl:sameAs <http://aksw.org/SebastianTramp>, <https://ns.eccenca.com/stramp> ;
    schema:affiliation <https://ns.eccenca.com/eccenca-GmbH> ;
.

<http://dbpedia.org/resource/University_of_Bonn>
    rdf:type schema:CollegeOrUniversity;
    rdfs:label "University of Bonn"@en, "Rheinische Friedrich-Wilhelms-Universität Bonn"@de;
.

<https://ns.eccenca.com/eccenca-GmbH>
    rdf:type schema:Corporation;
    rdfs:label "eccenca GmbH";
.

<http://www.opendatacommons.org/licenses/pddl/1.0/>
    rdfs:label "ODC Public Domain Dedication and Licence (PDDL) 1.0"@en ;
.

# Level 0

[]
    rdf:type owl:AllDifferent ;
    owl:distinctMembers (
      scor:Aptitude scor:Competency scor:Experience scor:Skill
      scor:Training scor:Practice scor:Process
      schema:Person
    ) .

scor:Aptitude
    rdf:type owl:Class ;
    rdfs:comment "A natural, acquired, learned or developed ability to perform a certain kind of work at a"@en  ;
    rdfs:label "Aptitude"@en  ;
    rdfs:isDefinedBy scor: ;
    vs:term_status "testing" ;
    dct:modified "2015-11-05"^^xsd:date ;
 .

scor:Competency
    rdf:type owl:Class ;
    rdfs:comment "Describes the level or state of qualification to perform a certain role or tasks"@en  ;
    rdfs:label "Competency"@en  ;
    rdfs:isDefinedBy scor: ;
    vs:term_status "testing" ;
    dct:modified "2015-11-05"^^xsd:date ;
 .

scor:Experience
    rdf:type owl:Class ;
    rdfs:comment " the knowledge or ability acquired by observation or active participation. "@en  ;
    rdfs:label "Experience"@en  ;
    rdfs:isDefinedBy scor: ;
    vs:term_status "testing" ;
    dct:modified "2015-11-05"^^xsd:date ;
 .

scor:Skill
    rdf:type owl:Class ;
    rdfs:comment "The capacity to deliver pre-determined results with minimal input of time and energy"@en  ;
    rdfs:label "Skill"@en  ;
    rdfs:isDefinedBy scor: ;
    vs:term_status "testing" ;
    dct:modified "2015-11-05"^^xsd:date ;
 .

scor:Training
    rdf:type owl:Class ;
    rdfs:comment "Develops a skill or type of behavior through instruction"@en  ;
    rdfs:label "Training"@en  ;
    rdfs:isDefinedBy scor: ;
    vs:term_status "testing" ;
    dct:modified "2015-11-05"^^xsd:date ;
 .

schema:Person
    rdf:type owl:Class ;
    rdfs:comment "Models person in a Supply Chain"@en ;
    rdfs:label "Person"@en ;
 .

scor:Practice
    rdf:type owl:Class ;
    rdfs:comment "A practice is a unique way to configure a process or a set of processes"@en ;
    rdfs:label "Practice"@en ;
    rdfs:isDefinedBy scor: ;
    vs:term_status "testing" ;
    dct:modified "2015-11-05"^^xsd:date ;
 .

scor:Process
    rdf:type owl:Class ;
    rdfs:comment "A process is a unique activity performed to meet predefined outcomes"@en ;
    rdfs:label "Process"@en ;
    rdfs:isDefinedBy scor: ;
    vs:term_status "testing" ;
    dct:modified "2015-11-05"^^xsd:date ;
 .

# Level 1 Practice

[]
    rdf:type owl:AllDifferent ;
    owl:distinctMembers (
      scor:BestPractice scor:EmergingPractice scor:StandardPractice
    ) .

scor:BestPractice
    rdf:type owl:Class ;
    rdfs:comment "Best practices are 'current', 'structured' and 'repeatable' practices that have had a proved and positive impact on supply chain performance"@en ;
    rdfs:label "Best Practice"@en ;
    rdfs:subClassOf scor:Practice ;
    skos:notation "BP.B" ;
    rdfs:isDefinedBy scor: ;
    vs:term_status "testing" ;
    dct:modified "2015-11-05"^^xsd:date ;
 .

scor:EmergingPractice
    rdf:type owl:Class ;
    rdfs:comment "Introduce new technology, knowledge or radically different ways of organizing processes"@en ;
    rdfs:label "Emerging Practice"@en ;
    rdfs:subClassOf scor:Practice ;
    skos:notation "BP.E" ;
    rdfs:isDefinedBy scor: ;
    vs:term_status "testing" ;
    dct:modified "2015-11-05"^^xsd:date ;
 .

scor:StandardPractice
    rdf:type owl:Class ;
    rdfs:comment "How a wide range of companies have historically done business by default or happenstance"@en ;
    rdfs:label "Standard Practice"@en ;
    rdfs:subClassOf scor:Practice ;
    skos:notation "BP.S" ;
    rdfs:isDefinedBy scor: ;
    vs:term_status "testing" ;
    dct:modified "2015-11-05"^^xsd:date ;
 .

# Level 1 Processes

[]
    rdf:type owl:AllDifferent ;
    owl:distinctMembers (
      scor:Plan scor:Source scor:Make scor:Deliver scor:Return scor:Enable
    ) .

scor:Plan
    rdf:type owl:Class ;
    rdfs:subClassOf scor:Process ;
    rdfs:comment "Describes the planning activities associated with operating a supply chain. This includes gathering customer requirements, collecting information on available resources, and balancing requirements and resources to determine planned capabilities and resource gaps. This is followed by identifying the actions required to correct any gaps."@en ;
    rdfs:label "Plan"@en ;
    rdfs:subClassOf scor:Process ;
    skos:notation "sP" ;
    rdfs:isDefinedBy scor: ;
    vs:term_status "testing" ;
    dct:modified "2015-11-05"^^xsd:date ;
 .

scor:Source
    rdf:type owl:Class ;
    rdfs:subClassOf scor:Process ;
    rdfs:comment "Order, deliver, receipt and transfer of raw material items, subassemblies, product and/or services"@en ;
    rdfs:label "Source"@en ;
    rdfs:subClassOf scor:Process ;
    skos:notation "sS" ;
    rdfs:isDefinedBy scor: ;
    vs:term_status "testing" ;
    dct:modified "2015-11-05"^^xsd:date ;
 .

scor:Make
    rdf:type owl:Class ;
    rdfs:subClassOf scor:Process ;
    rdfs:comment "Adds value to products through mixing, separating, forming, machining, and chemical processes"@en ;
    rdfs:label "Make"@en ;
    rdfs:subClassOf scor:Process ;
    skos:notation "sM" ;
    rdfs:isDefinedBy scor: ;
    vs:term_status "testing" ;
    dct:modified "2015-11-05"^^xsd:date ;
 .

scor:Deliver
    rdf:type owl:Class ;
    rdfs:subClassOf scor:Process ;
    rdfs:comment "Performs customer-facing order management and order fulfillment activities"@en ;
    rdfs:label "Deliver"@en ;
    rdfs:subClassOf scor:Process ;
    skos:notation "sD" ;
    rdfs:isDefinedBy scor: ;
    vs:term_status "testing" ;
    dct:modified "2015-11-05"^^xsd:date ;
 .

scor:Return
    rdf:type owl:Class ;
    rdfs:subClassOf scor:Process ;
    rdfs:comment "Moves material from a customer back through the supply chain to address defects in product, ordering, or manufacturing, or to perform upkeep activities"@en ;
    rdfs:label "Return"@en ;
    rdfs:subClassOf scor:Process ;
    skos:notation "sR" ;
    rdfs:isDefinedBy scor: ;
    vs:term_status "testing" ;
    dct:modified "2015-11-05"^^xsd:date ;
 .

scor:Enable
    rdf:type owl:Class ;
    rdfs:subClassOf scor:Process ;
    rdfs:comment "Establishing, maintaining and monitoring information, relationships, resources, assets, business rules, compliance and contracts required to operate the supply chain"@en ;
    rdfs:label "Enable"@en ;
    rdfs:subClassOf scor:Process ;
    skos:notation "sE" ;
    rdfs:isDefinedBy scor: ;
    vs:term_status "testing" ;
    dct:modified "2015-11-05"^^xsd:date ;
 .

# Level 2 Processes

# Plan

[]
    rdf:type owl:AllDifferent ;
    owl:distinctMembers (
      scor:PlanSupplyChain scor:PlanSource scor:PlanMake scor:PlanDeliver scor:PlanReturn
    ) .

scor:PlanSupplyChain
    rdf:type owl:Class ;
    rdfs:subClassOf scor:Plan ;
    rdfs:comment "The development and establishment of courses of action over specified time periods that represent a projected appropriation of supply chain resources to meet supply chain requirements for the longest time fence constraints of supply resources"@en ;
    rdfs:label "Plan Supply Chain"@en ;
    rdfs:subClassOf scor:Plan ;
    skos:notation "sP1" ;
    rdfs:isDefinedBy scor: ;
    vs:term_status "testing" ;
    dct:modified "2015-11-05"^^xsd:date ;
 .

scor:PlanSource
    rdf:type owl:Class ;
    rdfs:subClassOf scor:Plan ;
    rdfs:comment "The development and establishment of courses of action over specified time periods that represent a projected appropriation of material resources to meet supply chain requirements"@en ;
    rdfs:label "Plan Source"@en ;
    rdfs:subClassOf scor:Plan ;
    skos:notation "sP2" ;
    rdfs:isDefinedBy scor: ;
    vs:term_status "testing" ;
    dct:modified "2015-11-05"^^xsd:date ;
 .

scor:PlanMake
    rdf:type owl:Class ;
    rdfs:subClassOf scor:Plan ;
    rdfs:comment "The development and establishment of courses of action over specified time periods that represent a projected appropriation of production resources to meet production requirements"@en ;
    rdfs:label "Plan Make"@en ;
    rdfs:subClassOf scor:Plan ;
    skos:notation "sP3" ;
    rdfs:isDefinedBy scor: ;
    vs:term_status "testing" ;
    dct:modified "2015-11-05"^^xsd:date ;
 .

scor:PlanDeliver
    rdf:type owl:Class ;
    rdfs:subClassOf scor:Plan ;
    rdfs:comment "The development and establishment of courses of action over specified time periods that represent a projected appropriation of delivery resources to meet delivery requirements"@en ;
    rdfs:label "Plan Deliver"@en ;
    rdfs:subClassOf scor:Plan ;
    skos:notation "sP4" ;
    rdfs:isDefinedBy scor: ;
    vs:term_status "testing" ;
    dct:modified "2015-11-05"^^xsd:date ;
 .

scor:PlanReturn
    rdf:type owl:Class ;
    rdfs:subClassOf scor:Plan ;
    rdfs:comment "establish and adjust courses of action or tasks over specified time periods that represent a projected appropriation of return resources and assets to meet anticipated as well as unanticipated return requirements"@en ;
    rdfs:label "Plan Return"@en ;
    rdfs:subClassOf scor:Plan ;
    skos:notation "sP5" ;
    rdfs:isDefinedBy scor: ;
    vs:term_status "testing" ;
    dct:modified "2015-11-05"^^xsd:date ;
 .

# Source

[]
    rdf:type owl:AllDifferent ;
    owl:distinctMembers (
      scor:SourceStockedProduct scor:SourceMakeToOrderProduct scor:SourceEngineerToOrderProduct
    ) .

scor:SourceStockedProduct
    rdf:type owl:Class ;
    rdfs:subClassOf scor:Source ;
    rdfs:comment "The process of ordering, receiving and transferring raw material items, sub-assemblies, product and or services based on aggregated demand requirements."@en;
    rdfs:label "Source Stocked Product"@en ;
    skos:notation "sS1" ;
    rdfs:isDefinedBy scor: ;
    vs:term_status "testing" ;
    dct:modified "2015-11-05"^^xsd:date ;
 .

scor:SourceMakeToOrderProduct
    rdf:type owl:Class ;
    rdfs:subClassOf scor:Source ;
    rdfs:comment "The processes of ordering and receiving product or material that is ordered (and may be configured) only when required by a specific customer order."@en ;
    rdfs:label "Source Make-to-Order Product"@en ;
    skos:notation "sS2" ;
    rdfs:isDefinedBy scor: ;
    vs:term_status "testing" ;
    dct:modified "2015-11-05"^^xsd:date ;
 .

scor:SourceEngineerToOrderProduct
    rdf:type owl:Class ;
    rdfs:subClassOf scor:Source ;
    rdfs:comment "The processes of identifying and selecting sources of supply, negotiating, validating, scheduling, ordering and receiving parts, assemblies or specialized products or services that are designed, ordered and/or built based on the requirements or specifications of a specific customer order."@en ;
    rdfs:label "Source Engineer-to-Order Product"@en ;
    skos:notation "sS3" ;
    rdfs:isDefinedBy scor: ;
    vs:term_status "testing" ;
    dct:modified "2015-11-05"^^xsd:date ;
 .

# Make

[]
    rdf:type owl:AllDifferent ;
    owl:distinctMembers (
      scor:MakeToStock scor:MakeToOrder scor:MakeEngineerToOrder
    ) .

scor:MakeToStock
    rdf:type owl:Class ;
    rdfs:subClassOf scor:Make ;
    rdfs:comment "The process of manufacturing in a make-to-stock environment adds value to products through mixing, separating, forming, machining, and chemical processes."@en ;
    rdfs:label "Make-to-Stock"@en ;
    skos:notation "sM1" ;
    rdfs:isDefinedBy scor: ;
    vs:term_status "testing" ;
    dct:modified "2015-11-05"^^xsd:date ;
 .

scor:MakeToOrder
    rdf:type owl:Class ;
    rdfs:subClassOf scor:Make ;
    rdfs:comment "The process of manufacturing in a make-to-order environment adds value to products through mixing, separating, forming, machining, and chemical processes for a specific customer order."@en ;
    rdfs:label "Make-to-Order"@en ;
    skos:notation "sM2" ;
    rdfs:isDefinedBy scor: ;
    vs:term_status "testing" ;
    dct:modified "2015-11-05"^^xsd:date ;
 .

scor:MakeEngineerToOrder
    rdf:type owl:Class ;
    rdfs:subClassOf scor:Make ;
    rdfs:comment "The process of developing, designing, validating, and ultimately using a manufacturing process to produce products or services based on the requirements of a specific customer."@en;
    rdfs:label "Engineer-to-Order"@en ;
    skos:notation "sM3" ;
    rdfs:isDefinedBy scor: ;
    vs:term_status "testing" ;
    dct:modified "2015-11-05"^^xsd:date ;
 .

# Deliver

[]
    rdf:type owl:AllDifferent ;
    owl:distinctMembers (
      scor:DeliverStockedProduct scor:DeliverMakeToOrderProduct
      scor:DeliverEngineerToOrderProduct scor:DeliverRetailProduct
    ) .

scor:DeliverStockedProduct
    rdf:type owl:Class ;
    rdfs:subClassOf scor:Deliver ;
    rdfs:comment "Delivers product that is sourced or made based on aggregated customer orders, projected orders/demand and inventory re-ordering parameters"@en ;
    rdfs:label "Deliver Stocked Product"@en ;
    skos:notation "sD1" ;
    rdfs:isDefinedBy scor: ;
    vs:term_status "testing" ;
    dct:modified "2015-11-05"^^xsd:date ;
 .

scor:DeliverMakeToOrderProduct
    rdf:type owl:Class ;
    rdfs:subClassOf scor:Deliver ;
    rdfs:comment "Delivers product that is sourced, configured, manufactured, and/or assembled from standard raw materials, parts, ingredients or sub-assemblies, in response to a specific firm customer order"@en ;
    rdfs:label "Deliver Make-to-Order Product"@en ;
    skos:notation "sD2" ;
    rdfs:isDefinedBy scor: ;
    vs:term_status "testing" ;
    dct:modified "2015-11-05"^^xsd:date ;
 .

scor:DeliverEngineerToOrderProduct
    rdf:type owl:Class ;
    rdfs:subClassOf scor:Deliver ;
    rdfs:comment "Obtaining, responding to, and allocating resources for a customer order that has unique requirements or specifications and delivering a product that is partially or fully designed, redesigned, manufactured, and/or assembled from a bill of materials or recipe that includes one or more custom parts or ingredients"@en ;
    rdfs:label "Deliver Engineer-to-Order Product"@en ;
    skos:notation "sD3" ;
    rdfs:isDefinedBy scor: ;
    vs:term_status "testing" ;
    dct:modified "2015-11-05"^^xsd:date ;
 .

scor:DeliverRetailProduct
    rdf:type owl:Class ;
    rdfs:subClassOf scor:Deliver ;
    rdfs:comment "To acquire, merchandise, and sell finished goods at a retail store"@en ;
    rdfs:label "Deliver Retail Product"@en ;
    skos:notation "sD4" ;
    rdfs:isDefinedBy scor: ;
    vs:term_status "testing" ;
    dct:modified "2015-11-05"^^xsd:date ;
 .

# Return

[]
    rdf:type owl:AllDifferent ;
    owl:distinctMembers (
        scor:DeliverReturnDefectiveProduct scor:DeliverReturnMROProduct
        scor:DeliverReturnExcessProduct scor:ReturnMROProduct
        scor:SourceReturnDefectiveProduct scor:SourceReturnExcessProduct
    ) .

scor:DeliverReturnDefectiveProduct
    rdf:type owl:Class ;
    rdfs:subClassOf scor:Return ;
    rdfs:comment "The receipt and disposition determination of defective products as defined by the warranty claims, product recall, non-conforming product and/or other similar policies including appropriate replacement"@en ;
    rdfs:label "Deliver Return Defective Product"@en ;
    skos:notation "sDR1" ;
    rdfs:isDefinedBy scor: ;
    vs:term_status "testing" ;
    dct:modified "2015-11-05"^^xsd:date ;
 .

scor:DeliverReturnMROProduct
    rdf:type owl:Class ;
    rdfs:subClassOf scor:Return ;
    rdfs:comment "The receipt of Maintenance, Repair and Overhaul (MRO) products or company assets for the purpose of servicing, repairing or upgrading it, as defined by Maintenance Plans or the occurrence or anticipation of risk of failure"@en ;
    rdfs:label "Deliver Return MRO Product"@en ;
    skos:notation "sDR2" ;
    rdfs:isDefinedBy scor: ;
    vs:term_status "testing" ;
    dct:modified "2015-11-05"^^xsd:date ;
 .

scor:DeliverReturnExcessProduct
    rdf:type owl:Class ;
    rdfs:subClassOf scor:Return ;
    rdfs:comment "The receipt of excess or aging inventory or obsolete products as defined by the terms and conditions of a customer/supplier contract"@en ;
    rdfs:label "Deliver Return Excess Product"@en ;
    skos:notation "sDR3" ;
    rdfs:isDefinedBy scor: ;
    vs:term_status "testing" ;
    dct:modified "2015-11-05"^^xsd:date ;
 .

scor:ReturnMROProduct
    rdf:type owl:Class ;
    rdfs:subClassOf scor:Return ;
    rdfs:comment "The return of Maintenance, Repair and Overhaul (MRO) products or company assets for the purpose of servicing, repairing or upgrading it, as defined by Maintenance Plans or the occurrence or anticipation of risk of failure"@en ;
    rdfs:label "Return MRO Product"@en ;
    skos:notation "sSR2" ;
    rdfs:isDefinedBy scor: ;
    vs:term_status "testing" ;
    dct:modified "2015-11-05"^^xsd:date ;
 .

scor:SourceReturnDefectiveProduct
    rdf:type owl:Class ;
    rdfs:subClassOf scor:Return ;
    rdfs:comment "The return and disposition determination of defective products as defined by the warranty claims, product recall, non-conforming product and/or other similar policies including appropriate replacement"@en ;
    rdfs:label "Source Return Defective Product"@en ;
    skos:notation "sSR1" ;
    rdfs:isDefinedBy scor: ;
    vs:term_status "testing" ;
    dct:modified "2015-11-05"^^xsd:date ;
 .

scor:SourceReturnExcessProduct
    rdf:type owl:Class ;
    rdfs:subClassOf scor:Return ;
    rdfs:comment "The return of excess or aging inventory or obsolete products as defined by the terms and conditions of a customer/supplier contract"@en ;
    rdfs:label "Source Return Excess Product"@en ;
    skos:notation "sSR3" ;
    rdfs:isDefinedBy scor: ;
    vs:term_status "testing" ;
    dct:modified "2015-11-05"^^xsd:date ;
 .

# Enable

[]
    rdf:type owl:AllDifferent ;
    owl:distinctMembers (
        scor:ManagePerformance scor:ManageSupplyChainBusinessRules
        scor:ManageDataInformation scor:ManageSupplyChainHumanResources
        scor:ManageSupplyChainAssets scor:ManageSupplyChainContracts
        scor:ManageSupplyChainNetworks scor:ManageRegulatoryCompliance
        scor:ManageSupplyChainRisk
    ) .

scor:ManageSupplyChainBusinessRules
    rdf:type owl:Class ;
    rdfs:subClassOf scor:Enable ;
    rdfs:comment "Establishing, documenting, communicating and publishing supply chain business rules"@en ;
    rdfs:label "Manage Supply Chain Business Rules"@en ;
    skos:notation "sE1" ;
    rdfs:isDefinedBy scor: ;
    vs:term_status "testing" ;
    dct:modified "2015-11-05"^^xsd:date ;
 .

scor:ManagePerformance
    rdf:type owl:Class ;
    rdfs:subClassOf scor:Enable ;
    rdfs:comment "Reporting performance, identifying gaps in performance, performing root cause analysis, and developing and launching corrective actions to close gaps in performance"@en ;
    rdfs:label "Manage Performance"@en ;
    skos:notation "sE2" ;
    rdfs:isDefinedBy scor: ;
    vs:term_status "testing" ;
    dct:modified "2015-11-05"^^xsd:date ;
 .

scor:ManageDataInformation
    rdf:type owl:Class ;
    rdfs:subClassOf scor:Enable ;
    rdfs:comment "Collecting, maintaining and publishing data and information required to plan, operate, measure and manage the supply chain"@en ;
    rdfs:label "Manage Data and Information"@en ;
    skos:notation "sE3" ;
    rdfs:isDefinedBy scor: ;
    vs:term_status "testing" ;
    dct:modified "2015-11-05"^^xsd:date ;
 .

scor:ManageSupplyChainHumanResources
    rdf:type owl:Class ;
    rdfs:subClassOf scor:Enable ;
    rdfs:comment "Developing, governing and maintaining an organization of permanent, temporary and outsourced staff, with the right qualifications, in support of the business objects and supply chain goals"@en ;
    rdfs:label "Manage Supply Chain Human Resources"@en ;
    skos:notation "sE4" ;
    rdfs:isDefinedBy scor: ;
    vs:term_status "testing" ;
    dct:modified "2015-11-05"^^xsd:date ;
 .

scor:ManageSupplyChainAssets
    rdf:type owl:Class ;
    rdfs:subClassOf scor:Enable ;
    rdfs:comment "Scheduling, maintaining and dispositioning of supply chain assets that operate supply chain processes"@en ;
    rdfs:label "Manage Supply Chain Assets"@en ;
    skos:notation "sE5" ;
    rdfs:isDefinedBy scor: ;
    vs:term_status "testing" ;
    dct:modified "2015-11-05"^^xsd:date ;
 .

scor:ManageSupplyChainContracts
    rdf:type owl:Class ;
    rdfs:subClassOf scor:Enable ;
    rdfs:comment "The management and communication of contractual agreements in support of business objectives and supply chain goals"@en ;
    rdfs:label "Manage Supply Chain Contracts"@en ;
    skos:notation "sE6" ;
    rdfs:isDefinedBy scor: ;
    vs:term_status "testing" ;
    dct:modified "2015-11-05"^^xsd:date ;
 .

scor:ManageSupplyChainNetworks
    rdf:type owl:Class ;
    rdfs:subClassOf scor:Enable ;
    rdfs:comment "Developing, governing and maintaining a network of supply chain assets"@en ;
    rdfs:label "Manage Supply Chain Networks"@en ;
    skos:notation "sE7" ;
    rdfs:isDefinedBy scor: ;
    vs:term_status "testing" ;
    dct:modified "2015-11-05"^^xsd:date ;
 .

scor:ManageRegulatoryCompliance
    rdf:type owl:Class ;
    rdfs:subClassOf scor:Enable ;
    rdfs:comment "Identifying, collecting, assessing and integrating regulatory compliance requirements in standard supply chain processes, policies and business rules"@en ;
    rdfs:label "Manage Regulatory Compliance"@en ;
    skos:notation "sE8" ;
    rdfs:isDefinedBy scor: ;
    vs:term_status "testing" ;
    dct:modified "2015-11-05"^^xsd:date ;
 .

scor:ManageSupplyChainRisk
    rdf:type owl:Class ;
    rdfs:subClassOf scor:Enable ;
    rdfs:comment "Identification and assessment of potential disruptions (risks) in the supply chain and developing a plan to mitigate these threats to operating the supply chain"@en ;
    rdfs:label "Manage Supply Chain Risk"@en ;
    skos:notation "sE9" ;
    rdfs:isDefinedBy scor: ;
    vs:term_status "testing" ;
    dct:modified "2015-11-05"^^xsd:date ;
 .

# Level 3 Processes

# Plan SC

scor:PSCIdentifyPrioritizeAggregateSCRequirements
    rdf:type owl:Class ;
    rdfs:comment "The process of identifying, aggregating, and prioritizing, all sources of demand for the integrated supply chain of a product or service at the appropriate level, horizon and interval."@en ;
    rdfs:label "Identify, Prioritize Aggregate Supply Chain Requirements"@en ;
    rdfs:subClassOf scor:PlanSupplyChain ;
    skos:notation "sP1.1" ;
    olo:next scor:IdentifyPrioritizeAggregateSCResources;
    rdfs:isDefinedBy scor: ;
    vs:term_status "testing" ;
    dct:modified "2015-11-05"^^xsd:date ;
 .

scor:IdentifyPrioritizeAggregateSCResources
    rdf:type owl:Class ;
    rdfs:comment "The process of identifying, prioritizing, and aggregating, as a whole with constituent parts, all sources of supply that are required and add value in the supply chain of a product or service at the appropriate level, horizon and interval."@en ;
    rdfs:label "Identify, Prioritize Aggregate Supply Chain Resources"@en ;
    rdfs:subClassOf scor:PlanSupplyChain ;
    olo:next scor:BalanceSCResourcesWithSCRequirements;
    skos:notation "sP1.2" ;
    rdfs:isDefinedBy scor: ;
    vs:term_status "testing" ;
    dct:modified "2015-11-05"^^xsd:date ;
 .

scor:BalanceSCResourcesWithSCRequirements
    rdf:type owl:Class ;
    rdfs:comment "The process of identifying and measuring the gaps and imbalances between demand and resources in order to determine how to best resolve the variances through marketing, pricing, packaging, warehousing, outsource plans or some other action that will optimize service, flexibility, costs, assets, (or other supply chain inconsistencies) in an iterative and collaborative environment."@en ;
    rdfs:label "Balance Supply Chain Resources with SC Requirements"@en ;
    rdfs:subClassOf scor:PlanSupplyChain ;
    olo:next scor:EstablishCommunicateSCPlans;
    skos:notation "sP1.3" ;
    rdfs:isDefinedBy scor: ;
    vs:term_status "testing" ;
    dct:modified "2015-11-05"^^xsd:date ;
 .

scor:EstablishCommunicateSCPlans
    rdf:type owl:Class ;
    rdfs:comment "The establishment and communication of courses of action over the appropriate time-defined (long-term, annual, monthly, weekly) planning horizon and interval, representing a projected appropriation of supply-chain resources to meet supply chain requirements."@en ;
    rdfs:label "Establish and Communicate Supply Chain Plans"@en ;
    rdfs:subClassOf scor:PlanSupplyChain ;
    skos:notation "sP1.4" ;
    rdfs:isDefinedBy scor: ;
    vs:term_status "testing" ;
    dct:modified "2015-11-05"^^xsd:date ;
 .

# Plan Source

scor:IdentifyPrioritizeAggregateProductRequirements
    rdf:type owl:Class ;
    rdfs:comment "The process of identifying, prioritizing, and considering, as a whole with constituent parts, all sources of demand for a product or service in the supply chain."@en ;
    rdfs:label "Identify, Prioritize and Aggregate Product Requirements"@en ;
    rdfs:subClassOf scor:PlanSource ;
    olo:next scor:IdentifyAssessAggregateProductResources;
    skos:notation "sP2.1" ;
    rdfs:isDefinedBy scor: ;
    vs:term_status "testing" ;
    dct:modified "2015-11-05"^^xsd:date ;
 .

scor:IdentifyAssessAggregateProductResources
    rdf:type owl:Class ;
    rdfs:comment "The process of identifying, evaluating, and considering, as a whole with constituent parts, all material and other resources used to add value in the supply chain for a product or services."@en ;
    rdfs:label "Identify, Assess and Aggregate Product Resources"@en ;
    rdfs:subClassOf scor:PlanSource ;
    skos:notation "sP2.2" ;
    olo:next scor:BalanceProductResourcesWithProductRequirements;
    rdfs:isDefinedBy scor: ;
    vs:term_status "testing" ;
    dct:modified "2015-11-05"^^xsd:date ;
 .

scor:BalanceProductResourcesWithProductRequirements
    rdf:type owl:Class ;
    rdfs:comment "The process of developing a time-phased course of action that commits resources to meet requirements."@en ;
    rdfs:label "Balance Product Resources with Product Requirements"@en ;
    rdfs:subClassOf scor:PlanSource ;
    olo:next scor:EstablishSourcingPlans;
    skos:notation "sP2.3" ;
    rdfs:isDefinedBy scor: ;
    vs:term_status "testing" ;
    dct:modified "2015-11-05"^^xsd:date ;
 .

scor:EstablishSourcingPlans
    rdf:type owl:Class ;
    rdfs:comment "The establishment of courses of action over specified time periods that represent a projected appropriation of supply resources to meet sourcing plan requirements."@en ;
    rdfs:label "Establish Sourcing Plans"@en ;
    rdfs:subClassOf scor:PlanSource ;
    skos:notation "sP2.4" ;
    rdfs:isDefinedBy scor: ;
    vs:term_status "testing" ;
    dct:modified "2015-11-05"^^xsd:date ;
 .

# Plan Make

scor:IdentifyPrioritizeAggregateProductionRequirements
    rdf:type owl:Class ;
    rdfs:comment "The process of identifying, prioritizing, and considering as a whole with constituent parts, all sources of demand in the creation of a product or service."@en ;
    rdfs:label "Identify, Prioritize and Aggregate Production Requirements"@en ;
    rdfs:subClassOf scor:PlanMake ;
    olo:next scor:IdentifyAssessAggregateProductionResources;
    skos:notation "sP3.1" ;
    rdfs:isDefinedBy scor: ;
    vs:term_status "testing" ;
    dct:modified "2015-11-05"^^xsd:date ;
 .

scor:IdentifyAssessAggregateProductionResources
    rdf:type owl:Class ;
    rdfs:comment "The process of identifying, evaluating, and considering, as a whole with constituent parts, all things that add value in the creation of a product or performance of a service."@en ;
    rdfs:label "Identify, Assess and Aggregate Production Resources"@en ;
    rdfs:subClassOf scor:PlanMake ;
    olo:next scor:BalanceProductionResourcesWithProductionRequirements;
    skos:notation "sP3.2" ;
    rdfs:isDefinedBy scor: ;
    vs:term_status "testing" ;
    dct:modified "2015-11-05"^^xsd:date ;
 .

scor:BalanceProductionResourcesWithProductionRequirements
    rdf:type owl:Class ;
    rdfs:comment "The process of developing a time-phased course of action that commits creation and operation resources to meet creation and operation requirements."@en ;
    rdfs:label "Balance Production Resources with Production Requirements"@en ;
    rdfs:subClassOf scor:PlanMake ;
    olo:next scor:EstablishProductionPlans;
    skos:notation "sP3.3" ;
    rdfs:isDefinedBy scor: ;
    vs:term_status "testing" ;
    dct:modified "2015-11-05"^^xsd:date ;
 .

scor:EstablishProductionPlans
    rdf:type owl:Class ;
    rdfs:comment "The establishment of courses of action over specified time periods that represent a projected appropriation of supply resources to meet production and operating plan requirements."@en ;
    rdfs:label "Establish Production Plans"@en ;
    rdfs:subClassOf scor:PlanMake ;
    skos:notation "sP3.4" ;
    rdfs:isDefinedBy scor: ;
    vs:term_status "testing" ;
    dct:modified "2015-11-05"^^xsd:date ;
 .

# Plan Deliver

scor:IdentifyPrioritizeAggregateDeliveryRequirements
    rdf:type owl:Class ;
    rdfs:comment "The process of identifying, prioritizing, and considering, as a whole with constituent parts, all sources of demand in the delivery of a product or service."@en ;
    rdfs:label "Identify, Prioritize and Aggregate Delivery Requirements"@en ;
    rdfs:subClassOf scor:PlanDeliver ;
    olo:next scor:IdentifyAssessAggregateDeliveryResources;
    skos:notation "sP4.1" ;
    rdfs:isDefinedBy scor: ;
    vs:term_status "testing" ;
    dct:modified "2015-11-05"^^xsd:date ;
 .

scor:IdentifyAssessAggregateDeliveryResources
    rdf:type owl:Class ;
    rdfs:comment "The process of identifying, evaluating, and considering, as a whole with constituent parts, all things that add value in the delivery of a product or service."@en ;
    rdfs:label "Identify, Assess and Aggregate Delivery Resources"@en ;
    rdfs:subClassOf scor:PlanDeliver ;
    olo:next scor:BalanceDeliveryResourcesCapabilitiesWithDeliveryRequirements;
    skos:notation "sP4.2" ;
    rdfs:isDefinedBy scor: ;
    vs:term_status "testing" ;
    dct:modified "2015-11-05"^^xsd:date ;
 .

scor:BalanceDeliveryResourcesCapabilitiesWithDeliveryRequirements
    rdf:type owl:Class ;
    rdfs:comment "The process of developing a time-phased course of action that commits delivery resources to meet delivery requirements."@en ;
    rdfs:label "Balance Delivery Resources and Capabilities with Delivery Requirements"@en ;
    rdfs:subClassOf scor:PlanDeliver ;
    olo:next scor:EstablishDeliveryPlans;
    skos:notation "sP4.3" ;
    rdfs:isDefinedBy scor: ;
    vs:term_status "testing" ;
    dct:modified "2015-11-05"^^xsd:date ;
 .

scor:EstablishDeliveryPlans
    rdf:type owl:Class ;
    rdfs:comment "The establishment of courses of action over specified time periods that represent a projected appropriation of delivery resources to meet delivery requirements."@en ;
    rdfs:label "Establish Delivery Plans"@en ;
    rdfs:subClassOf scor:PlanDeliver ;
    skos:notation "sP4.4" ;
    rdfs:isDefinedBy scor: ;
    vs:term_status "testing" ;
    dct:modified "2015-11-05"^^xsd:date ;
 .

# Plan Return

scor:AssessAggregateReturnRequirements
    rdf:type owl:Class ;
    rdfs:comment "The process of identifying, evaluating, and considering, as a whole with constituent parts, all sources of demand for the return of a product."@en ;
    rdfs:label "Assess and Aggregate Return Requirements"@en ;
    rdfs:subClassOf scor:PlanReturn ;
    olo:next scor:IdentifyAssessAggregateReturnResources;
    skos:notation "sP5.1" ;
    rdfs:isDefinedBy scor: ;
    vs:term_status "testing" ;
    dct:modified "2015-11-05"^^xsd:date ;
 .

scor:IdentifyAssessAggregateReturnResources
    rdf:type owl:Class ;
    rdfs:comment "The process of identifying, evaluating, and consideration for all resources that add value to, execute, or constrain the processes for the return of a product.."@en ;
    rdfs:label "Identify, Assess and Aggregate Return Resources"@en ;
    rdfs:subClassOf scor:PlanReturn ;
    olo:next scor:BalanceReturnResourcesWithReturnRequirements;
    skos:notation "sP5.2" ;
    rdfs:isDefinedBy scor: ;
    vs:term_status "testing" ;
    dct:modified "2015-11-05"^^xsd:date ;
 .

scor:BalanceReturnResourcesWithReturnRequirements
    rdf:type owl:Class ;
    rdfs:comment "The process of developing courses of action that make feasible the commitment the appropriate return resources and or assets to satisfy return requirements."@en ;
    rdfs:label "Balance Return Resources with Return Requirements"@en ;
    rdfs:subClassOf scor:PlanReturn ;
    olo:next scor:EstablishCommunicateReturnPlans;
    skos:notation "sP5.3" ;
    rdfs:isDefinedBy scor: ;
    vs:term_status "testing" ;
    dct:modified "2015-11-05"^^xsd:date ;
 .

scor:EstablishCommunicateReturnPlans
    rdf:type owl:Class ;
    rdfs:comment "The establishment and communication of courses of action over specified time periods that represent a projected appropriation of required return resources and or assets to meet return process requirements."@en ;
    rdfs:label "Establish and Communicate Return Plans"@en ;
    rdfs:subClassOf scor:PlanReturn ;
    skos:notation "sP5.4" ;
    rdfs:isDefinedBy scor: ;
    vs:term_status "testing" ;
    dct:modified "2015-11-05"^^xsd:date ;
 .

# Source Stocked Product

scor:SSPScheduleProductDeliveries
    rdf:type owl:Class ;
    rdfs:comment "Scheduling and managing the execution of the individual deliveries of product against an existing contract or purchase order."@en ;
    rdfs:label "Schedule Product Deliveries (Source Stocked Product)"@en ;
    rdfs:subClassOf scor:SourceStockedProduct ;
    skos:notation "sS1.1" ;
    olo:next scor:SSPReceiveProduct;
    rdfs:isDefinedBy scor: ;
    vs:term_status "testing" ;
    dct:modified "2015-11-05"^^xsd:date ;
 .

scor:SSPReceiveProduct
    rdf:type owl:Class ;
    rdfs:comment "The process and associated activities of receiving product to contract requirements."@en ;
    rdfs:label "Receive Product (Source Stocked Product)"@en ;
    rdfs:subClassOf scor:SourceStockedProduct ;
    skos:notation "sS1.2" ;
    olo:next scor:SSPVerifyProduct;
    rdfs:isDefinedBy scor: ;
    vs:term_status "testing" ;
    dct:modified "2015-11-05"^^xsd:date ;
 .

scor:SSPVerifyProduct
    rdf:type owl:Class ;
    rdfs:comment "The process and associated activities of receiving product to contract requirements."@en ;
    rdfs:label "Verify Product (Source Stocked Product)"@en ;
    rdfs:subClassOf scor:SourceStockedProduct ;
    olo:next scor:SSPTransferProduct;
    skos:notation "sS1.3" ;
    rdfs:isDefinedBy scor: ;
    vs:term_status "testing" ;
    dct:modified "2015-11-05"^^xsd:date ;
 .

scor:SSPTransferProduct
    rdf:type owl:Class ;
    rdfs:comment "The transfer of accepted product to the appropriate stocking location within the supply chain."@en ;
    rdfs:label "Transfer Product (Source Stocked Product)"@en ;
    rdfs:subClassOf scor:SourceStockedProduct ;
    olo:next scor:AuthorizeSupplierPayment;
    skos:notation "sS1.4" ;
    rdfs:isDefinedBy scor: ;
    vs:term_status "testing" ;
    dct:modified "2015-11-05"^^xsd:date ;
 .

scor:AuthorizeSupplierPayment
    rdf:type owl:Class ;
    rdfs:comment "The process of authorizing payments and paying suppliers for product or services."@en ;
    rdfs:label "Authorize Supplier Payment (Source Stocked Product)"@en ;
    rdfs:subClassOf scor:SourceStockedProduct ;
    skos:notation "sS1.5" ;
    rdfs:isDefinedBy scor: ;
    vs:term_status "testing" ;
    dct:modified "2015-11-05"^^xsd:date ;
 .

# Source MakeToOrderProduct

scor:MOPScheduleProductDeliveries
    rdf:type owl:Class ;
    rdfs:comment "Scheduling and managing the execution of the individual deliveries of product against the contract."@en ;
    rdfs:label "Schedule Product Deliveries (Source Make To Order Product)"@en ;
    rdfs:subClassOf scor:SourceMakeToOrderProduct ;
    olo:next scor:MOPScheduleProductDeliveries;
    skos:notation "sS2.1" ;
    rdfs:isDefinedBy scor: ;
    vs:term_status "testing" ;
    dct:modified "2015-11-05"^^xsd:date ;
 .

scor:SMOPReceiveProduct
    rdf:type owl:Class ;
    rdfs:comment "The process and associated activities of receiving product to contract requirements."@en ;
    rdfs:label "Receive Product (Source Make To Order Product)"@en ;
    rdfs:subClassOf scor:SourceMakeToOrderProduct ;
    olo:next scor:SMOPVerifyProduct;
    skos:notation "sS2.2" ;
    rdfs:isDefinedBy scor: ;
    vs:term_status "testing" ;
    dct:modified "2015-11-05"^^xsd:date ;
 .

scor:SMOPVerifyProduct
    rdf:type owl:Class ;
    rdfs:comment "The process and actions required determining product conformance to requirements and criteria."@en ;
    rdfs:label "Verify Product (Source Make To Order Product)"@en ;
    rdfs:subClassOf scor:SourceMakeToOrderProduct ;
    olo:next scor:SMOPTransferProduct;
    skos:notation "sS2.3" ;
    rdfs:isDefinedBy scor: ;
    vs:term_status "testing" ;
    dct:modified "2015-11-05"^^xsd:date ;
 .

scor:SMOPTransferProduct
    rdf:type owl:Class ;
    rdfs:comment "The transfer of accepted product to the appropriate stocking location within the supply chain."@en ;
    rdfs:label "Transfer Product (Source Make To Order Product)"@en ;
    rdfs:subClassOf scor:SourceMakeToOrderProduct ;
    olo:next scor:SMOPAuthorizeSupplierPayment;
    skos:notation "sS2.4" ;
    rdfs:isDefinedBy scor: ;
    vs:term_status "testing" ;
    dct:modified "2015-11-05"^^xsd:date ;
 .

scor:SMOPAuthorizeSupplierPayment
    rdf:type owl:Class ;
    rdfs:comment "The process of authorizing payments and paying suppliers for product or services."@en ;
    rdfs:label "Supplier Payment (Source Make To Order Product)"@en ;
    rdfs:subClassOf scor:SourceMakeToOrderProduct ;
    skos:notation "sS2.4" ;
    rdfs:isDefinedBy scor: ;
    vs:term_status "testing" ;
    dct:modified "2015-11-05"^^xsd:date ;
 .

# SourceEngineerToOrderProduct

scor:IdentifySourcesOfSupply
    rdf:type owl:Class ;
    rdfs:comment "The identification and qualification of potential suppliers capable of designing and delivering product that will meet all of the required product specifications."@en ;
    rdfs:label "Identify Sources of Supply"@en ;
    rdfs:subClassOf scor:SourceEngineerToOrderProduct ;
    olo:next scor:SelectFinalSupplierNegotiate;
    skos:notation "sS3.1" ;
    rdfs:isDefinedBy scor: ;
    vs:term_status "testing" ;
    dct:modified "2015-11-05"^^xsd:date ;
 .

scor:SelectFinalSupplierNegotiate
    rdf:type owl:Class ;
    rdfs:comment "The identification of the final supplier(s) based on the evaluation of RFQs, supplier qualifications and the generation of a contract defining the costs and terms and conditions of product availability."@en ;
    rdfs:label "Select Final Supplier and Negotiate"@en ;
    rdfs:subClassOf scor:SourceEngineerToOrderProduct ;
    olo:next scor:SEOPScheduleProductDeliveries;
    skos:notation "sS3.2" ;
    rdfs:isDefinedBy scor: ;
    vs:term_status "testing" ;
    dct:modified "2015-11-05"^^xsd:date ;
 .

scor:SEOPScheduleProductDeliveries
    rdf:type owl:Class ;
    rdfs:comment "Scheduling and managing the execution of the individual deliveries of product against the contract."@en ;
    rdfs:label "Schedule Product Deliveries (Source Engineer To Order Product)"@en ;
    rdfs:subClassOf scor:SourceEngineerToOrderProduct ;
    olo:next scor:SEOPReceiveProduct;
    skos:notation "sS3.3" ;
    rdfs:isDefinedBy scor: ;
    vs:term_status "testing" ;
    dct:modified "2015-11-05"^^xsd:date ;
 .

scor:SEOPReceiveProduct
    rdf:type owl:Class ;
    rdfs:comment "The process and associated activities of receiving product to contract requirements."@en ;
    rdfs:label "Receive Product (Source Engineer To Order Product)"@en ;
    rdfs:subClassOf scor:SourceEngineerToOrderProduct ;
    olo:next scor:SEOPVerifyProduct;
    skos:notation "sS3.4" ;
    rdfs:isDefinedBy scor: ;
    vs:term_status "testing" ;
    dct:modified "2015-11-05"^^xsd:date ;
 .

scor:SEOPVerifyProduct
    rdf:type owl:Class ;
    rdfs:comment "The process and actions required determining product conformance to requirements and criteria."@en ;
    rdfs:label "Verify Product (Source Engineer To Order Product)"@en ;
    rdfs:subClassOf scor:SourceEngineerToOrderProduct ;
    olo:next scor:SEOPTransferProduct;
    skos:notation "sS3.5" ;
    rdfs:isDefinedBy scor: ;
    vs:term_status "testing" ;
    dct:modified "2015-11-05"^^xsd:date ;
 .

scor:SEOPTransferProduct
    rdf:type owl:Class ;
    rdfs:comment "The transfer of accepted product to the appropriate stocking location within the supply chain."@en ;
    rdfs:label "Transfer Product (Source Engineer To Order Product)"@en ;
    rdfs:subClassOf scor:SourceEngineerToOrderProduct ;
    olo:next scor:SEOPAuthorizeSupplierPayment;
    skos:notation "sS3.6" ;
    rdfs:isDefinedBy scor: ;
    vs:term_status "testing" ;
    dct:modified "2015-11-05"^^xsd:date ;
 .

scor:SEOPAuthorizeSupplierPayment
    rdf:type owl:Class ;
    rdfs:comment "The process of authorizing payments and paying suppliers for product or services. This process includes invoice collection, invoice matching and the issuance of checks."@en ;
    rdfs:label "Authorize Supplier Payment (Source Engineer To Order Product)"@en ;
    rdfs:subClassOf scor:SourceEngineerToOrderProduct ;
    skos:notation "sS3.7" ;
    rdfs:isDefinedBy scor: ;
    vs:term_status "testing" ;
    dct:modified "2015-11-05"^^xsd:date ;
 .

# Make MakeToStock

scor:MSScheduleProductionActivities
    rdf:type owl:Class ;
    rdfs:comment "Given plans for the production of specific parts, products, or formulations in specified quantities and planned availability of required sourced products, the scheduling of the operations to be performed in accordance with these plans."@en ;
    rdfs:label "Schedule Production Activities (Make To Stock)"@en ;
    rdfs:subClassOf scor:MakeToStock ;
    olo:next scor:IssueMaterial;
    skos:notation "sM1.1" ;
    rdfs:isDefinedBy scor: ;
    vs:term_status "testing" ;
    dct:modified "2015-11-05"^^xsd:date ;
 .

scor:IssueMaterial
    rdf:type owl:Class ;
    rdfs:comment "The selection and physical movement of sourced/in-process product (e.g., raw materials, fabricated components, subassemblies, required ingredients or intermediate formulations) from a stocking location (e.g., stockroom, a location on the production floor, a supplier) to a specific point of use location."@en ;
    rdfs:label "Issue Material"@en ;
    rdfs:subClassOf scor:MakeToStock ;
    olo:next scor:MSProduceTest;
    skos:notation "sM1.2" ;
    rdfs:isDefinedBy scor: ;
    vs:term_status "testing" ;
    dct:modified "2015-11-05"^^xsd:date ;
 .

scor:MSProduceTest
    rdf:type owl:Class ;
    rdfs:comment "The series of activities performed upon sourced/in-process product to convert it from the raw or semi-finished state to a state of completion and greater value."@en ;
    rdfs:label "Produce and Test (Make To Stock)"@en ;
    rdfs:subClassOf scor:MakeToStock ;
    olo:next scor:MSPackage;
    skos:notation "sM1.3" ;
    rdfs:isDefinedBy scor: ;
    vs:term_status "testing" ;
    dct:modified "2015-11-05"^^xsd:date ;
 .

scor:MSPackage
    rdf:type owl:Class ;
    rdfs:comment "The series of activities that containerize completed products for storage or sale to end-users."@en ;
    rdfs:label "Package (Make To Stock)"@en ;
    rdfs:subClassOf scor:MakeToStock ;
    olo:next scor:StageProduct;
    skos:notation "sM1.4" ;
    rdfs:isDefinedBy scor: ;
    vs:term_status "testing" ;
    dct:modified "2015-11-05"^^xsd:date ;
 .

scor:StageProduct
    rdf:type owl:Class ;
    rdfs:comment "The movement of packaged products into a temporary holding location to await movement to a finished goods location."@en ;
    rdfs:label "Stage Product"@en ;
    rdfs:subClassOf scor:MakeToStock ;
    olo:next scor:ReleaseProductToDeliver;
    skos:notation "sM1.5" ;
    rdfs:isDefinedBy scor: ;
    vs:term_status "testing" ;
    dct:modified "2015-11-05"^^xsd:date ;
 .

scor:ReleaseProductToDeliver
    rdf:type owl:Class ;
    rdfs:comment "Activities associated with post-production documentation, testing, or certification required prior to delivery of finished product to customer."@en ;
    rdfs:label "Release Product to Deliver (Make To Stock)"@en ;
    rdfs:subClassOf scor:MakeToStock ;
    olo:next scor:MSWasteDisposal;
    skos:notation "sM1.6" ;
    rdfs:isDefinedBy scor: ;
    vs:term_status "testing" ;
    dct:modified "2015-11-05"^^xsd:date ;
 .

scor:MSWasteDisposal
    rdf:type owl:Class ;
    rdfs:comment "Activities associated with collecting and managing waste produced during the produce and test process including scrap material and non-conforming product."@en ;
    rdfs:label "Waste Disposal (Make To Stock)"@en ;
    rdfs:subClassOf scor:MakeToStock ;
    skos:notation "sM1.7" ;
    rdfs:isDefinedBy scor: ;
    vs:term_status "testing" ;
    dct:modified "2015-11-05"^^xsd:date ;
 .

# Make MakeToOrder

scor:MOScheduleProductionActivities
    rdf:type owl:Class ;
    rdfs:comment "Given plans for the production of specific parts, products, or formulations in specific quantities and planned availability of required sourced products, the scheduling of the operations to be preformed in accordance with these plans."@en ;
    rdfs:label "Schedule Production Activities (Make To Order)"@en ;
    rdfs:subClassOf scor:MakeToOrder ;
    olo:next scor:IssueSourcedInProcessProduct;
    skos:notation "sM2.1" ;
    rdfs:isDefinedBy scor: ;
    vs:term_status "testing" ;
    dct:modified "2015-11-05"^^xsd:date ;
 .

scor:IssueSourcedInProcessProduct
    rdf:type owl:Class ;
    rdfs:comment "The selection and physical movement of sourced/in-process products (e.g., raw materials, fabricated components, subassemblies, required ingredients or intermediate formulations) from a stocking location (e.g., stockroom, a location on the production floor, a supplier) to a specific point of use location."@en ;
    rdfs:label "Issue Sourced In-Process Product (Make To Order)"@en ;
    rdfs:subClassOf scor:MakeToOrder ;
    olo:next scor:MOProduceTest;
    skos:notation "sM2.2" ;
    rdfs:isDefinedBy scor: ;
    vs:term_status "testing" ;
    dct:modified "2015-11-05"^^xsd:date ;
 .

scor:MOProduceTest
    rdf:type owl:Class ;
    rdfs:comment "The series of activities performed upon sourced/in-process product to convert it from the raw or semi-finished state to a state of completion and greater value."@en ;
    rdfs:label "Produce and Test (Make to Order)"@en ;
    rdfs:subClassOf scor:MakeToOrder ;
    olo:next scor:MOPackage;
    skos:notation "sM2.3" ;
    rdfs:isDefinedBy scor: ;
    vs:term_status "testing" ;
    dct:modified "2015-11-05"^^xsd:date ;
 .

scor:MOPackage
    rdf:type owl:Class ;
    rdfs:comment "The series of activities that containerize completed products for storage or sale to end-users."@en ;
    rdfs:label "Package (Make To Order)"@en ;
    rdfs:subClassOf scor:MakeToOrder ;
    olo:next scor:StageFinishedProduct;
    skos:notation "sM2.4" ;
    rdfs:isDefinedBy scor: ;
    vs:term_status "testing" ;
    dct:modified "2015-11-05"^^xsd:date ;
 .

scor:StageFinishedProduct
    rdf:type owl:Class ;
    rdfs:comment "The movement of packaged products into a temporary holding location to await movement to a finished goods location."@en ;
    rdfs:label "Stage Finished Product (Make To Order)"@en ;
    rdfs:subClassOf scor:MakeToOrder ;
    olo:next scor:ReleaseFinishedProductToDeliver;
    skos:notation "sM2.5" ;
    rdfs:isDefinedBy scor: ;
    vs:term_status "testing" ;
    dct:modified "2015-11-05"^^xsd:date ;
 .

scor:ReleaseFinishedProductToDeliver
    rdf:type owl:Class ;
    rdfs:comment "Activities associated with post-production documentation, testing, or certification required prior to delivery of finished product to customer."@en ;
    rdfs:label "Release Finished Product to Deliver"@en ;
    rdfs:subClassOf scor:MakeToOrder ;
    olo:next scor:MOWasteDisposal;
    skos:notation "sM2.6" ;
    rdfs:isDefinedBy scor: ;
    vs:term_status "testing" ;
    dct:modified "2015-11-05"^^xsd:date ;
 .

scor:MOWasteDisposal
    rdf:type owl:Class ;
    rdfs:comment "Activities associated with collecting and managing waste produced during the produce and test process including scrap material and non-conforming product."@en ;
    rdfs:label "Waste Disposal (Make To Order)"@en ;
    rdfs:subClassOf scor:MakeToOrder ;
    skos:notation "sM2.7" ;
    rdfs:isDefinedBy scor: ;
    vs:term_status "testing" ;
    dct:modified "2015-11-05"^^xsd:date ;
 .

# Make Engineer to Order

scor:FinalizeProductionEngineering
    rdf:type owl:Class ;
    rdfs:comment "Engineering activities required after acceptance of order, but before product can be produced. May include generation and delivery of final drawings, specifications, formulas, part programs, etc."@en ;
    rdfs:label "Finalize Production Engineering"@en ;
    rdfs:subClassOf scor:MakeEngineerToOrder ;
    olo:next scor:MEOScheduleProductionActivities;
    skos:notation "sM3.1" ;
    rdfs:isDefinedBy scor: ;
    vs:term_status "testing" ;
    dct:modified "2015-11-05"^^xsd:date ;
 .

scor:MEOScheduleProductionActivities
    rdf:type owl:Class ;
    rdfs:comment "Given plans for the production of specific parts, products, or formulations in specified quantities and planned availability of required sourced products, the scheduling of the operations to be performed in accordance with these plans"@en ;
    rdfs:label "Schedule Production Activities (Engineer To Order)"@en ;
    rdfs:subClassOf scor:MakeEngineerToOrder ;
    olo:next scor:MEOSourcedInProcessProduct;
    skos:notation "sM3.2" ;
    rdfs:isDefinedBy scor: ;
    vs:term_status "testing" ;
    dct:modified "2015-11-05"^^xsd:date ;
 .

scor:MEOSourcedInProcessProduct
    rdf:type owl:Class ;
    rdfs:comment "The selection and physical movement of sourced/in-process products (e.g., raw materials, fabricated components, subassemblies, required ingredients or intermediate formulations) from a stocking location (e.g., stockroom, a location on the production floor, a supplier) to a specific point of use location"@en ;
    rdfs:label "Issue Sourced In-Process Product (Engineer To Order)"@en ;
    rdfs:subClassOf scor:MakeEngineerToOrder ;
    olo:next scor:MEOProduceTest;
    skos:notation "sM3.3" ;
    rdfs:isDefinedBy scor: ;
    vs:term_status "testing" ;
    dct:modified "2015-11-05"^^xsd:date ;
 .

scor:MEOProduceTest
    rdf:type owl:Class ;
    rdfs:comment "The series of activities performed upon sourced/in-process product to convert it from the raw or semi-finished state to a state of completion and greater value"@en ;
    rdfs:label "Produce and Test (Engineer to Order)"@en ;
    rdfs:subClassOf scor:MakeEngineerToOrder ;
    olo:next scor:MEOPackage;
    skos:notation "sM3.4" ;
    rdfs:isDefinedBy scor: ;
    vs:term_status "testing" ;
    dct:modified "2015-11-05"^^xsd:date ;
 .

scor:MEOPackage
    rdf:type owl:Class ;
    rdfs:comment "The series of activities that containerize completed products for storage or sale to end-users."@en ;
    rdfs:label "Package (Engineer To Order)"@en ;
    rdfs:subClassOf scor:MakeEngineerToOrder ;
    olo:next scor:MEOStageFinishedProduct;
    skos:notation "sM3.5" ;
    rdfs:isDefinedBy scor: ;
    vs:term_status "testing" ;
    dct:modified "2015-11-05"^^xsd:date ;
 .

scor:MEOStageFinishedProduct
    rdf:type owl:Class ;
    rdfs:comment "The movement of packaged products into a temporary holding location to await movement to a finished goods location."@en ;
    rdfs:label "Stage Finished Product (Engineer To Order)"@en ;
    rdfs:subClassOf scor:MakeEngineerToOrder ;
    olo:next scor:MEOReleaseProductToDeliver;
    skos:notation "sM3.6" ;
    rdfs:isDefinedBy scor: ;
    vs:term_status "testing" ;
    dct:modified "2015-11-05"^^xsd:date ;
 .

scor:MEOReleaseProductToDeliver
    rdf:type owl:Class ;
    rdfs:comment "Activities associated with post-production documentation, testing, or certification required prior to delivery of finished product to customer."@en ;
    rdfs:label "Release Product to Deliver (Engineer To Order)"@en ;
    rdfs:subClassOf scor:MakeEngineerToOrder ;
    olo:next scor:MEOWasteDisposal;
    skos:notation "sM3.7" ;
    rdfs:isDefinedBy scor: ;
    vs:term_status "testing" ;
    dct:modified "2015-11-05"^^xsd:date ;
 .

scor:MEOWasteDisposal
    rdf:type owl:Class ;
    rdfs:comment "Activities associated with collecting and managing waste produced during the produce and test process including scrap material and non-conforming product."@en ;
    rdfs:label "Waste Disposal (Engineer To Order)"@en ;
    rdfs:subClassOf scor:MakeEngineerToOrder ;
    skos:notation "sM3.8" ;
    rdfs:isDefinedBy scor: ;
    vs:term_status "testing" ;
    dct:modified "2015-11-05"^^xsd:date ;
 .

# Deliver Stocked Product

scor:ProcessInquiryQuote
    rdf:type owl:Class ;
    rdfs:comment "Receive and respond to general customer inquiries and requests for quotes."@en ;
    rdfs:label "Process Inquiry and Quote (Deliver Stocked Product)"@en ;
    rdfs:subClassOf scor:DeliverStockedProduct ;
    olo:next scor:ReceiveEnterValidateOrder;
    skos:notation "sD1.1" ;
    rdfs:isDefinedBy scor: ;
    vs:term_status "testing" ;
    dct:modified "2015-11-05"^^xsd:date ;
 .

scor:ReceiveEnterValidateOrder
    rdf:type owl:Class ;
    rdfs:comment "Receive orders from the customer and enter them into a company's order processing system."@en ;
    rdfs:label "Receive, Enter, and Validate Order"@en ;
    rdfs:subClassOf scor:DeliverStockedProduct ;
    olo:next scor:DSPReserveInventoryDetermineDeliveryDate;
    skos:notation "sD1.2" ;
    rdfs:isDefinedBy scor: ;
    vs:term_status "testing" ;
    dct:modified "2015-11-05"^^xsd:date ;
 .

scor:DSPReserveInventoryDetermineDeliveryDate
    rdf:type owl:Class ;
    rdfs:comment "Inventory (both on hand and scheduled) is identified and reserved for specific orders and a delivery date is committed and scheduled."@en ;
    rdfs:label "Reserve Inventory and Determine Delivery Date (Deliver Stocked Product)"@en ;
    rdfs:subClassOf scor:DeliverStockedProduct ;
    olo:next scor:DSPConsolidateOrders;
    skos:notation "sD1.3" ;
    rdfs:isDefinedBy scor: ;
    vs:term_status "testing" ;
    dct:modified "2015-11-05"^^xsd:date ;
 .

scor:DSPConsolidateOrders
    rdf:type owl:Class ;
    rdfs:comment "The process of analyzing orders to determine the groupings that result in least cost/best service fulfillment and transportation."@en ;
    rdfs:label "Consolidate Orders (Deliver Stocked Product)"@en ;
    rdfs:subClassOf scor:DeliverStockedProduct ;
    olo:next scor:BuildLoads;
    skos:notation "sD1.4" ;
    rdfs:isDefinedBy scor: ;
    vs:term_status "testing" ;
    dct:modified "2015-11-05"^^xsd:date ;
 .

scor:BuildLoads
    rdf:type owl:Class ;
    rdfs:comment "Transportation modes are selected and efficient loads are built."@en ;
    rdfs:label "Build Loads (Deliver Stocked Product)"@en ;
    rdfs:subClassOf scor:DeliverStockedProduct ;
    olo:next scor:DSPRouteShipments;
    skos:notation "sD1.5" ;
    rdfs:isDefinedBy scor: ;
    vs:term_status "testing" ;
    dct:modified "2015-11-05"^^xsd:date ;
 .

scor:DSPRouteShipments
    rdf:type owl:Class ;
    rdfs:comment "Loads are consolidated and routed by mode, lane and location."@en ;
    rdfs:label "Route Shipments (Deliver Stocked Product)"@en ;
    rdfs:subClassOf scor:DeliverStockedProduct ;
    olo:next scor:SelectCarriersRateShipments;
    skos:notation "sD1.6" ;
    rdfs:isDefinedBy scor: ;
    vs:term_status "testing" ;
    dct:modified "2015-11-05"^^xsd:date ;
 .

scor:SelectCarriersRateShipments
    rdf:type owl:Class ;
    rdfs:comment "Specific carriers are selected by lowest cost per route and shipments are rated and tendered."@en ;
    rdfs:label "Select Carriers and Rate Shipments (Deliver Stocked Product)"@en ;
    rdfs:subClassOf scor:DeliverStockedProduct ;
    olo:next scor:ReceiveProductFromSourceMake;
    skos:notation "sD1.7" ;
    rdfs:isDefinedBy scor: ;
    vs:term_status "testing" ;
    dct:modified "2015-11-05"^^xsd:date ;
 .

scor:ReceiveProductFromSourceMake
    rdf:type owl:Class ;
    rdfs:comment "The activities such as receiving product, verifying, recording product receipt, determining put-away location, putting away and recording location that a company performs at its own warehouses."@en ;
    rdfs:label "Receive Product from Source or Make (Deliver Stocked Product)"@en ;
    rdfs:subClassOf scor:DeliverStockedProduct ;
    olo:next scor:PickProduct;
    skos:notation "sD1.8" ;
    rdfs:isDefinedBy scor: ;
    vs:term_status "testing" ;
    dct:modified "2015-11-05"^^xsd:date ;
 .

scor:PickProduct
    rdf:type owl:Class ;
    rdfs:comment "The series of activities including retrieving orders to pick, determining inventory availability, building the pick wave, picking the product, recording the pick and delivering product to shipping in response to an order."@en ;
    rdfs:label "Pick Product (Deliver Stocked Product)"@en ;
    rdfs:subClassOf scor:DeliverStockedProduct ;
    olo:next scor:PackProduct;
    skos:notation "sD1.9" ;
    rdfs:isDefinedBy scor: ;
    vs:term_status "testing" ;
    dct:modified "2015-11-05"^^xsd:date ;
 .

scor:PackProduct
    rdf:type owl:Class ;
    rdfs:comment "The activities such as sorting / combining the products, packing / kitting the products, paste labels, barcodes etc. and delivering the products to the shipping area for loading."@en ;
    rdfs:label "Pack Product (Deliver Stocked Product)"@en ;
    rdfs:subClassOf scor:DeliverStockedProduct ;
    olo:next scor:LoadVehicleGenerateShippingDocuments;
    skos:notation "sD1.10" ;
    rdfs:isDefinedBy scor: ;
    vs:term_status "testing" ;
    dct:modified "2015-11-05"^^xsd:date ;
 .

scor:LoadVehicleGenerateShippingDocuments
    rdf:type owl:Class ;
    rdfs:comment "The series of tasks including placing/loading product onto modes of transportation, and generating the documentation necessary to meet internal, customer, carrier and government needs."@en ;
    rdfs:label "Load Vehicle and Generate Shipping Documents"@en ;
    rdfs:subClassOf scor:DeliverStockedProduct ;
    olo:next scor:DeliverStockedProduct;
    skos:notation "sD1.11" ;
    rdfs:isDefinedBy scor: ;
    vs:term_status "testing" ;
    dct:modified "2015-11-05"^^xsd:date ;
 .

scor:DSPShipProduct
    rdf:type owl:Class ;
    rdfs:comment "The process of shipping the product to the customer site."@en ;
    rdfs:label "Ship Product (Deliver Stocked Product)"@en ;
    rdfs:subClassOf scor:DeliverStockedProduct ;
    olo:next scor:DSPReceiveVerifyProductByCustomer;
    skos:notation "sD1.12" ;
    rdfs:isDefinedBy scor: ;
    vs:term_status "testing" ;
    dct:modified "2015-11-05"^^xsd:date ;
 .

scor:DSPReceiveVerifyProductByCustomer
    rdf:type owl:Class ;
    rdfs:comment "The process of receiving the shipment by the customer (either at customer site or at shipping area in case of self-collection) and verifying that the order was shipped complete and that the product meets delivery terms."@en ;
    rdfs:label "Receive and verify Product by Customer (Deliver Stocked Product)"@en ;
    rdfs:subClassOf scor:DeliverStockedProduct ;
    olo:next scor:InstallProduct;
    skos:notation "sD1.13" ;
    rdfs:isDefinedBy scor: ;
    vs:term_status "testing" ;
    dct:modified "2015-11-05"^^xsd:date ;
 .

scor:InstallProduct
    rdf:type owl:Class ;
    rdfs:comment "the process of preparing, testing and installing the product at the customer site. The product is fully functional upon completion."@en ;
    rdfs:label "Install Product (Deliver Stocked Product)"@en ;
    rdfs:subClassOf scor:DeliverStockedProduct ;
    olo:next scor:DSPInvoice;
    skos:notation "sD1.14" ;
    rdfs:isDefinedBy scor: ;
    vs:term_status "testing" ;
    dct:modified "2015-11-05"^^xsd:date ;
 .

scor:DSPInvoice
    rdf:type owl:Class ;
    rdfs:comment "A signal is sent to the financial organization that the order has been shipped and that the billing process should begin and payment be received or be closed out if payment has already been received."@en ;
    rdfs:label "Invoice (Deliver Stocked Product)"@en ;
    rdfs:subClassOf scor:DeliverStockedProduct ;
    skos:notation "sD1.15" ;
    rdfs:isDefinedBy scor: ;
    vs:term_status "testing" ;
    dct:modified "2015-11-05"^^xsd:date ;
 .

# Deliver Make-to-Order Product

scor:DeliverMakeToOrderProductProcessInquiryQuote
    rdf:type owl:Class ;
    rdfs:comment "Receive and respond to general customer inquiries and requests for quotes."@en ;
    rdfs:label "Process Inquiry and Quote (Deliver Make To Order Product)"@en ;
    rdfs:subClassOf scor:DeliverMakeToOrderProduct ;
    olo:next scor:ReceiveConfigureEnterValidateOrder;
    skos:notation "sD2.1" ;
    rdfs:isDefinedBy scor: ;
    vs:term_status "testing" ;
    dct:modified "2015-11-05"^^xsd:date ;
 .

scor:ReceiveConfigureEnterValidateOrder
    rdf:type owl:Class ;
    rdfs:comment "Receive orders from the customer and enter them into a company's order processing system."@en ;
    rdfs:label "Receive, Configure, Enter and Validate Order"@en ;
    rdfs:subClassOf scor:DeliverMakeToOrderProduct ;
    olo:next scor:DMOPReserveInventoryDetermineDeliveryDate;
    skos:notation "sD2.2" ;
    rdfs:isDefinedBy scor: ;
    vs:term_status "testing" ;
    dct:modified "2015-11-05"^^xsd:date ;
 .

scor:DMOPReserveInventoryDetermineDeliveryDate
    rdf:type owl:Class ;
    rdfs:comment "Inventory and/or planned capacity is identified and reserved for specific orders, and a delivery date is committed and scheduled."@en ;
    rdfs:label "Reserve Inventory and Determine Delivery Date (Deliver Make To Order Product)"@en ;
    rdfs:subClassOf scor:DeliverMakeToOrderProduct ;
    olo:next scor:DMOPConsolidateOrders;
    skos:notation "sD2.3" ;
    rdfs:isDefinedBy scor: ;
    vs:term_status "testing" ;
    dct:modified "2015-11-05"^^xsd:date ;
 .

scor:DMOPConsolidateOrders
    rdf:type owl:Class ;
    rdfs:comment "The process of analyzing orders to determine the groupings that result in least cost/best service fulfillment and transportation."@en ;
    rdfs:label "Consolidate Orders (Deliver Make To Order Product)"@en ;
    rdfs:subClassOf scor:DeliverMakeToOrderProduct ;
    olo:next scor:DeliverMakeToOrderProductProcessBuildLoads;
    skos:notation "sD2.4" ;
    rdfs:isDefinedBy scor: ;
    vs:term_status "testing" ;
    dct:modified "2015-11-05"^^xsd:date ;
 .

scor:DeliverMakeToOrderProductProcessBuildLoads
    rdf:type owl:Class ;
    rdfs:comment "Transportation modes are selected and efficient loads are built."@en ;
    rdfs:label "Build Loads (Deliver Make To Order Product)"@en ;
    rdfs:subClassOf scor:DeliverMakeToOrderProduct ;
    olo:next scor:DMOPRouteShipments;
    skos:notation "sD2.5" ;
    rdfs:isDefinedBy scor: ;
    vs:term_status "testing" ;
    dct:modified "2015-11-05"^^xsd:date ;
 .

scor:DMOPRouteShipments
    rdf:type owl:Class ;
    rdfs:comment "Loads are consolidated and routed by mode, lane, and location."@en ;
    rdfs:label "Route Shipments (Deliver Make To Order Product)"@en ;
    rdfs:subClassOf scor:DeliverMakeToOrderProduct ;
    olo:next scor:DMOPSelectCarriersRateShipments;
    skos:notation "sD2.6" ;
    rdfs:isDefinedBy scor: ;
    vs:term_status "testing" ;
    dct:modified "2015-11-05"^^xsd:date ;
 .

scor:DMOPSelectCarriersRateShipments
    rdf:type owl:Class ;
    rdfs:comment "Specific carriers are selected by lowest cost per route and shipments are rated and tendered."@en ;
    rdfs:label "Select Carriers and Rate Shipments (Deliver Make To Order Product)"@en ;
    rdfs:subClassOf scor:DeliverMakeToOrderProduct ;
    olo:next scor:DMOPReceiveProductFromSourceMake;
    skos:notation "sD2.7" ;
    rdfs:isDefinedBy scor: ;
    vs:term_status "testing" ;
    dct:modified "2015-11-05"^^xsd:date ;
 .

scor:DMOPReceiveProductFromSourceMake
    rdf:type owl:Class ;
    rdfs:comment "The activities such as receiving product, verifying, recording product receipt, determining put-away location, putting away and recording location for goods received from either Make or Source."@en ;
    rdfs:label "Receive Product from Source or Make (Deliver Make To Order Product)"@en ;
    olo:next scor:DMOPReceiveProductFromSourceMake;
    rdfs:subClassOf scor:DMOPPickProduct ;
    skos:notation "sD2.8" ;
    rdfs:isDefinedBy scor: ;
    vs:term_status "testing" ;
    dct:modified "2015-11-05"^^xsd:date ;
 .

scor:DMOPPickProduct
    rdf:type owl:Class ;
    rdfs:comment "The series of activities including retrieving orders to pick, verifying inventory availability, building the pick wave, picking the product, recording the pick and delivering product to packing area in response to an order."@en ;
    rdfs:label "Pick Product (Deliver Make To Order Product)"@en ;
    rdfs:subClassOf scor:DeliverMakeToOrderProduct ;
    olo:next scor:DMOPPackProduct;
    skos:notation "sD2.9" ;
    rdfs:isDefinedBy scor: ;
    vs:term_status "testing" ;
    dct:modified "2015-11-05"^^xsd:date ;
 .

scor:DMOPPackProduct
    rdf:type owl:Class ;
    rdfs:comment "The activities such as sorting / combining the products, packing / kitting the products, paste labels, barcodes etc. and delivering the products to the shipping area for loading."@en ;
    rdfs:label "Pack Product (Make To Order Product)"@en ;
    rdfs:subClassOf scor:DeliverMakeToOrderProduct ;
    olo:next scor:DMOPLoadProductGenerateShippingDocs;
    skos:notation "sD2.10" ;
    rdfs:isDefinedBy scor: ;
    vs:term_status "testing" ;
    dct:modified "2015-11-05"^^xsd:date ;
 .

scor:DMOPLoadProductGenerateShippingDocs
    rdf:type owl:Class ;
    rdfs:comment "The series of tasks including placing/loading product onto modes of transportation, and generating the documentation necessary to meet internal, customer, carrier and government needs."@en ;
    rdfs:label "Load Product Generate Shipping Docs"@en ;
    rdfs:subClassOf scor:DeliverMakeToOrderProduct ;
    olo:next scor:DMOPShipProduct;
    skos:notation "sD2.11" ;
    rdfs:isDefinedBy scor: ;
    vs:term_status "testing" ;
    dct:modified "2015-11-05"^^xsd:date ;
 .

scor:DMOPShipProduct
    rdf:type owl:Class ;
    rdfs:comment "The process of shipping the product to the customer site."@en ;
    rdfs:label "Ship Product (Deliver Make To Order Product)"@en ;
    rdfs:subClassOf scor:DeliverMakeToOrderProduct ;
    olo:next scor:DMOPReceiveVerifyProductByCustomer;
    skos:notation "sD2.12" ;
    rdfs:isDefinedBy scor: ;
    vs:term_status "testing" ;
    dct:modified "2015-11-05"^^xsd:date ;
 .

scor:DMOPReceiveVerifyProductByCustomer
    rdf:type owl:Class ;
    rdfs:comment "The process of receiving the shipment at the customer (either at customer site or at shipping area in case of self-collection) and verifying that the order was shipped complete and that the product meets delivery terms."@en ;
    rdfs:label "Receive and verify Product by Customer (Deliver Make To Order Product)"@en ;
    rdfs:subClassOf scor:DeliverMakeToOrderProduct ;
    olo:next scor:DeliverMakeToOrderProduct;
    skos:notation "sD2.13" ;
    rdfs:isDefinedBy scor: ;
    vs:term_status "testing" ;
    dct:modified "2015-11-05"^^xsd:date ;
 .

scor:DeliverMakeToOrderProductInstallProduct
    rdf:type owl:Class ;
    rdfs:comment "the process of preparing, testing and installing the product at the customer site."@en ;
    rdfs:label "Install Product (Deliver Make To Order Product)"@en ;
    rdfs:subClassOf scor:DeliverMakeToOrderProduct ;
    olo:next scor:DMOPInvoice;
    skos:notation "sD2.14" ;
    rdfs:isDefinedBy scor: ;
    vs:term_status "testing" ;
    dct:modified "2015-11-05"^^xsd:date ;
 .

scor:DMOPInvoice
    rdf:type owl:Class ;
    rdfs:comment "A signal is sent to the financial organization that the order has been shipped and that the billing process should begin and payment be received or be closed out if payment has already been received."@en ;
    rdfs:label "Invoice (Deliver Make To Order Product)"@en ;
    rdfs:subClassOf scor:DeliverMakeToOrderProduct ;
    skos:notation "sD2.15" ;
    rdfs:isDefinedBy scor: ;
    vs:term_status "testing" ;
    dct:modified "2015-11-05"^^xsd:date ;
 .

# Deliver Engineer-to-Order Product

scor:ObtainRespondToRFPRFQ
    rdf:type owl:Class ;
    rdfs:comment "The process of receiving a request for proposal or request for quote, evaluating the request (estimating the schedule, developing costs estimates, establishing price), and responding to the potential customer."@en ;
    rdfs:label "Obtain and Respond to RFP-RFQ"@en ;
    rdfs:subClassOf scor:DeliverEngineerToOrderProduct ;
    olo:next scor:NegotiateReceiveContract;
    skos:notation "sD3.1" ;
    rdfs:isDefinedBy scor: ;
    vs:term_status "testing" ;
    dct:modified "2015-11-05"^^xsd:date ;
 .

scor:NegotiateReceiveContract
    rdf:type owl:Class ;
    rdfs:comment "The process of negotiating order details with customer (e.g., price, schedule, product performance) and finalizing the contract."@en ;
    rdfs:label "Negotiate and Receive Contract"@en ;
    rdfs:subClassOf scor:DeliverEngineerToOrderProduct ;
    olo:next scor:EnterOrderCommitResourcesLaunchProgram;
    skos:notation "sD3.2" ;
    rdfs:isDefinedBy scor: ;
    vs:term_status "testing" ;
    dct:modified "2015-11-05"^^xsd:date ;
 .

scor:EnterOrderCommitResourcesLaunchProgram
    rdf:type owl:Class ;
    rdfs:comment "The process of entering/finalizing the customers order, approving the planned resources (e.g., engineering, manufacturing, etc.) and officially launching the program."@en ;
    rdfs:label "Enter Order, Commit Resources Launch Program"@en ;
    rdfs:subClassOf scor:DeliverEngineerToOrderProduct ;
    olo:next scor:ScheduleInstallation;
    skos:notation "sD3.3" ;
    rdfs:isDefinedBy scor: ;
    vs:term_status "testing" ;
    dct:modified "2015-11-05"^^xsd:date ;
 .

scor:ScheduleInstallation
    rdf:type owl:Class ;
    rdfs:comment "The process of evaluating the design and build schedules relative to customer requested installation date to determine installation schedule."@en ;
    rdfs:label "Schedule Installation"@en ;
    rdfs:subClassOf scor:DeliverEngineerToOrderProduct ;
    olo:next scor:DEOPBuildLoads;
    skos:notation "sD3.4" ;
    rdfs:isDefinedBy scor: ;
    vs:term_status "testing" ;
    dct:modified "2015-11-05"^^xsd:date ;
 .

scor:DEOPBuildLoads
    rdf:type owl:Class ;
    rdfs:comment "The process of evaluating the design and build schedules relative to customer requested installation date to determine installation schedule."@en ;
    rdfs:label "Build Loads (Deliver Engineer To Order Product)"@en ;
    rdfs:subClassOf scor:DeliverEngineerToOrderProduct ;
    olo:next scor:DEOPRouteShipments;
    skos:notation "sD3.5" ;
    rdfs:isDefinedBy scor: ;
    vs:term_status "testing" ;
    dct:modified "2015-11-05"^^xsd:date ;
 .

scor:DEOPRouteShipments
    rdf:type owl:Class ;
    rdfs:comment "Loads are consolidated and routed by mode, lane, and location."@en ;
    rdfs:label "Route Shipments (Deliver Engineer To Order Product)"@en ;
    rdfs:subClassOf scor:DeliverEngineerToOrderProduct ;
    olo:next scor:DEOPSelectCarriersRateShipments;
    skos:notation "sD3.6" ;
    rdfs:isDefinedBy scor: ;
    vs:term_status "testing" ;
    dct:modified "2015-11-05"^^xsd:date ;
 .

scor:DEOPSelectCarriersRateShipments
    rdf:type owl:Class ;
    rdfs:comment "Specific carriers are selected by lowest cost per route and shipments are rated and tendered."@en ;
    rdfs:label "Select Carriers Rate Shipments"@en ;
    rdfs:subClassOf scor:DeliverEngineerToOrderProduct ;
    olo:next scor:DEOPReceiveProductFromSourceMake;
    skos:notation "sD3.7" ;
    rdfs:isDefinedBy scor: ;
    vs:term_status "testing" ;
    dct:modified "2015-11-05"^^xsd:date ;
 .

scor:DEOPReceiveProductFromSourceMake
    rdf:type owl:Class ;
    rdfs:comment "The activities such as receiving product, verifying, recording product receipt, determining put-away location, putting away and recording location for goods received from either Make or Source."@en ;
    rdfs:label "Receive Product from Source or Make (Deliver Engineer To Order Product)"@en ;
    rdfs:subClassOf scor:DeliverEngineerToOrderProduct ;
    olo:next scor:DEOPPickProduct;
    skos:notation "sD3.8" ;
    rdfs:isDefinedBy scor: ;
    vs:term_status "testing" ;
    dct:modified "2015-11-05"^^xsd:date ;
 .

scor:DEOPPickProduct
    rdf:type owl:Class ;
    rdfs:comment "The series of activities including retrieving orders to pick, verifying inventory availability, building the pick wave, picking the product, recording the pick and delivering product to packing area in response to an order."@en ;
    rdfs:label "Pick Product (Deliver Engineer To Order Product)"@en ;
    rdfs:subClassOf scor:DeliverEngineerToOrderProduct ;
    olo:next scor:DEOPPackProduct;
    skos:notation "sD3.9" ;
    rdfs:isDefinedBy scor: ;
    vs:term_status "testing" ;
    dct:modified "2015-11-05"^^xsd:date ;
 .

scor:DEOPPackProduct
    rdf:type owl:Class ;
    rdfs:comment "The activities such as sorting / combining the products, packing / kitting the products, paste labels, barcodes etc. and delivering the products to the shipping area for loading."@en ;
    rdfs:label "Pack Product (Deliver Engineer To Order Product)"@en ;
    rdfs:subClassOf scor:DeliverEngineerToOrderProduct ;
    olo:next scor:DEOPLoadProductGenerateShippingDocs;
    skos:notation "sD3.10" ;
    rdfs:isDefinedBy scor: ;
    vs:term_status "testing" ;
    dct:modified "2015-11-05"^^xsd:date ;
 .

scor:DEOPLoadProductGenerateShippingDocs
    rdf:type owl:Class ;
    rdfs:comment "The series of tasks including placing/loading product onto modes of transportation, and generating the documentation necessary to meet internal, customer, carrier and government needs."@en ;
    rdfs:label "Load Product & Generate Shipping Docs"@en ;
    rdfs:subClassOf scor:DeliverEngineerToOrderProduct ;
    olo:next scor:DEOPShipProduct;
    skos:notation "sD3.11" ;
    rdfs:isDefinedBy scor: ;
    vs:term_status "testing" ;
    dct:modified "2015-11-05"^^xsd:date ;
 .

scor:DEOPShipProduct
    rdf:type owl:Class ;
    rdfs:comment "The process of shipping the product to the customer site."@en ;
    rdfs:label "Ship Product"@en ;
    rdfs:subClassOf scor:DeliverEngineerToOrderProduct ;
    olo:next scor:DEOPReceiveVerifyProductByCustomer;
    skos:notation "sD3.12" ;
    rdfs:isDefinedBy scor: ;
    vs:term_status "testing" ;
    dct:modified "2015-11-05"^^xsd:date ;
 .

scor:DEOPReceiveVerifyProductByCustomer
    rdf:type owl:Class ;
    rdfs:comment "The process of receiving the shipment (either at customer site or at shipping area in case of self-collection) and verifying that the order was shipped complete and that the product meets delivery terms."@en ;
    rdfs:label "Receive and verify Product by Customer (Deliver Engineer To Order Product)"@en ;
    rdfs:subClassOf scor:DeliverEngineerToOrderProduct ;
    olo:next scor:DEOPInstallProduct;
    skos:notation "sD3.13" ;
    rdfs:isDefinedBy scor: ;
    vs:term_status "testing" ;
    dct:modified "2015-11-05"^^xsd:date ;
 .

scor:DEOPInstallProduct
    rdf:type owl:Class ;
    rdfs:comment "The process of preparing, testing and installing the product at the customer site. The product is fully functional upon completion."@en ;
    rdfs:label "Install Product (Deliver Engineer To Order Product)"@en ;
    rdfs:subClassOf scor:DeliverEngineerToOrderProduct ;
    olo:next scor:DEOPInvoice;
    skos:notation "sD3.14" ;
    rdfs:isDefinedBy scor: ;
    vs:term_status "testing" ;
    dct:modified "2015-11-05"^^xsd:date ;
 .

scor:DEOPInvoice
    rdf:type owl:Class ;
    rdfs:comment "A signal is sent to the financial organization that the order has been shipped and that the billing process should begin and payment be received or be closed out if payment has already been received."@en ;
    rdfs:label "Invoice (Deliver Engineer To Order Product)"@en ;
    rdfs:subClassOf scor:DeliverEngineerToOrderProduct ;
    skos:notation "sD3.15" ;
    rdfs:isDefinedBy scor: ;
    vs:term_status "testing" ;
    dct:modified "2015-11-05"^^xsd:date ;
 .

# DeliverRetailProduct

scor:GenerateStockingSchedule
    rdf:type owl:Class ;
    rdfs:comment "The process of scheduling resources to support item-stocking requirements."@en ;
    rdfs:label "Generate Stocking Schedule"@en ;
    rdfs:subClassOf scor:DeliverRetailProduct ;
    olo:next scor:ReceiveProductAtStore;
    skos:notation "sD4.1" ;
    rdfs:isDefinedBy scor: ;
    vs:term_status "testing" ;
    dct:modified "2015-11-05"^^xsd:date ;
 .

scor:ReceiveProductAtStore
    rdf:type owl:Class ;
    rdfs:comment "The activities such as receiving product, verifying, recording product receipt, determining put-away location, putting away and recording location that a company performs at its own stores."@en ;
    rdfs:label "Receive Product at Store"@en ;
    rdfs:subClassOf scor:DeliverRetailProduct ;
    olo:next scor:PickProductFromBackroom;
    skos:notation "sD4.2" ;
    rdfs:isDefinedBy scor: ;
    vs:term_status "testing" ;
    dct:modified "2015-11-05"^^xsd:date ;
 .

scor:PickProductFromBackroom
    rdf:type owl:Class ;
    rdfs:comment "The process of retrieving restocking orders to pick, determining inventory availability, building a pick wave, picking item and quantity from a designated backroom warehouse location, recording the resulting inventory transaction, and delivering the product to point of stock."@en ;
    rdfs:label "Pick Product from backroom"@en ;
    rdfs:subClassOf scor:DeliverRetailProduct ;
    olo:next scor:StockShelf;
    skos:notation "sD4.3" ;
    rdfs:isDefinedBy scor: ;
    vs:term_status "testing" ;
    dct:modified "2015-11-05"^^xsd:date ;
 .

scor:StockShelf
    rdf:type owl:Class ;
    rdfs:comment "For restocks, the tasks associated with identifying the item location, stocking the shelf according to merchandise plans, and recording the appropriate inventory transaction."@en ;
    rdfs:label "Stock Shelf"@en ;
    rdfs:subClassOf scor:DeliverRetailProduct ;
    olo:next scor:FillShoppingCart;
    skos:notation "sD4.4" ;
    rdfs:isDefinedBy scor: ;
    vs:term_status "testing" ;
    dct:modified "2015-11-05"^^xsd:date ;
 .

scor:FillShoppingCart
    rdf:type owl:Class ;
    rdfs:comment "Typical set of tasks associated with product selection, storage and movement through to checkout."@en ;
    rdfs:label "Fill Shopping Cart"@en ;
    rdfs:subClassOf scor:DeliverRetailProduct ;
    olo:next scor:Checkout;
    skos:notation "sD4.5" ;
    rdfs:isDefinedBy scor: ;
    vs:term_status "testing" ;
    dct:modified "2015-11-05"^^xsd:date ;
 .

scor:Checkout
    rdf:type owl:Class ;
    rdfs:comment "The processes and tasks associated with product checkout including scanning, method of payment, credit application and approval, service agreement, order confirmation, and/or invoice or receipt."@en ;
    rdfs:label "Checkout"@en ;
    rdfs:subClassOf scor:DeliverRetailProduct ;
    olo:next scor:DeliverInstall;
    skos:notation "sD4.6" ;
    rdfs:isDefinedBy scor: ;
    vs:term_status "testing" ;
    dct:modified "2015-11-05"^^xsd:date ;
 .

scor:DeliverInstall
    rdf:type owl:Class ;
    rdfs:comment "The process of preparing and installing the product at the customer site. The product is fully functional upon completion."@en ;
    rdfs:label "Deliver and/or install"@en ;
    rdfs:subClassOf scor:DeliverRetailProduct ;
    skos:notation "sD4.7" ;
    rdfs:isDefinedBy scor: ;
    vs:term_status "testing" ;
    dct:modified "2015-11-05"^^xsd:date ;
 .

# Source Return Defective Product

scor:IdentifyDefectiveProductCondition
    rdf:type owl:Class ;
    rdfs:comment "The process where the customer utilizes planned policies, business rules and product operating conditions inspection as criteria to identify and confirm that material is excess to requirements defective."@en ;
    rdfs:label "Identify Defective Product Condition"@en ;
    olo:next scor:DispositionDefectiveProduct;
    rdfs:subClassOf scor:SourceReturnDefectiveProduct ;
    skos:notation "sSR1.1" ;
    rdfs:isDefinedBy scor: ;
    vs:term_status "testing" ;
    dct:modified "2015-11-05"^^xsd:date ;
.

scor:DispositionDefectiveProduct 
    rdf:type owl:Class ;
    rdfs:comment "The process of the customer determining whether to return the defective item and the appropriate source contact for a return authorization."@en ;
    rdfs:label "Disposition Defective Product"@en ;
    rdfs:subClassOf scor:SourceReturnDefectiveProduct ;
    olo:next scor:RequestDefectiveProductReturnAuthorization;
    skos:notation "sSR1.2" ;
    rdfs:isDefinedBy scor: ;
    vs:term_status "testing" ;
    dct:modified "2015-11-05"^^xsd:date ;
.

scor:RequestDefectiveProductReturnAuthorization
    rdf:type owl:Class ;
    rdfs:comment "The process of a customer requesting and obtaining authorization, from last known holder or designated return center, for the return of defective product. Additionally, the customer and last known holder or designated return center would discuss enabling conditions such as return replacement or credit, packaging, handling, transportation and import / export requirements to facilitate the efficient return of the defective product."@en ;
    rdfs:label "Request Defective Product Return Authorization"@en ;
    rdfs:subClassOf scor:SourceReturnDefectiveProduct ;
    olo:next scor:ScheduleDefectiveProductShipment;
    skos:notation "sSR1.3" ;
    rdfs:isDefinedBy scor: ;
    vs:term_status "testing" ;
    dct:modified "2015-11-05"^^xsd:date ;
.

scor:ScheduleDefectiveProductShipment
    rdf:type owl:Class ;
    rdfs:comment "The process where the customer develops the schedule for a carrier to pick-up for delivery of the defective product. Activities include selecting the carrier and rates, preparing the item for transfer, preparing scheduling documentation and managing overall scheduling administration."@en ;
    rdfs:label "Schedule Defective Product Shipment"@en ;
    rdfs:subClassOf scor:SourceReturnDefectiveProduct ;
    olo:next scor:ReturnDefectiveProduct;
    skos:notation "sSR1.4" ;
    rdfs:isDefinedBy scor: ;
    vs:term_status "testing" ;
    dct:modified "2015-11-05"^^xsd:date ;
.

scor:ReturnDefectiveProduct
    rdf:type owl:Class ;
    rdfs:comment "The process where the customer packages, and handles the defective product in preparation for shipping in accord with pre-determined conditions. The product is then provided by the customer to the carrier who physically transports the product and its associated documentation to the last known holder or designated return center."@en ;
    rdfs:label "Return Defective Product"@en ;
    rdfs:subClassOf scor:SourceReturnDefectiveProduct ;
    skos:notation "sSR1.5" ;
    rdfs:isDefinedBy scor: ;
    vs:term_status "testing" ;
    dct:modified "2015-11-05"^^xsd:date ;
.
# Deliver Return Defective Product

scor:AuthorizeDefectiveProductReturn
    rdf:type owl:Class ;
    rdfs:comment "The process where the last known holder or designated return center receives a defective product return authorization request from a customer, determines if the item can be accepted and communicates decision to the customer. Accepting the request would include negotiating the conditions of the return with the customer, including authorizing return replacement or credit. Rejecting the request would include providing a reason for the rejection to the customer."@en ;
    rdfs:label "Authorize Defective Product Return"@en ;
    rdfs:subClassOf scor:DeliverReturnDefectiveProduct ;
    olo:next scor:ScheduleDefectiveReturnReceipt;
    skos:notation "sDR1.1" ;
    rdfs:isDefinedBy scor: ;
    vs:term_status "testing" ;
    dct:modified "2015-11-05"^^xsd:date ;
.

scor:ScheduleDefectiveReturnReceipt
    rdf:type owl:Class ;
    rdfs:comment "The process where the last known holder or designated return center evaluates the defective product handling requirements including negotiated conditions and develops a schedule that tells the Customer when to ship the product. The scheduling activity would also inform Receiving when to expect the shipment and where to send the product, for disposition, upon receipt."@en ;
    rdfs:label "Schedule Defective Return Receipt"@en ;
    rdfs:subClassOf scor:DeliverReturnDefectiveProduct ;
    olo:next scor:ReceiveDefectiveProduct;
    skos:notation "sDR1.2" ;
    rdfs:isDefinedBy scor: ;
    vs:term_status "testing" ;
    dct:modified "2015-11-05"^^xsd:date ;
.

scor:ReceiveDefectiveProduct
    rdf:type owl:Class ;
    rdfs:comment "The process where the last known holder or designated return center receives and verifies the returned defective product against the return authorization and other documentation and prepares the item for transfer."@en ;
    rdfs:label "Receive Defective Product"@en ;
    rdfs:subClassOf scor:DeliverReturnDefectiveProduct ;
    olo:next scor:TransferDefectiveProduct;
    skos:notation "sDR1.3" ;
    rdfs:isDefinedBy scor: ;
    vs:term_status "testing" ;
    dct:modified "2015-11-05"^^xsd:date ;
.

scor:TransferDefectiveProduct
    rdf:type owl:Class ;
    rdfs:comment "The process where the last known holder or designated return center transfers the defective product to the appropriate process to implement the disposition decision."@en ;
    rdfs:label "Transfer Defective Product"@en ;
    rdfs:subClassOf scor:DeliverReturnDefectiveProduct ;
    skos:notation "sDR1.4" ;
    rdfs:isDefinedBy scor: ;
    vs:term_status "testing" ;
    dct:modified "2015-11-05"^^xsd:date ;
.


# Return MRO Product

scor:IdentifyMROProductCondition
    rdf:type owl:Class ;
    rdfs:comment "The process where the customer utilizes pre-determined MRO policies, business rules and product operating conditions as criteria to identify and confirm that an item requires maintenance, repair, overhaul or disposal. Includes operating failures and planned maintenance requirements."@en ;
    rdfs:label "Identify MRO Product Condition"@en ;
    rdfs:subClassOf scor:ReturnMROProduct ;
    olo:next scor:DispositionMROProduct;
    skos:notation "sSR2.1" ;
    rdfs:isDefinedBy scor: ;
    vs:term_status "testing" ;
    dct:modified "2015-11-05"^^xsd:date ;
.

scor:DispositionMROProduct
    rdf:type owl:Class ;
    rdfs:comment "The process of the customer determining whether to service the item, what service is required, and who the appropriate service provider would be to service the item. Outputs include a decision to: (1) send a return authorization request to a service provider, (2) send the product back into service without requiring a return authorization request, or (3) discard the item."@en ;
    rdfs:label "Disposition MRO Product"@en ;
    rdfs:subClassOf scor:ReturnMROProduct ;
    olo:next scor:RequestMROReturnAuthorization;
    skos:notation "sSR2.2" ;
    rdfs:isDefinedBy scor: ;
    vs:term_status "testing" ;
    dct:modified "2015-11-05"^^xsd:date ;
.

scor:RequestMROReturnAuthorization
    rdf:type owl:Class ;
    rdfs:comment "The process of a customer requesting and obtaining authorization, from a service provider, for the return of an MRO product. In addition to discussing the MRO issue, the customer and service provider would discuss enabling conditions such as return replacement or credit, packaging, handling, transportation and import / export requirements to facilitate the efficient return of the MRO product to the service provider. The customer may need to go through several return authorization iterations with multiple service providers before authorization is received."@en ;
    rdfs:label "Request MRO Return Authorization"@en ;
    rdfs:subClassOf scor:ReturnMROProduct ;
    olo:next scor:ScheduleMROShipment;
    skos:notation "sSR2.3" ;
    rdfs:isDefinedBy scor: ;
    vs:term_status "testing" ;
    dct:modified "2015-11-05"^^xsd:date ;
.

scor:ScheduleMROShipment
    rdf:type owl:Class ;
    rdfs:comment "The process where the customer develops the schedule for a carrier to pick-up and deliver the MRO product. Activities include selecting the carrier and rates, preparing the item for transfer, preparing scheduling documentation and managing overall scheduling administration."@en ;
    rdfs:label "Schedule MRO Shipment"@en ;
    rdfs:subClassOf scor:ReturnMROProduct ;
    olo:next scor:ReturnMROPRoduct;
    skos:notation "sSR2.4" ;
    rdfs:isDefinedBy scor: ;
    vs:term_status "testing" ;
    dct:modified "2015-11-05"^^xsd:date ;
.

scor:ReturnMROPRoduct
    rdf:type owl:Class ;
    rdfs:comment "The process where the customer packages, and handles the MRO product in preparation for shipping in accord with pre-determined conditions. The product is then provided by the customer to the carrier who physically transports the product and its associated documentation to the service provider."@en ;
    rdfs:label "Return MRO Shipment"@en ;
    rdfs:subClassOf scor:DeliverReturnMROProduct ;
    skos:notation "sSR2.5" ;
    rdfs:isDefinedBy scor: ;
    vs:term_status "testing" ;
    dct:modified "2015-11-05"^^xsd:date ;
.


# Deliver Return MRO Product

 scor:AuthorizeMROProductReturn
    rdf:type owl:Class ;
    rdfs:comment "The process where a service provider receives an MRO product return authorization request from a customer, determines if the item can be accepted for MRO and communicates their decision to the customer. Accepting the request would include negotiating the conditions of the return with the customer, including authorizing return replacement or credit. Rejecting the request would include providing a reason for the rejection to the customer."@en ;
    rdfs:label "Authorize MRO Product Return"@en ;
    rdfs:subClassOf scor:DeliverReturnMROProduct ;
    olo:next scor:ScheduleMROReturnReceipt;
    skos:notation "sDR2.1" ;
    rdfs:isDefinedBy scor: ;
    vs:term_status "testing" ;
    dct:modified "2015-11-05"^^xsd:date ;
.

 scor:ScheduleMROReturnReceipt
    rdf:type owl:Class ;
    rdfs:comment "The process where the service provider evaluates the MRO service requirements including negotiated conditions and develops a schedule that tells the Customer when to ship the part. The scheduling activity would also inform Receiving when to expect the shipment and where to send the part, for induction or storage, upon receipt."@en ;
    rdfs:label "Schedule MRO Return Receipt"@en ;
    rdfs:subClassOf scor:DeliverReturnMROProduct ;
    olo:next scor:ReceiveMROProduct;
    skos:notation "sDR2.2" ;
    rdfs:isDefinedBy scor: ;
    vs:term_status "testing" ;
    dct:modified "2015-11-05"^^xsd:date ;
.

 scor:ReceiveMROProduct
    rdf:type owl:Class ;
    rdfs:comment "The process where the service provider receives and verifies the returned MRO item against the return authorization and other documentation and prepares the item for transfer."@en ;
    rdfs:label "Receive MRO Product"@en ;
    rdfs:subClassOf scor:DeliverReturnMROProduct ;
    olo:next scor:TransferMROProduct;
    skos:notation "sDR2.3" ;
    rdfs:isDefinedBy scor: ;
    vs:term_status "testing" ;
    dct:modified "2015-11-05"^^xsd:date ;
.

 scor:TransferMROProduct
    rdf:type owl:Class ;
    rdfs:comment "The process where the service provider transfers the MRO product to the appropriate process to implement the disposition decision."@en ;
    rdfs:label "Transfer MRO Product"@en ;
    rdfs:subClassOf scor:DeliverReturnMROProduct ;
    skos:notation "sDR2.4" ;
    rdfs:isDefinedBy scor: ;
    vs:term_status "testing" ;
    dct:modified "2015-11-05"^^xsd:date ;
.


# Source Return Excess Product

 scor:IdentifyExcessProductCondition
    rdf:type owl:Class ;
    rdfs:comment "The process where the customer utilizes planned policies, business rules and product inspection as criteria to identify and confirm that material is in excess of the current requirements."@en ;
    rdfs:label "Identify Excess Product Condition"@en ;
    rdfs:subClassOf scor:SourceReturnExcessProduct ;
    olo:next scor:DispositionExcessProduct;
    skos:notation "sSR3.1" ;
    rdfs:isDefinedBy scor: ;
    vs:term_status "testing" ;
    dct:modified "2015-11-05"^^xsd:date ;
.

 scor:DispositionExcessProduct
    rdf:type owl:Class ;
    rdfs:comment "The process of the customer determining whether to return the excess material and identification of a designated return center a return authorization."@en ;
    rdfs:label "Disposition Excess Product"@en ;
    rdfs:subClassOf scor:SourceReturnExcessProduct ;
    olo:next scor:RequestExcessProductReturnAuthorization;
    skos:notation "sSR3.2" ;
    rdfs:isDefinedBy scor: ;
    vs:term_status "testing" ;
    dct:modified "2015-11-05"^^xsd:date ;
.

 scor:RequestExcessProductReturnAuthorization
    rdf:type owl:Class ;
    rdfs:comment "The process of a customer requesting and obtaining authorization, from the designated return center, for the return of excess product. Additionally, the customer and designated return center would negotiate enabling conditions such as return credit or cash discount, packaging, handling, transportation and import / export requirements to facilitate the efficient return of the excess product."@en ;
    rdfs:label "Request Excess Product Return Authorization"@en ;
    rdfs:subClassOf scor:SourceReturnExcessProduct ;
    olo:next scor:ScheduleExcessProductShipment;
    skos:notation "sSR3.3" ;
    rdfs:isDefinedBy scor: ;
    vs:term_status "testing" ;
    dct:modified "2015-11-05"^^xsd:date ;
.

 scor:ScheduleExcessProductShipment
    rdf:type owl:Class ;
    rdfs:comment "The process where the customer develops the schedule for a carrier to pick-up the excess product. Activities include selecting the carrier and rates, preparing the item for transfer, preparing scheduling documentation and managing overall scheduling administration."@en ;
    rdfs:label "Schedule Excess Product Shipment"@en ;
    rdfs:subClassOf scor:SourceReturnExcessProduct ;
    olo:next scor:ReturnExcessProduct;
    skos:notation "sSR3.4" ;
    rdfs:isDefinedBy scor: ;
    vs:term_status "testing" ;
    dct:modified "2015-11-05"^^xsd:date ;
.

 scor:ReturnExcessProduct
    rdf:type owl:Class ;
    rdfs:comment "The process where the customer packages, and handles the excess product in preparation for shipping in accord with pre-determined conditions. The product is then provided by the customer to the carrier who physically transports the product and its associated documentation to the last known holder or designated return center."@en ;
    rdfs:label "Return Excess Product"@en ;
    rdfs:subClassOf scor:SourceReturnExcessProduct ;
    skos:notation "sSR3.5" ;
    rdfs:isDefinedBy scor: ;
    vs:term_status "testing" ;
    dct:modified "2015-11-05"^^xsd:date ;
.

# Deliver Return Excess Product

 scor:AuthorizeExcessProductReturn
    rdf:type owl:Class ;
    rdfs:comment "The process where the designated return center receives an excess product return authorization request from a customer, determines if the item can be accepted and communicates their decision to the customer. Accepting the request would include negotiating the conditions of the return with the customer, including authorizing credit or cash discount. Rejecting the request would include providing a reason for the rejection to the customer."@en ;
    rdfs:label "Authorize Excess Product Return"@en ;
    rdfs:subClassOf scor:DeliverReturnExcessProduct ;
    olo:next scor:ScheduleExcessReturnReceipt;
    skos:notation "sDR3.1" ;
    rdfs:isDefinedBy scor: ;
    vs:term_status "testing" ;
    dct:modified "2015-11-05"^^xsd:date ;
.

 scor:ScheduleExcessReturnReceipt
    rdf:type owl:Class ;
    rdfs:comment "The process where the l designated return center evaluates an authorized excess material return toolsdetermine packaging and handling requirements. This assessment will lead to the development of a return disposition decision and a return schedule with terms and conditions that will tell the Customer how and when to ship the product. The scheduling activity would also inform the Return Center?s Receiving department when to expect the shipment and where to send the product, for disposition, upon receipt."@en ;
    rdfs:label "Schedule Excess Return Receipt"@en ;
    rdfs:subClassOf scor:DeliverReturnExcessProduct ;
    olo:next scor:ReceiveExcessProduct;
    skos:notation "sDR3.2" ;
    rdfs:isDefinedBy scor: ;
    vs:term_status "testing" ;
    dct:modified "2015-11-05"^^xsd:date ;
.

 scor:ReceiveExcessProduct
    rdf:type owl:Class ;
    rdfs:comment "The process where the designated return center receives and verifies the returned excess product and associated documentation against the return authorization and other documentation and prepares the item for transfer. Administrate any discrepancies that arise."@en ;
    rdfs:label "Receive Excess Product"@en ;
    rdfs:subClassOf scor:DeliverReturnExcessProduct ;
    olo:next scor:TransferExcessProduct;
    skos:notation "sDR3.3" ;
    rdfs:isDefinedBy scor: ;
    vs:term_status "testing" ;
    dct:modified "2015-11-05"^^xsd:date ;
.

 scor:TransferExcessProduct
    rdf:type owl:Class ;
    rdfs:comment "The process where the designated return center transfers the excess product to the appropriate process to implement the disposition decision."@en ;
    rdfs:label "Transfer Excess Product"@en ;
    rdfs:subClassOf scor:DeliverReturnExcessProduct ;
    skos:notation "sDR3.4" ;
    rdfs:isDefinedBy scor: ;
    vs:term_status "testing" ;
    dct:modified "2015-11-05"^^xsd:date ;
.

#############################################################################################
#############################################################################################
#############################################################################################
#### Properties

scor:hasStep
    rdf:type owl:ObjectProperty ;
    rdfs:label "has Step"@en ;
    rdfs:domain scor:Process ;
    rdfs:range  scor:Process ;
    rdfs:comment "Steps which are part of a certain process"@en  ;
    rdfs:isDefinedBy scor: ;
    vs:term_status "testing" ;
    dct:modified "2015-11-05"^^xsd:date ;
 .

scor:hasAptitude
    rdf:type rdf:Property ;
    rdfs:domain scor:Skill ;
    rdfs:range scor:Aptitude ;
    rdfs:comment "An aptitude required for certain skills"@en  ;
    rdfs:label "has Aptitude"@en  ;
    rdfs:isDefinedBy scor: ;
    vs:term_status "testing" ;
    dct:modified "2015-11-05"^^xsd:date ;
 .

scor:hasExperience
    rdf:type rdf:Property ;
    rdfs:domain scor:Skill ;
    rdfs:range scor:Experience ;
    rdfs:label "has Experience"@en  ;
    rdfs:comment "An Experience required for certain skills"@en  ;
    rdfs:isDefinedBy scor: ;
    vs:term_status "testing" ;
    dct:modified "2015-11-05"^^xsd:date ;
 .

scor:hasSkill
    rdf:type rdf:Property ;
    rdfs:domain schema:Person ;
    rdfs:label "has Skill"@en  ;
    rdfs:comment "A Skill of a Person"@en  ;
    rdfs:range scor:Skill ;
    rdfs:isDefinedBy scor: ;
    vs:term_status "testing" ;
    dct:modified "2015-11-05"^^xsd:date ;
 .

scor:hasTraining
    rdf:type rdf:Property ;
    rdfs:domain scor:Skill ;
    rdfs:label "has Training"@en  ;
    rdfs:comment "A Training required to gain a skill"@en  ;
    rdfs:range scor:Training ;
    rdfs:isDefinedBy scor: ;
    vs:term_status "testing" ;
    dct:modified "2015-11-05"^^xsd:date ;
 .

##########################################################################################
#### Metric Properties


scor:hasMetric
    rdf:type owl:DatatypeProperty ;
    rdfs:range xsd:float ;
    rdfs:isDefinedBy scor: ;
    rdfs:comment "A Meric related to Processes"@en ;
    rdfs:label "has Metric"@en;
    vs:term_status "testing" ;
    dct:modified "2015-11-05"^^xsd:date ;
 .


######### Reliability Metrics

scor:hasMetricRL_1 rdfs:domain scor:ReleaseProductToDeliver ;
    rdfs:label "# of complaints regarding missing environmental documentation"@en;
    rdfs:comment "The number of products released without proper environmental documentation as a percent of total products released"@en ;
    rdfs:subPropertyOf scor:hasMetric; 
    rdfs:isDefinedBy scor: ;
    vs:term_status "testing" ;
    dct:modified "2015-11-05"^^xsd:date ;
 .

scor:hasMetricRL_2 rdfs:domain scor:ReleaseProductToDeliver ;
    rdfs:label "# of recordkeeping related NOVs"@en;
    rdfs:comment "The number of recordkeeping related regulatory violations received per year"@en;
    rdfs:subPropertyOf scor:hasMetric; 
    rdfs:isDefinedBy scor: ;
    vs:term_status "testing" ;
    dct:modified "2015-11-05"^^xsd:date ;
 .

#3 seems to be deprecated #

scor:hasMetricRL_4 rdfs:domain [owl:unionOf (scor:PackProduct
                                           scor:PickProduct
                                           scor:SSPReceiveProduct)] ;
    rdfs:label "% correct material documentation"@en;
    rdfs:comment "The percent of total shipments that include the correct environmental documentation"@en;
    rdfs:subPropertyOf scor:hasMetric; 
    rdfs:isDefinedBy scor: ;
    vs:term_status "testing" ;
    dct:modified "2015-11-05"^^xsd:date ;
 .

scor:hasMetricRL_5 rdfs:domain [owl:unionOf (scor:ReturnDefectiveProduct
                                           scor:ReturnMROPRoduct
                                           scor:ReturnExcessProduct)] ;
    rdfs:label "% Error-freeReturns Shipped"@en;
    rdfs:comment "Percentage of Error-free Returns Shipped"@en;
    rdfs:isDefinedBy scor: ;
    rdfs:subPropertyOf scor:hasMetric; 
    vs:term_status "testing" ;
    dct:modified "2015-11-05"^^xsd:date ;
 .

scor:hasMetricRL_6 rdfs:domain scor:DispositionMROProduct ;
    rdfs:label "% Identified MROProducts ReturnedTo Service"@en;
    rdfs:comment "Percentage Identified MROProducts ReturnedTo Service"@en;
    rdfs:subPropertyOf scor:hasMetric;
    rdfs:isDefinedBy scor: ;
    vs:term_status "testing" ;
    dct:modified "2015-11-05"^^xsd:date ;
 .

scor:hasMetricRL_7 rdfs:domain scor:FillShoppingCart;
    rdfs:label "Item Location Accuracy"@en;
    rdfs:comment "Item Location Accuracy"@en;
    rdfs:subPropertyOf scor:hasMetric;
    rdfs:isDefinedBy scor: ;
    vs:term_status "testing" ;
    dct:modified "2015-11-05"^^xsd:date ;
 .

#8 seems to be deprecated

#9 seems to be deprecated

scor:hasMetricRL_10 rdfs:domain [owl:unionOf (scor:SourceReturnExcessProduct
                                            scor:DeliverReturnExcessProduct)] ;
    rdfs:label "% of Excess Product Returns Delivered Complete to the Designated Return Center"@en;
    rdfs:comment "Correct destination, according to the schedule, with the correct part and documentation"@en;
    rdfs:subPropertyOf scor:hasMetric;
    rdfs:isDefinedBy scor: ;
    vs:term_status "testing" ;
    dct:modified "2015-11-05"^^xsd:date ;
 .

scor:hasMetricRL_11 rdfs:domain [owl:unionOf (scor:DSPInvoice
                                            scor:DMOPInvoice
                                            scor:DEOPInvoice)] ;
    rdfs:label "% of Faultless Invoices"@en;
    rdfs:comment "The number of invoices processed without issues and or errors divided by the total number of invoices. Examples of potential invoice defects are: Change from customer purchase order without proper customer involvement Wrong Customer Information (e.g., name, address, telephone number) Wrong Product Information (e.g., part number, product description) Wrong Price (e.g., discounts not applied) Wrong Quantity or Wrong Terms or Wrong Date"@en;
    rdfs:subPropertyOf scor:hasMetric;
    rdfs:isDefinedBy scor: ;
    vs:term_status "testing" ;
    dct:modified "2015-11-05"^^xsd:date ;
 .

scor:hasMetricRL_12 rdfs:domain scor:InstallProduct ;
    rdfs:label "% Of Faultless Installations"@en;
    rdfs:comment "Number of Faultless Installations divided by Total Number of Units Installed."@en;
    rdfs:subPropertyOf scor:hasMetric;
    rdfs:isDefinedBy scor: ;
    vs:term_status "testing" ;
    dct:modified "2015-11-05"^^xsd:date ;
 .

scor:hasMetricRL_13 rdfs:domain scor:DeliverReturnMROProduct ;
    rdfs:label "% of MRO returnsdelivered to the correct service provider location"@en;
    rdfs:comment "% of MRO returns delivered to the correct service provider location, within schedule, with the correct part and documentation"@en;
    rdfs:isDefinedBy scor: ;
    rdfs:subPropertyOf scor:hasMetric;
    vs:term_status "testing" ;
    dct:modified "2015-11-05"^^xsd:date ;
 .

scor:hasMetricRL_14 rdfs:domain scor:ReleaseFinishedProductToDeliver ;
    rdfs:label "% of products meeting specified environmental performance requirements"@en;
    rdfs:comment "The number of products that meet desired environmental performance specifications as a percent of total products produced"@en;
    rdfs:isDefinedBy scor: ;
    rdfs:subPropertyOf scor:hasMetric;
    vs:term_status "testing" ;
    dct:modified "2015-11-05"^^xsd:date ;
 .

scor:hasMetricRL_15 rdfs:domain scor:ReleaseFinishedProductToDeliver ;
    rdfs:label "% of products with proper environmental labeling (if required)"@en;
    rdfs:comment "The number of products with proper environmental labels in place as a per cent of total products produced"@en;
    rdfs:isDefinedBy scor: ;
    rdfs:subPropertyOf scor:hasMetric;
    vs:term_status "testing" ;
    dct:modified "2015-11-05"^^xsd:date ;
 .

scor:hasMetricRL_16 rdfs:domain scor:SelectCarriersRateShipments ;
    rdfs:label "% of suppliers meeting environmental metrics/ criteria"@en;
    rdfs:comment "Number of suppliers that completely meet agreement environmental criteria divided by the total number of suppliers used."@en;
    rdfs:isDefinedBy scor: ;
    rdfs:subPropertyOf scor:hasMetric;
    vs:term_status "testing" ;
    dct:modified "2015-11-05"^^xsd:date ;
 .

scor:hasMetricRL_17 rdfs:domain scor:SelectFinalSupplierNegotiate ;
    rdfs:label "% of suppliers with an EMS or ISO 14001 certification"@en;
    rdfs:comment "Percent of suppliers used that have a validated Environmental Management System or ISO 14000 certification"@en;
    rdfs:isDefinedBy scor: ;
    rdfs:subPropertyOf scor:hasMetric;
    vs:term_status "testing" ;
    dct:modified "2015-11-05"^^xsd:date ;
 .

scor:hasMetricRL_18 rdfs:domain [owl:unionOf (scor:SSPReceiveProduct
                                            scor:SMOPReceiveProduct
                                            scor:SEOPReceiveProduct)] ;
    rdfs:label "% Orders/ Lines Processed Complete"@en;
    rdfs:comment "The number of orders / lines that are processed complete divided by the total orders / lines processed within the measurement period"@en;
    rdfs:isDefinedBy scor: ;
    rdfs:subPropertyOf scor:hasMetric;
    vs:term_status "testing" ;
    dct:modified "2015-11-05"^^xsd:date ;
 .

scor:hasMetricRL_19 rdfs:domain [owl:unionOf (scor:SSPVerifyProduct
                                            scor:SMOPVerifyProduct
                                            scor:SEOPVerifyProduct)] ;
    rdfs:label "% Orders/ Lines Received Defect Free"@en;
    rdfs:comment "The number of orders / lines that are received defect free divided by the total orders / lines processed in the measurement period."@en;
    rdfs:isDefinedBy scor: ;
    rdfs:subPropertyOf scor:hasMetric;
    vs:term_status "testing" ;
    dct:modified "2015-11-05"^^xsd:date ;
 .

scor:hasMetricRL_20 rdfs:domain [owl:unionOf (scor:SSPReceiveProduct
                                            scor:SMOPReceiveProduct
                                            scor:SEOPReceiveProduct)] ;
    rdfs:label "% Orders/ Lines Received On-Time To Demand Requirement"@en;
    rdfs:comment "The number of orders / lines that are received on- time to the demand requirements divided by the total orders / lines for the demand requirements in the measurement period"@en;
    rdfs:subPropertyOf scor:hasMetric;
    rdfs:isDefinedBy scor: ;
    vs:term_status "testing" ;
    dct:modified "2015-11-05"^^xsd:date ;
 .

scor:hasMetricRL_21 rdfs:domain [owl:unionOf (scor:SSPVerifyProduct
                                            scor:SMOPVerifyProduct
                                            scor:SEOPVerifyProduct)] ;
    rdfs:label "% Orders/ lines received with correct content"@en;
    rdfs:comment "Percent of orders or lines received that have the correct material content as specified in the product design specs and supplier agreements."@en;
    rdfs:isDefinedBy scor: ;
    rdfs:subPropertyOf scor:hasMetric;
    vs:term_status "testing" ;
    dct:modified "2015-11-05"^^xsd:date ;
 .

 scor:hasMetricRL_22 rdfs:domain [owl:unionOf (scor:SSPReceiveProduct
                                            scor:SMOPReceiveProduct
                                            scor:SEOPReceiveProduct)] ;
    rdfs:label "% Orders/ lines received with correct packaging"@en;
    rdfs:comment "Percent of orders or lines received that are packaged correctly with the right type and quantity of packaging material."@en;
    rdfs:isDefinedBy scor: ;
    rdfs:subPropertyOf scor:hasMetric;
    vs:term_status "testing" ;
    dct:modified "2015-11-05"^^xsd:date ;
 .

scor:hasMetricRL_23 rdfs:domain [owl:unionOf (scor:SSPReceiveProduct
                                            scor:SMOPReceiveProduct
                                            scor:SEOPReceiveProduct)] ;
    rdfs:label "% Orders/ Lines Received with Correct Shipping Documents"@en;
    rdfs:comment "The number of orders / lines that are received on- time with correct shipping documents divided by the total orders / lines processed in the measurement period"@en;
    rdfs:isDefinedBy scor: ;
    rdfs:subPropertyOf scor:hasMetric;
    vs:term_status "testing" ;
    dct:modified "2015-11-05"^^xsd:date ;
 .

scor:hasMetricRL_24 rdfs:domain [owl:unionOf (scor:SSPVerifyProduct
                                            scor:SMOPVerifyProduct
                                            scor:SEOPVerifyProduct)] ;
    rdfs:label "% Orders/lines received damage free"@en;
    rdfs:comment "The number of orders / lines that are processed damage free divided by the total orders / Lines processed in the measurement period"@en;
    rdfs:isDefinedBy scor: ;
    rdfs:subPropertyOf scor:hasMetric;
    vs:term_status "testing" ;
    dct:modified "2015-11-05"^^xsd:date ;
 .

scor:hasMetricRL_25 rdfs:domain [owl:unionOf (scor:SSPTransferProduct
                                            scor:SMOPTransferProduct
                                            scor:SEOPTransferProduct)] ;
    rdfs:label "% Product Transferred On-Time to Demand Requirement"@en;
    rdfs:comment "The number of product orders / lines that are transferred on-time to demand requirements divided by the total orders / lines transferred in the measurement period"@en;
    rdfs:isDefinedBy scor: ;
    rdfs:subPropertyOf scor:hasMetric;
    vs:term_status "testing" ;
    dct:modified "2015-11-05"^^xsd:date ;
 .

scor:hasMetricRL_26 rdfs:domain [owl:unionOf (scor:SSPTransferProduct
                                            scor:SMOPTransferProduct
                                            scor:SEOPTransferProduct)] ;
    rdfs:label "% Product Transferred without Transaction Errors"@en;
    rdfs:comment "The number of transactions processed without error divided by the total transactions processed in the measurement period."@en;
    rdfs:isDefinedBy scor: ;
    rdfs:subPropertyOf scor:hasMetric;
    vs:term_status "testing" ;
    dct:modified "2015-11-05"^^xsd:date ;
 .

scor:hasMetricRL_27 rdfs:domain [owl:unionOf (scor:SSPScheduleProductDeliveries
                                            scor:MOPScheduleProductDeliveries
                                            scor:SEOPScheduleProductDeliveries)] ;
    rdfs:label "% Schedules Changed within Supplier's Lead Time"@en;
    rdfs:comment "The number of schedules that are changed within the suppliers lead-time divided by the total number Deliveries of schedules generated within the measurement period"@en;
    rdfs:subPropertyOf scor:hasMetric;
    rdfs:isDefinedBy scor: ;
    vs:term_status "testing" ;
    dct:modified "2015-11-05"^^xsd:date ;
 .

scor:hasMetricRL_28 rdfs:domain [owl:unionOf (scor:ScheduleDefectiveProductShipment
                                            scor:ScheduleMROShipment
                                            scor:ScheduleExcessProductShipment)] ;
    rdfs:label "% Shipping Schedules that Support Customer Required Return by Date"@en;
    rdfs:comment "Percentage Shipping Schedules that Support Customer Required Return by Date"@en;
    rdfs:isDefinedBy scor: ;
    rdfs:subPropertyOf scor:hasMetric;
    vs:term_status "testing" ;
    dct:modified "2015-11-05"^^xsd:date ;
 .

#29 seems to be deprecated

#30 seems to be deprecated

scor:hasMetricRL_31 rdfs:domain [owl:unionOf (scor:MSPackage
                                            scor:MOPackage
                                            scor:MEOPackage
                                            scor:LoadVehicleGenerateShippingDocuments
                                            scor:DMOPLoadProductGenerateShippingDocs
                                            scor:DEOPLoadProductGenerateShippingDocs)] ;
    rdfs:label "Compliance Documentation Accuracy"@en;
    rdfs:comment "Percentage of compliance documentations are complete, correct, and readily available when and  how expected by customer, Government and other supply chain regulatory entities. Compliance documentation includes material safety data sheets."@en;
    rdfs:isDefinedBy scor: ;
    rdfs:subPropertyOf scor:hasMetric;
    vs:term_status "testing" ;
    dct:modified "2015-11-05"^^xsd:date ;
 .

 

scor:hasMetricRL_32 rdfs:domain [owl:unionOf (scor:DSPReceiveVerifyProductByCustomer
                                            scor:DMOPReceiveVerifyProductByCustomer
                                            scor:DEOPReceiveVerifyProductByCustomer)] ;
    rdfs:label "Customer Commit Date Achievement Time"@en;
    rdfs:comment "Percentage of orders which is received on time as defined by the custome"@en;
    rdfs:isDefinedBy scor: ;
    vs:term_status "testing" ;
    rdfs:subPropertyOf scor:hasMetric;
    dct:modified "2015-11-05"^^xsd:date ;
 .

scor:hasMetricRL_33 rdfs:domain [owl:unionOf (scor:ReceiveEnterValidateOrder
                                            scor:DSPConsolidateOrders
                                            scor:LoadVehicleGenerateShippingDocuments
                                            scor:DSPShipProduct
                                            scor:DSPReceiveVerifyProductByCustomer
                                            scor:ReceiveConfigureEnterValidateOrder
                                            scor:DMOPConsolidateOrders
                                            scor:DMOPLoadProductGenerateShippingDocs
                                            scor:DMOPShipProduct
                                            scor:DMOPReceiveVerifyProductByCustomer
                                            scor:EnterOrderCommitResourcesLaunchProgram
                                            scor:DEOPRouteShipments
                                            scor:DEOPLoadProductGenerateShippingDocs
                                            scor:DEOPShipProduct
                                            scor:DMOPReceiveVerifyProductByCustomer)] ;
    rdfs:label "Delivery Item Accuracy"@en;
    rdfs:comment "Percentage of orders in which all items ordered are the items actually provided, and no extra items are provided"@en;
    rdfs:isDefinedBy scor: ;
    rdfs:subPropertyOf scor:hasMetric;
    vs:term_status "testing" ;
    dct:modified "2015-11-05"^^xsd:date ;
 .

scor:hasMetricRL_34 rdfs:domain [owl:unionOf (scor:ReceiveEnterValidateOrder
                                            scor:DSPConsolidateOrders
                                            scor:LoadVehicleGenerateShippingDocuments
                                            scor:DSPShipProduct
                                            scor:DSPReceiveVerifyProductByCustomer
                                            scor:ReceiveConfigureEnterValidateOrder
                                            scor:DMOPConsolidateOrders
                                            scor:DMOPLoadProductGenerateShippingDocs
                                            scor:DMOPShipProduct
                                            scor:DSPReceiveVerifyProductByCustomer
                                            scor:EnterOrderCommitResourcesLaunchProgram
                                            scor:DEOPRouteShipments
                                            scor:DEOPLoadProductGenerateShippingDocs
                                            scor:DEOPShipProduct
                                            scor:DEOPReceiveVerifyProductByCustomer)] ;
    rdfs:label "Delivery Location Accuracy"@en;
    rdfs:comment "Percentage of orders which is delivered to the correct location and customer entity"@en;
    rdfs:isDefinedBy scor: ;
    rdfs:subPropertyOf scor:hasMetric;
    vs:term_status "testing" ;
    dct:modified "2015-11-05"^^xsd:date ;
 .

scor:hasMetricRL_35 rdfs:domain [owl:unionOf (scor:ReceiveEnterValidateOrder
                                            scor:DSPConsolidateOrders
                                            scor:LoadVehicleGenerateShippingDocuments
                                            scor:DSPShipProduct
                                            scor:DSPReceiveVerifyProductByCustomer
                                            scor:ReceiveConfigureEnterValidateOrder
                                            scor:DMOPConsolidateOrders
                                            scor:DMOPLoadProductGenerateShippingDocs
                                            scor:DMOPShipProduct
                                            scor:DMOPReceiveVerifyProductByCustomer
                                            scor:EnterOrderCommitResourcesLaunchProgram
                                            scor:DEOPRouteShipments
                                            scor:DEOPLoadProductGenerateShippingDocs
                                            scor:DEOPShipProduct
                                            scor:DEOPReceiveVerifyProductByCustomer)] ;
    rdfs:label "Delivery Quantity Accuracy"@en;
    rdfs:comment "Percentage of orders in which all quantities received by the customer match the order quantities (within mutually agreed tolerances)"@en;
    rdfs:isDefinedBy scor: ;
    rdfs:subPropertyOf scor:hasMetric;
    vs:term_status "testing" ;
    dct:modified "2015-11-05"^^xsd:date ;
 .

scor:hasMetricRL_36 rdfs:domain [owl:unionOf (scor:BalanceSCResourcesWithSCRequirements
                                            scor:EstablishDeliveryPlans
                                            scor:MSProduceTest
                                            scor:DSPReserveInventoryDetermineDeliveryDate
                                            scor:PickProduct)] ;
    rdfs:label "Fill Rate"@en;
    rdfs:comment "The percentage of ship-from-stock orders shipped within 24 hours of order receipt. For services, this metric is the proportion for services that are filled so that the service is completed within 24 hours"@en;
    rdfs:isDefinedBy scor: ;
    rdfs:subPropertyOf scor:hasMetric;
    vs:term_status "testing" ;
    dct:modified "2015-11-05"^^xsd:date ;
 .

scor:hasMetricRL_37 rdfs:domain [owl:unionOf (scor:PSCIdentifyPrioritizeAggregateSCRequirements
                                            scor:IdentifyPrioritizeAggregateProductRequirements
                                            scor:IdentifyPrioritizeAggregateProductionRequirements
                                            scor:IdentifyPrioritizeAggregateDeliveryRequirements
                                            scor:IdentifyAssessAggregateDeliveryResources
                                            scor:ManageSupplyChainHumanResources
                                            scor:ManageSupplyChainAssets
                                            scor:ManageSupplyChainContracts
                                            scor:ManageSupplyChainNetworks)] ;
    rdfs:label "Forecast Accuracy"@en;
    rdfs:comment "Forecast accuracy is calculated for products and/or families for markets/distribution channels, in unit measurement. Common calculation (Sum Actuals - Sum of Variance) / Sum Actuals to determine percentage error. *monitoring the delta of Forecast Accuracy over measured time periods can determine success rates."@en;
    rdfs:isDefinedBy scor: ;
    rdfs:subPropertyOf scor:hasMetric;
    vs:term_status "testing" ;
    dct:modified "2015-11-05"^^xsd:date ;
 .

#38 seems to be deprecated

scor:hasMetricRL_39 rdfs:domain scor:DispositionExcessProduct;
    rdfs:label "Number of occurrences of incorrect designated return center"@en;
    rdfs:comment "Number of occurrences of incorrect designated return center"@en;
    rdfs:isDefinedBy scor: ;
    rdfs:subPropertyOf scor:hasMetric;
    vs:term_status "testing" ;
    dct:modified "2015-11-05"^^xsd:date ;
 .

scor:hasMetricRL_40 rdfs:domain scor:IdentifyExcessProductCondition ;
    rdfs:label "Number of occurrences where excessive inventory is returned and followed"@en;
    rdfs:comment ""@en;
    rdfs:subPropertyOf scor:hasMetric;
    rdfs:isDefinedBy scor: ;
    vs:term_status "testing" ;
    dct:modified "2015-11-05"^^xsd:date ;
 .

scor:hasMetricRL_41 rdfs:domain [owl:unionOf (scor:DSPReceiveVerifyProductByCustomer
                                            scor:DMOPReceiveVerifyProductByCustomer
                                            scor:DEOPReceiveVerifyProductByCustomer)] ;
    rdfs:label "Orders Delivered Damage Free Conformance"@en;
    rdfs:comment "Percentage of orders which is delivered without damage."@en;
    rdfs:isDefinedBy scor: ;
    rdfs:subPropertyOf scor:hasMetric;
    vs:term_status "testing" ;
    dct:modified "2015-11-05"^^xsd:date ;
 .

scor:hasMetricRL_42 rdfs:domain [owl:unionOf (scor:DSPReceiveVerifyProductByCustomer
                                            scor:DMOPReceiveVerifyProductByCustomer
                                            scor:DEOPReceiveVerifyProductByCustomer)] ;
    rdfs:label "Orders Delivered Defect Free Conformance"@en;
    rdfs:comment "Percentage of orders which is delivered without defect"@en;
    rdfs:isDefinedBy scor: ;
    rdfs:subPropertyOf scor:hasMetric;
    vs:term_status "testing" ;
    dct:modified "2015-11-05"^^xsd:date ;
 .


scor:hasMetricRL_43 rdfs:domain [owl:unionOf (scor:LoadVehicleGenerateShippingDocuments
                                            scor:DMOPLoadProductGenerateShippingDocs
                                            scor:DEOPLoadProductGenerateShippingDocs)] ;
    rdfs:label "Other Required Documentation Accuracy"@en;
    rdfs:comment "Percentage of other required documentations (besides of compliance documentation, payment documentation and shipping documentation) are complete, correct, and readily available when and how expected by customer, Government and other supply chain regulatory entities. This kind of documentations includes quality certification"@en;
    rdfs:isDefinedBy scor: ;
    rdfs:subPropertyOf scor:hasMetric;
    vs:term_status "testing" ;
    dct:modified "2015-11-05"^^xsd:date ;
 .

#44 seems to be deprecated

scor:hasMetricRL_45 rdfs:domain [owl:unionOf (scor:LoadVehicleGenerateShippingDocuments
                                            scor:DMOPLoadProductGenerateShippingDocs
                                            scor:DEOPLoadProductGenerateShippingDocs)] ;
    rdfs:label "Payment Documentation Accuracy"@en;
    rdfs:comment "Percentage of payment documentations are complete, correct, and readily available when and how expected by customer, Government and other supply chain regulatory entities. Payment documentations includes invoice, contractual outline agreement"@en;
    rdfs:isDefinedBy scor: ;
    rdfs:subPropertyOf scor:hasMetric;
    vs:term_status "testing" ;
    dct:modified "2015-11-05"^^xsd:date ;
 .



#46 seems to be deprecated

scor:hasMetricRL_47 rdfs:domain [owl:unionOf (scor:ReturnDefectiveProduct
                                            scor:ReturnMROPRoduct
                                            scor:DEOPLoadProductGenerateShippingDocs)] ;
    rdfs:label "Return Shipments on Time"@en;
    rdfs:comment "Return Shipments on Time"@en;
    rdfs:subPropertyOf scor:hasMetric;
    rdfs:isDefinedBy scor: ;
    vs:term_status "testing" ;
    dct:modified "2015-11-05"^^xsd:date ;
 .

#48 seems to be deprecated

scor:hasMetricRL_49 rdfs:domain [owl:unionOf (scor:MSScheduleProductionActivities
                                            scor:MOScheduleProductionActivities
                                            scor:MEOScheduleProductionActivities)] ;
    rdfs:label "Schedule Achievement"@en;
    rdfs:comment "The percentage of time that a plant achieves its production schedule. This calculation is based on the number of scheduled end-items or total volume for a specific period. Note: over-shipments do not make up for under-shipments."@en;
    rdfs:isDefinedBy scor: ;
    rdfs:subPropertyOf scor:hasMetric;
    vs:term_status "testing" ;
    dct:modified "2015-11-05"^^xsd:date ;
 .


scor:hasMetricRL_50 rdfs:domain [owl:unionOf (scor:LoadVehicleGenerateShippingDocuments
                                            scor:DMOPLoadProductGenerateShippingDocs
                                            scor:DEOPLoadProductGenerateShippingDocs)] ;
    rdfs:label "Shipping Documentation Accuracy"@en;
    rdfs:comment "Percentage of shipping documentations are complete, correct, and readily available when and how expected by customer, Government and other supply chain regulatory entities. Shipping documentations includes packing slips (customers), bill of lading (carriers) and government or customs documentation/forms"@en;
    rdfs:isDefinedBy scor: ;
    rdfs:subPropertyOf scor:hasMetric;
    vs:term_status "testing" ;
    dct:modified "2015-11-05"^^xsd:date ;
 .



#51-54 seem to be deprecated

scor:hasMetricRL_55 rdfs:domain [owl:unionOf (scor:MSProduceTest
                                            scor:MSPackage)] ;
    rdfs:label "Warranty and Returns"@en;
    rdfs:comment "Warranty costs include materials, labor and problem diagnosis for product defects."@en;
    rdfs:isDefinedBy scor: ;
    rdfs:subPropertyOf scor:hasMetric;
    vs:term_status "testing" ;
    dct:modified "2015-11-05"^^xsd:date ;
 .

scor:hasMetricRL_56 rdfs:domain [owl:unionOf (scor:MSProduceTest
                                            scor:MSPackage
                                            scor:MOProduceTest
                                            scor:MOPackage
                                            scor:MEOProduceTest
                                            scor:MEOPackage)] ;
    rdfs:label "Warranty Costs"@en;
    rdfs:comment "Warranty costs include materials, labor and problem diagnosis for product defects."@en;
    rdfs:isDefinedBy scor: ;
    vs:term_status "testing" ;
    rdfs:subPropertyOf scor:hasMetric;
    dct:modified "2015-11-05"^^xsd:date ;
 .

scor:hasMetricRL_57 rdfs:domain [owl:unionOf (scor:MSWasteDisposal
                                            scor:MOWasteDisposal
                                            scor:MEOWasteDisposal)] ;
    rdfs:label "Waste Processing Errors"@en;
    rdfs:comment "Number of errors in waste transactions as percent of total waste transactions"@en;
    rdfs:subPropertyOf scor:hasMetric;
    rdfs:isDefinedBy scor: ;
    vs:term_status "testing" ;
    dct:modified "2015-11-05"^^xsd:date ;
 .

scor:hasMetricRL_58 rdfs:domain [owl:unionOf (scor:MakeToStock
                                            scor:MSProduceTest
                                            scor:MSPackage
                                            scor:MakeToOrder
                                            scor:MOProduceTest
                                            scor:MOPackage
                                            scor:MakeEngineerToOrder
                                            scor:MEOProduceTest
                                            scor:MEOPackage)] ;
    rdfs:label "Yield"@en;
    rdfs:comment "The ratio of usable output from a process to its input."@en;
    rdfs:subPropertyOf scor:hasMetric;
    rdfs:isDefinedBy scor: ;
    vs:term_status "testing" ;
    dct:modified "2015-11-05"^^xsd:date ;
 .

scor:hasMetricRL_59 rdfs:domain [owl:unionOf (scor:MSProduceTest
                                            scor:MOProduceTest
                                            scor:MEOProduceTest)] ;
    rdfs:label "Yield Availability"@en;
    rdfs:comment "The condition that occurs when the output of a process is not consistently repeatable either in quantity, quality, or combination of these."@en;
    rdfs:isDefinedBy scor: ;
    rdfs:subPropertyOf scor:hasMetric;
    vs:term_status "testing" ;
    dct:modified "2015-11-05"^^xsd:date ;
 .


######### Responsiveness Metrics

######### Agility Metrics

######### Cost Metrics

######### Asset Management Efficiency Metrics


#############################################################################################
#############################################################################################
#############################################################################################
#### Individuals

## Skills

scor:3WayReceivingMatch
    rdf:type scor:Skill ;
    rdfs:comment "Knowledge of the process of reconciling invoices with purchase orders and goods received notes in order to authorize payment of invoices"@en  ;
    rdfs:label "3-way Receiving Match"@en ;
    skos:notation "HS.0001"@en  ;
    rdfs:isDefinedBy scor: ;
    vs:term_status "testing" ;
    dct:modified "2015-11-05"^^xsd:date ;
 .

scor:AcceptanceTesting
    rdf:type scor:Skill ;
    rdfs:comment "Working knowledge of Functional and/or Quality Assurance testing of product to ensure it will perform in accordance with its intended contractual agreement for form, fit and function"@en  ;
      rdfs:label "Acceptance testing"@en ;
    skos:notation "HS.0002"@en  ;
    rdfs:isDefinedBy scor: ;
    vs:term_status "testing" ;
    dct:modified "2015-11-05"^^xsd:date ;
 .

scor:Accounting
    rdf:type scor:Skill ;
    rdfs:comment "The process of collecting, analyzing, and communicating financial information about a business entity to specified stakeholders"@en  ;
    rdfs:label "Accounting"@en ;
    skos:notation "HS.0003"@en  ;
    rdfs:isDefinedBy scor: ;
    vs:term_status "testing" ;
    dct:modified "2015-11-05"^^xsd:date ;
 .

scor:AdvertisingMethodologies
    rdf:type scor:Skill ;
    rdfs:comment "Knowledge of effective procurement or business development communication techniques to inform and/or solicit potential suppliers regarding product or service specifications"@en  ;
      rdfs:label "Advertising Methodologies"@en ;
    skos:notation "HS.0004"@en  ;
    rdfs:isDefinedBy scor: ;
    vs:term_status "testing" ;
    dct:modified "2015-11-05"^^xsd:date ;
 .

scor:AssemblyProcessDesign
    rdf:type scor:Skill ;
    rdfs:comment "The arrangement of workers, machines, and equipment in which the product being assembled passes consecutively from operation to operation until completed"@en  ;
    rdfs:label "Assembly Process Design"@en ;
    skos:notation "HS.0005"@en  ;
    rdfs:isDefinedBy scor: ;
    vs:term_status "testing" ;
    dct:modified "2015-11-05"^^xsd:date ;
 .

scor:AssetManagement
    rdf:type scor:Skill ;
    rdfs:comment "The process (which requires the use of spreadsheets or software) to identify, collect, maintain and track the companies assets"@en  ;
    rdfs:label "Asset Management"@en ;
    skos:notation "HS.0006"@en  ;
    rdfs:isDefinedBy scor: ;
    vs:term_status "testing" ;
    dct:modified "2015-11-05"^^xsd:date ;
 .

scor:AvailabilityManagement
    rdf:type scor:Skill ;
    rdfs:comment "The process of managing and allocating available resources and inventory (at various levels) based on business rules"@en  ;
    rdfs:label "Availability Management"@en ;
    skos:notation "HS.0007"@en  ;
    rdfs:isDefinedBy scor: ;
    vs:term_status "testing" ;
    dct:modified "2015-11-05"^^xsd:date ;
 .

scor:BarCodeHandlingRFID
    rdf:type scor:Skill ;
    rdfs:comment "Basic working knowledge of the concept of applying or incorporating onto/into a product an optical machine-readable representation of data (bar code) and /or using radio waves with radio-frequency identification tags (RFID) for the purpose of the identification and tracking of that product"@en  ;
    rdfs:label "Bar Code Handling/RFID"@en ;
    skos:notation "HS.0009"@en  ;
    rdfs:isDefinedBy scor: ;
    vs:term_status "testing" ;
    dct:modified "2015-11-05"^^xsd:date ;
 .

scor:BasicFinance
    rdf:type scor:Skill ;
    rdfs:comment "Working knowledge and ability to effectively interpret and communicate general financial accounting practices and principles which maintain company and regulatory compliance"@en  ;
    rdfs:label "Basic Finance"@en ;
    skos:notation "HS.0010"@en  ;
    rdfs:isDefinedBy scor: ;
    vs:term_status "testing" ;
    dct:modified "2015-11-05"^^xsd:date ;
 .

scor:BasicTransportationManagement
    rdf:type scor:Skill ;
    rdfs:comment "The management of transportation operations of all types, including tracking and managing every aspect of vehicle maintenance"@en  ;
    rdfs:label "Basic Transportation Management"@en ;
    skos:notation "HS.0011"@en  ;
    rdfs:isDefinedBy scor: ;
    vs:term_status "testing" ;
    dct:modified "2015-11-05"^^xsd:date ;
 .

scor:Benchmarking
    rdf:type scor:Skill ;
    rdfs:comment "Working knowledge of the process of capturing and comparing one's own business processes and performance metrics to industry peers and/or best practices from other industries"@en  ;
    rdfs:label "Benchmarking"@en ;
    skos:notation "HS.0012"@en  ;
    rdfs:isDefinedBy scor: ;
    vs:term_status "testing" ;
    dct:modified "2015-11-05"^^xsd:date ;
 .

scor:BlanketPurchaseOrderProcess
    rdf:type scor:Skill ;
    rdfs:comment "Working knowledge of the procurement process for soliciting, issuing and administering open-ended (period for performance) type purchase orders or contracts"@en  ;
    rdfs:label "Blanket purchase order process"@en ;
    skos:notation "HS.0013"@en  ;
    rdfs:isDefinedBy scor: ;
    vs:term_status "testing" ;
    dct:modified "2015-11-05"^^xsd:date ;
 .

scor:BuildScheduleEvaluation
    rdf:type scor:Skill ;
    rdfs:comment "Analyzing a product installation schedule against the constraints and requirements in order to ensure feasibility to effectively and efficiently complete the installation process"@en  ;
    rdfs:label "Build Schedule Evaluation"@en ;
    skos:notation "HS.0014"@en  ;
    rdfs:isDefinedBy scor: ;
    vs:term_status "testing" ;
    dct:modified "2015-11-05"^^xsd:date ;
 .

scor:CADCAM
    rdf:type scor:Skill ;
    rdfs:comment "The process to use computer technology to aid in the design, analysis, and manufacture of products"@en  ;
    rdfs:label "CAD/CAM"@en ;
    skos:notation "HS.0015"@en  ;
    rdfs:isDefinedBy scor: ;
    vs:term_status "testing" ;
    dct:modified "2015-11-05"^^xsd:date ;
 .

scor:CapacityPlanningManagement
    rdf:type scor:Skill ;
    rdfs:comment "The process of determining and managing the production capacity needed by an organization to meet changing demands for its products"@en  ;
    rdfs:label "Capacity Planning/Management"@en ;
    skos:notation "HS.0016"@en  ;
    rdfs:isDefinedBy scor: ;
    vs:term_status "testing" ;
    dct:modified "2015-11-05"^^xsd:date ;
 .

scor:CarrierSelection
    rdf:type scor:Skill ;
    rdfs:comment "Selection of a transportation mode and service provider in order to meet due dates, cost and service objectives"@en  ;
    rdfs:label "Carrier Selection"@en ;
    skos:notation "HS.0018"@en  ;
    rdfs:isDefinedBy scor: ;
    vs:term_status "testing" ;
    dct:modified "2015-11-05"^^xsd:date ;
 .

scor:ChangeNoticeDevelopment
    rdf:type scor:Skill ;
    rdfs:comment "Working knowledge of the procurement process and the ability to clearly disseminate specific contractual or technical requirements which have changed to Sourced contractors, suppliers or vendors"@en  ;
    rdfs:label "Change Notice Development"@en ;
    skos:notation "HS.0019"@en  ;
    rdfs:isDefinedBy scor: ;
    vs:term_status "testing" ;
    dct:modified "2015-11-05"^^xsd:date ;
 .

scor:CompetitiveBidding
    rdf:type scor:Skill ;
    rdfs:comment "Working knowledge of procurement process for requesting and receiving bids/quotes from competing contractors, suppliers, or vendors based on product part numbers, scope, specifications, terms and conditions"@en  ;
    rdfs:label "Competitive Bidding"@en ;
    skos:notation "HS.0020"@en  ;
    rdfs:isDefinedBy scor: ;
    vs:term_status "testing" ;
    dct:modified "2015-11-05"^^xsd:date ;
 .

scor:ConsignmentAgreementDevelopment
    rdf:type scor:Skill ;
    rdfs:comment "Working knowledge of Consignment Agreements which are when one party provides goods/services to another party for sale by that other party"@en  ;
    rdfs:label "Consignment Agreement Development"@en ;
    skos:notation "HS.0021"@en  ;
    rdfs:isDefinedBy scor: ;
    vs:term_status "testing" ;
    dct:modified "2015-11-05"^^xsd:date ;
 .

scor:ContractManagement
    rdf:type scor:Skill ;
    rdfs:comment "Experience in solicitation process, bid/proposal evaluation, contract award and post award administration, and closeout"@en  ;
    rdfs:label "Contract Management"@en ;
    skos:notation "HS.0022"@en  ;
    rdfs:isDefinedBy scor: ;
    vs:term_status "testing" ;
    dct:modified "2015-11-05"^^xsd:date ;
 .

scor:ControlsCompliance
    rdf:type scor:Skill ;
    rdfs:comment "Awareness of relevant regulations, laws and requirements, whether external or internal, and the ability to devise, implement and document the relevant and necessary controls in order to maintain compliance and successfully pass auditing requirements"@en  ;
    rdfs:label "Controls and Compliance"@en ;
    skos:notation "HS.0023"@en  ;
    rdfs:isDefinedBy scor: ;
    vs:term_status "testing" ;
    dct:modified "2015-11-05"^^xsd:date ;
 .

scor:CostPriceAnalysis
    rdf:type scor:Skill ;
    rdfs:comment "Basic financial understanding of analyzing the costs/prices associated with a bid/proposal/quotation for a sourced product for the purpose of attaining best cost/price and/or best value for that product"@en  ;
    rdfs:label "Cost/Price Analysis"@en ;
    skos:notation "HS.0024"@en  ;
    rdfs:isDefinedBy scor: ;
    vs:term_status "testing" ;
    dct:modified "2015-11-05"^^xsd:date ;
 .

scor:BusinessPolicyManagement
    rdf:type scor:Skill ;
    rdfs:comment "A documented set of basic principles and associated guidelines, formulated and enforced by the governing body or an assigned committee of an organization that direct and limit a company's decisions and actions in pursuit of its objectives"@en  ;
    rdfs:label "Business Rule/Policy Management"@en ;
    skos:notation "HS.0025"@en  ;
    rdfs:isDefinedBy scor: ;
    vs:term_status "testing" ;
    dct:modified "2015-11-05"^^xsd:date ;
 .

scor:CreditCollectionManagement
    rdf:type scor:Skill ;
    rdfs:comment "Set of activities to assess and rate the credit risk of a customer, identify/block non-creditworthy customers, manage outstanding balances, process credits, and investigate/pursue overdues"@en  ;
    rdfs:label "Credit/Collection Management"@en ;
    skos:notation "HS.0026"@en  ;
    rdfs:isDefinedBy scor: ;
    vs:term_status "testing" ;
    dct:modified "2015-11-05"^^xsd:date ;
 .

scor:HSCrossDocking
    rdf:type scor:Skill ;
    rdfs:comment "Basic knowledge of linking, staging and moving received sourced products with/to existing open orders minimizing the need for product inventory or storage"@en  ;
    rdfs:label "Cross Docking"@en ;
    skos:notation "HS.0027"@en  ;
    rdfs:isDefinedBy scor: ;
    vs:term_status "testing" ;
    dct:modified "2015-11-05"^^xsd:date ;
 .

scor:CustomerOrderManagement
    rdf:type scor:Skill ;
    rdfs:comment "The process or the work flow associated with the identification, receipt, acceptance, picking, packing, delivery and of the packed item(s) to a shipping carrier"@en  ;
    rdfs:label "Customer Order Management"@en ;
    skos:notation "HS.0028"@en  ;
    rdfs:isDefinedBy scor: ;
    vs:term_status "testing" ;
    dct:modified "2015-11-05"^^xsd:date ;
 .

scor:CustomerRelationshipManagement
    rdf:type scor:Skill ;
    rdfs:comment "Managing a company's relations and interactions with clients and sales prospects, possibly including the synchronization of business processes with the objective of identifying, attracting, and managing new and existing customers"@en  ;
    rdfs:label "Customer Relationship Management (CRM)"@en ;
    skos:notation "HS.0029"@en  ;
    rdfs:isDefinedBy scor: ;
    vs:term_status "testing" ;
    dct:modified "2015-11-05"^^xsd:date ;
 .

scor:CustomerRepair
    rdf:type scor:Skill ;
    rdfs:comment "The actions, tasks and responsibilities concerned with the decision to repair all mechanical/electrical out of order/broken products in line with the internal return rules"@en  ;
    rdfs:label "Customer Repair and Return Policy and Process"@en ;
    skos:notation "HS.0031"@en  ;
    rdfs:isDefinedBy scor: ;
    vs:term_status "testing" ;
    dct:modified "2015-11-05"^^xsd:date ;
 .

scor:CustomerSupplierCommunication
    rdf:type scor:Skill ;
    rdfs:comment "Process of transferring customer/supplier information by speech or writing"@en  ;
    rdfs:label "Customer/Supplier Communication"@en ;
    skos:notation "HS.0032"@en  ;
    rdfs:isDefinedBy scor: ;
    vs:term_status "testing" ;
    dct:modified "2015-11-05"^^xsd:date ;
 .

scor:DataManagement
    rdf:type scor:Skill ;
    rdfs:comment "Working knowledge of the processes required to develop, execute and sustain plans, policies, programs and practices that control, protect, deliver and enhance the value of data and information systems/assets"@en  ;
    rdfs:label "Data management"@en ;
    skos:notation "HS.0033"@en  ;
    rdfs:isDefinedBy scor: ;
    vs:term_status "testing" ;
    dct:modified "2015-11-05"^^xsd:date ;
 .

scor:DiscrepancyReportingResolution
    rdf:type scor:Skill ;
    rdfs:comment "Knowledge of techniques, systems, tools and human skills required to establish effective procedures to identify defective and missing product and then report onward, either internally or externally, ensuring closure on reports and improvements to avoid future repetition"@en  ;
    rdfs:label "Discrepancy Reporting and Resolution"@en ;
    skos:notation "HS.0034"@en  ;
    rdfs:isDefinedBy scor: ;
    vs:term_status "testing" ;
    dct:modified "2015-11-05"^^xsd:date ;
 .

scor:DeliveryBalancing
    rdf:type scor:Skill ;
    rdfs:comment "Delivery balancing is one part of Master Scheduling and involves the balancing of deliveries from suppliers against constrained criteria"@en  ;
    rdfs:label "Delivery Balancing"@en ;
    skos:notation "HS.0035"@en  ;
    rdfs:isDefinedBy scor: ;
    vs:term_status "testing" ;
    dct:modified "2015-11-05"^^xsd:date ;
 .

scor:DeliveryScheduling
    rdf:type scor:Skill ;
    rdfs:comment "Basic knowledge of scheduling and managing sourced product deliveries in order to meet the requirements of inventory replenishment or scheduled production plans"@en  ;
    rdfs:label "Delivery Scheduling"@en ;
    skos:notation "HS.0036"@en  ;
    rdfs:isDefinedBy scor: ;
    vs:term_status "testing" ;
    dct:modified "2015-11-05"^^xsd:date ;
 .

scor:HSDemandManagement
    rdf:type scor:Skill ;
    rdfs:comment "The manufacturing management process by which raw materials and production capacity are optimally allocated to meet demand"@en  ;
    rdfs:label "Demand Management (Skill)"@en ;
    skos:notation "HS.0037"@en  ;
    rdfs:isDefinedBy scor: ;
    vs:term_status "testing" ;
    dct:modified "2015-11-05"^^xsd:date ;
 .

scor:DesignEngineeringScheduleDevelopment
    rdf:type scor:Skill ;
    rdfs:comment "Analyzing the constraints and requirements of a product design cycle in order to evaluate and ensure the timely availability of the product design for building and installation of a product"@en  ;
    rdfs:label "Design/Engineering Schedule Development"@en ;
    skos:notation "HS.0038"@en  ;
    rdfs:isDefinedBy scor: ;
    vs:term_status "testing" ;
    dct:modified "2015-11-05"^^xsd:date ;
 .

scor:DrivingCertification
    rdf:type scor:Skill ;
    rdfs:comment "Ownership of the official, valid (not expired) document stating that the person is authorized and able to drive (a) class/es of vehicles"@en  ;
    rdfs:label "Driving Certification"@en ;
    skos:notation "HS.0039"@en  ;
    rdfs:isDefinedBy scor: ;
    vs:term_status "testing" ;
    dct:modified "2015-11-05"^^xsd:date ;
 .

scor:EHSregulations
    rdf:type scor:Skill ;
    rdfs:comment "The actions, tasks, and responsibilities concerned with the observance and application of the environment, health, and safety rules and standards"@en  ;
    rdfs:label "EHS regulations"@en ;
    skos:notation "HS.0041"@en  ;
    rdfs:isDefinedBy scor: ;
    vs:term_status "testing" ;
    dct:modified "2015-11-05"^^xsd:date ;
 .

scor:EnablingTechnology
    rdf:type scor:Skill ;
    rdfs:comment "Working awareness of relevant technology that could/can be used to improve the effectiveness or efficiency of operations within Source, but also widely across the Supply Chain or the enterprise"@en  ;
    rdfs:label "Enabling Technology"@en ;
    skos:notation "HS.0042"@en  ;
    rdfs:isDefinedBy scor: ;
    vs:term_status "testing" ;
    dct:modified "2015-11-05"^^xsd:date ;
 .

scor:Engineering
    rdf:type scor:Skill ;
    rdfs:comment "The discipline, art and profession of acquiring and applying technical, scientific, and mathematical knowledge to design and implement materials, structures, machines, devices, systems, and processes that safely realize a desired objective or invention"@en  ;
    rdfs:label "Engineering"@en ;
    skos:notation "HS.0043"@en  ;
    rdfs:isDefinedBy scor: ;
    vs:term_status "testing" ;
    dct:modified "2015-11-05"^^xsd:date ;
 .

scor:EnterpriseBusinessProcess
    rdf:type scor:Skill ;
    rdfs:comment "The end-to-end (cross-departmental, and often, cross-company) coordination of work activities that create and deliver ultimate value to customers"@en  ;
    rdfs:label "Enterprise Business Process"@en ;
    skos:notation "HS.0044"@en  ;
    rdfs:isDefinedBy scor: ;
    vs:term_status "testing" ;
    dct:modified "2015-11-05"^^xsd:date ;
 .

scor:EnvironmentalRequirements
    rdf:type scor:Skill ;
    rdfs:comment "Familiarity and understanding of internal and external goals, objectives, rules and laws pertaining to the operation of the Source function within the organization"@en  ;
    rdfs:label "Environmental Requirements"@en ;
    skos:notation "HS.0045"@en  ;
    rdfs:isDefinedBy scor: ;
    vs:term_status "testing" ;
    dct:modified "2015-11-05"^^xsd:date ;
 .

scor:ERPSystems
    rdf:type scor:Skill ;
    rdfs:comment "Working awareness of and conversant with installing and operating appropriate Enterprise Resource Planning (ERP) systems relevant to the organisation concerned"@en  ;
    rdfs:label "ERP Systems"@en ;
    skos:notation "HS.0046"@en  ;
    rdfs:isDefinedBy scor: ;
    vs:term_status "testing" ;
    dct:modified "2015-11-05"^^xsd:date ;
 .

scor:Forecasting
    rdf:type scor:Skill ;
    rdfs:comment "The process of predicting production requirements to meet estimated sales in a particular forecasting period"@en  ;
    rdfs:label "Forecasting"@en ;
    skos:notation "HS.0048"@en  ;
    rdfs:isDefinedBy scor: ;
    vs:term_status "testing" ;
    dct:modified "2015-11-05"^^xsd:date ;
 .

scor:IDDamageInspection
    rdf:type scor:Skill ;
    rdfs:comment "Working knowledge and ability to identify and inspect Sourced products for compliance with contractual part numbers, specifications, drawings, etc, including quality requirements and damage-free product receipt"@en  ;
    rdfs:label "ID and Damage Inspection"@en ;
    skos:notation "HS.0049"@en  ;
    rdfs:isDefinedBy scor: ;
    vs:term_status "testing" ;
    dct:modified "2015-11-05"^^xsd:date ;
 .

scor:ImportExportRegulations
    rdf:type scor:Skill ;
    rdfs:comment "The knowledge and understanding of the laws and regulations governing the import and export requirements of materials"@en  ;
    rdfs:label "Import/Export Regulations"@en ;
    skos:notation "HS.0050"@en  ;
    rdfs:isDefinedBy scor: ;
    vs:term_status "testing" ;
    dct:modified "2015-11-05"^^xsd:date ;
 .

scor:InstallationRequirements
    rdf:type scor:Skill ;
    rdfs:comment "The information, resources and skills requirements to effectively install purchased products as per customer requirements"@en  ;
    rdfs:label "Installation Requirements"@en ;
    skos:notation "HS.0051"@en  ;
    rdfs:isDefinedBy scor: ;
    vs:term_status "testing" ;
    dct:modified "2015-11-05"^^xsd:date ;
 .

scor:InstallationScheduling
    rdf:type scor:Skill ;
    rdfs:comment "The process of managing requirement and constraints associated with a installation schedule in order to effectively schedule product installation as per customer requirements"@en  ;
    rdfs:label "Installation Scheduling"@en ;
    skos:notation "HS.0052"@en  ;
    rdfs:isDefinedBy scor: ;
    vs:term_status "testing" ;
    dct:modified "2015-11-05"^^xsd:date ;
 .

scor:InstalledBaseManagement
    rdf:type scor:Skill ;
    rdfs:comment "Actions, tasks and responsibilities concerned with maintenance and update of info related to the number of units of the company products/platform actually installed and in use around the world"@en  ;
    rdfs:label "Installed base management"@en ;
    skos:notation "HS.0053"@en  ;
    rdfs:isDefinedBy scor: ;
    vs:term_status "testing" ;
    dct:modified "2015-11-05"^^xsd:date ;
 .

scor:IntellectualProperty
    rdf:type scor:Skill ;
    rdfs:comment "Conversant with and effectively manage Proprietary Data and Intellectual property on behalf of the organization"@en  ;
    rdfs:label "Intellectual Property/Proprietary Data"@en ;
    skos:notation "HS.0054"@en  ;
    rdfs:isDefinedBy scor: ;
    vs:term_status "testing" ;
    dct:modified "2015-11-05"^^xsd:date ;
 .

scor:InternationalTrade
    rdf:type scor:Skill ;
    rdfs:comment "The exchange of capital, goods, and services across international borders or territories"@en  ;
    rdfs:label "International Trade"@en ;
    skos:notation "HS.0055"@en  ;
    rdfs:isDefinedBy scor: ;
    vs:term_status "testing" ;
    dct:modified "2015-11-05"^^xsd:date ;
 .

scor:InterpretingSpecifications
    rdf:type scor:Skill ;
    rdfs:comment "Basic working knowledge and ability to read, interpret, understand, and effectively communicate technical specifications and/or drawings to support timely design and delivery of products meeting minimum requirements"@en  ;
    rdfs:label "Interpreting Specifications"@en ;
    skos:notation "HS.0056"@en  ;
    rdfs:isDefinedBy scor: ;
    vs:term_status "testing" ;
    dct:modified "2015-11-05"^^xsd:date ;
 .

scor:InventoryManagement
    rdf:type scor:Skill ;
    rdfs:comment "The formal management of the timing and quantities of goods to be ordered and stocked by an organization in order that demand can always be satisfied without excess expenditure"@en  ;
    rdfs:label "Inventory Management"@en ;
    skos:notation "HS.0058"@en  ;
    rdfs:isDefinedBy scor: ;
    vs:term_status "testing" ;
    dct:modified "2015-11-05"^^xsd:date ;
 .

scor:IssueProposalQuote
    rdf:type scor:Skill ;
    rdfs:comment "The compilation of all required specifications and details need to generate and communicate an RFP/Q"@en  ;
    rdfs:label "Issue Proposal/Quote"@en ;
    skos:notation "HS.0060"@en  ;
    rdfs:isDefinedBy scor: ;
    vs:term_status "testing" ;
    dct:modified "2015-11-05"^^xsd:date ;
 .

scor:ItemMaster
    rdf:type scor:Skill ;
    rdfs:comment "The ability to understand, interpret and effectively communicate a part master record (item master) or bill of materials (BOM) of parts lists that details description, unit of measure, dimensions, group/ family classification, production or sourcing data, quality requirements and/or restrictions"@en  ;
    rdfs:label "Item Master/BOM/BoL Interpretation"@en ;
    skos:notation "HS.0061"@en  ;
    rdfs:isDefinedBy scor: ;
    vs:term_status "testing" ;
    dct:modified "2015-11-05"^^xsd:date ;
 .

scor:KittingPacking
    rdf:type scor:Skill ;
    rdfs:comment "The process of aggregating and packing all elements belonging to a customer order"@en  ;
    rdfs:label "Kitting/Packing"@en ;
    skos:notation "HS.0062"@en  ;
    rdfs:isDefinedBy scor: ;
    vs:term_status "testing" ;
    dct:modified "2015-11-05"^^xsd:date ;
 .

scor:LaborCostsVerification
    rdf:type scor:Skill ;
    rdfs:comment "Capability of calculating, understanding, reporting on, and if necessary, be able to taking corrective action to control labour costs within one's area of responsibility against budgets or objectives that have been set"@en  ;
    rdfs:label "Labor Costs Verification"@en ;
    skos:notation "HS.0063"@en  ;
    rdfs:isDefinedBy scor: ;
    vs:term_status "testing" ;
    dct:modified "2015-11-05"^^xsd:date ;
 .

scor:LeadTimeValidation
    rdf:type scor:Skill ;
    rdfs:comment "The process of analyzing and validating feasibility of customer required lead-times"@en  ;
    rdfs:label "Lead-time validation"@en ;
    skos:notation "HS.0064"@en  ;
    rdfs:isDefinedBy scor: ;
    vs:term_status "testing" ;
    dct:modified "2015-11-05"^^xsd:date ;
 .

scor:LeanManufacturing
    rdf:type scor:Skill ;
    rdfs:comment "The process of identifying processes that impede the optimization of production"@en  ;
    rdfs:label "Lean Manufacturing"@en ;
    skos:notation "HS.0065"@en  ;
    rdfs:isDefinedBy scor: ;
    vs:term_status "testing" ;
    dct:modified "2015-11-05"^^xsd:date ;
 .

scor:LegislationStandards
    rdf:type scor:Skill ;
    rdfs:comment "Knowledge to manage conformance systems and actions for receiving product and relates to general legislation affecting the product being received as well as the specific standards or specifications that applies to the product"@en  ;
    rdfs:label "Legislation and Standards"@en ;
    skos:notation "HS.0066"@en  ;
    rdfs:isDefinedBy scor: ;
    vs:term_status "testing" ;
    dct:modified "2015-11-05"^^xsd:date ;
 .

scor:LinearProgramming
    rdf:type scor:Skill ;
    rdfs:comment "The branch of mathematics concerned with the minimization or maximization of a linear function of several variables and inequalities; used in many branches of industry to minimize costs or maximize production"@en  ;
    rdfs:label "Linear programming"@en ;
    skos:notation "HS.0067"@en  ;
    rdfs:isDefinedBy scor: ;
    vs:term_status "testing" ;
    dct:modified "2015-11-05"^^xsd:date ;
 .

scor:LoadBuilding
    rdf:type scor:Skill ;
    rdfs:comment "The process of order consolidation to meet service, cost, delivery and product specification requirements"@en  ;
    rdfs:label "Load Building"@en ;
    skos:notation "HS.0068"@en  ;
    rdfs:isDefinedBy scor: ;
    vs:term_status "testing" ;
    dct:modified "2015-11-05"^^xsd:date ;
 .

scor:LogisticsManagement
    rdf:type scor:Skill ;
    rdfs:comment "The process for planning, implementing, and controlling the flow and storage of goods, services, and related information between the point of origin and the point of consumption in order to meet customers’ requirements and thus add value for the customer"@en  ;
    rdfs:label "Logistics Management"@en ;
    skos:notation "HS.0069"@en  ;
    rdfs:isDefinedBy scor: ;
    vs:term_status "testing" ;
    dct:modified "2015-11-05"^^xsd:date ;
 .

scor:LogisticsNetworkModeling
    rdf:type scor:Skill ;
    rdfs:comment "The process of planning, implementing, and controlling the flow and storage of goods, services, and related information between the point of origin and the point of consumption in order to meet customers' requirements"@en  ;
    rdfs:label "Logistics network modeling"@en ;
    skos:notation "HS.0070"@en  ;
    rdfs:isDefinedBy scor: ;
    vs:term_status "testing" ;
    dct:modified "2015-11-05"^^xsd:date ;
 .

scor:LogisticsFreight
    rdf:type scor:Skill ;
    rdfs:comment "Working knowledge of the management and integration of information, sourced product/material, transportation, inventory, warehousing, material-handling, and packaging, and occasionally security, between the point of origin and the point of consumption in order to meet customer requirements"@en  ;
    rdfs:label "Logistics/Freight"@en ;
    skos:notation "HS.0071"@en  ;
    rdfs:isDefinedBy scor: ;
    vs:term_status "testing" ;
    dct:modified "2015-11-05"^^xsd:date ;
 .

scor:PerformanceManagement
    rdf:type scor:Skill ;
    rdfs:comment "A framework that identifies opportunities for performance improvement through use of performance measures such as standards and indicators"@en  ;
    rdfs:label "Performance Management"@en ;
    skos:notation "HS.0072"@en  ;
    rdfs:isDefinedBy scor: ;
    vs:term_status "testing" ;
    dct:modified "2015-11-05"^^xsd:date ;
 .

scor:ManufacturingResourceCommitment
    rdf:type scor:Skill ;
    rdfs:comment "The efficient and effective allocation of an organization's manufacturing resources and assets with the objective of meeting customer demands/requirements"@en  ;
    rdfs:label "Manufacturing Resource Commitment"@en ;
    skos:notation "HS.0073"@en  ;
    rdfs:isDefinedBy scor: ;
    vs:term_status "testing" ;
    dct:modified "2015-11-05"^^xsd:date ;
 .

scor:MasterScheduling
    rdf:type scor:Skill ;
    rdfs:comment "Knowledge of co-ordinating and keeping track of all the different components related to the Source activity"@en  ;
    rdfs:label "Master Scheduling"@en ;
    skos:notation "HS.0074"@en  ;
    rdfs:isDefinedBy scor: ;
    vs:term_status "testing" ;
    dct:modified "2015-11-05"^^xsd:date ;
 .

scor:MaterialHandlingEquipment
    rdf:type scor:Skill ;
    rdfs:comment "The ability to manipulate various types of material handling systems (e.g. forklifts, conveyors, palletizers, etc.) to pick, pack, and store orders and inventory"@en  ;
    rdfs:label "Material handling equipment usage"@en ;
    skos:notation "HS.0075"@en  ;
    rdfs:isDefinedBy scor: ;
    vs:term_status "testing" ;
    dct:modified "2015-11-05"^^xsd:date ;
 .

scor:MilestonePerformancePayments
    rdf:type scor:Skill ;
    rdfs:comment "Working knowledge of contractual requirements for the authorization of monetary payments for the successful completion of pre-defined development or performance milestones"@en  ;
    rdfs:label "Milestone/Performance Payments"@en ;
    skos:notation "HS.0076"@en  ;
    rdfs:isDefinedBy scor: ;
    vs:term_status "testing" ;
    dct:modified "2015-11-05"^^xsd:date ;
 .

scor:MPSMethodsTechniques
    rdf:type scor:Skill ;
    rdfs:comment "The techniques used in material requirements planning systems to develop a detailed plan for product manufacturing"@en  ;
    rdfs:label "MPS Methodologies and Techniques"@en ;
    skos:notation "HS.0077"@en  ;
    rdfs:isDefinedBy scor: ;
    vs:term_status "testing" ;
    dct:modified "2015-11-05"^^xsd:date ;
 .

scor:MROManagement
    rdf:type scor:Skill ;
    rdfs:comment "All actions which have the objective of retaining or restoring an item in or to a state in which it can perform its required function"@en  ;
    rdfs:label "MRO Management"@en ;
    skos:notation "HS.0078"@en  ;
    rdfs:isDefinedBy scor: ;
    vs:term_status "testing" ;
    dct:modified "2015-11-05"^^xsd:date ;
 .

scor:MRPSystems
    rdf:type scor:Skill ;
    rdfs:comment "The process of ensuring materials and products are available for production and delivery to customers, maintaining the lowest possible level of inventory and planning manufacturing activities, delivery schedules and purchasing activities"@en  ;
    rdfs:label "MRP Systems"@en ;
    skos:notation "HS.0079"@en  ;
    rdfs:isDefinedBy scor: ;
    vs:term_status "testing" ;
    dct:modified "2015-11-05"^^xsd:date ;
 .

scor:EnvironmentalInterpretation
    rdf:type scor:Skill ;
    rdfs:comment "Working knowledge and understanding of strict regulatory adherence to health and environmental requirements/restrictions associated with particular products as detailed on Material Safely Data Sheets (MSDS) or Certificates of Compliance CoC"@en  ;
    rdfs:label "Environmental Interpretation"@en ;
    skos:notation "HS.0080"@en  ;
    rdfs:isDefinedBy scor: ;
    vs:term_status "testing" ;
    dct:modified "2015-11-05"^^xsd:date ;
 .

scor:OfficeAutomationTools
    rdf:type scor:Skill ;
    rdfs:comment "Familiarity with relevant Office Automation Tools and be able to deploy against financial justification as appropriate taking account of project and change management requirements"@en  ;
    rdfs:label "Office automation tools"@en ;
    skos:notation "HS.0081"@en  ;
    rdfs:isDefinedBy scor: ;
    vs:term_status "testing" ;
    dct:modified "2015-11-05"^^xsd:date ;
 .

scor:Optimization
    rdf:type scor:Skill ;
    rdfs:comment "The process of improving various aspects of the business resulting in (such as) increased profits, improved product or greater customer satisfaction"@en  ;
    rdfs:label "Optimization"@en ;
    skos:notation "HS.0082"@en  ;
    rdfs:isDefinedBy scor: ;
    vs:term_status "testing" ;
    dct:modified "2015-11-05"^^xsd:date ;
 .

scor:OrderManagement
    rdf:type scor:Skill ;
    rdfs:comment "The process or the work flow associated with the identification, receipt, acceptance, picking, packing, delivery and of the packed item(s) to a shipping carrier"@en  ;
    rdfs:label "Order Management"@en ;
    skos:notation "HS.0083"@en  ;
    rdfs:isDefinedBy scor: ;
    vs:term_status "testing" ;
    dct:modified "2015-11-05"^^xsd:date ;
 .

scor:Outsourcing
    rdf:type scor:Skill ;
    rdfs:comment "A company that contracts with another company to provide services that might otherwise be performed by in-house employees"@en  ;
    rdfs:label "Outsourcing"@en ;
    skos:notation "HS.0085"@en  ;
    rdfs:isDefinedBy scor: ;
    vs:term_status "testing" ;
    dct:modified "2015-11-05"^^xsd:date ;
 .

scor:Packaging
    rdf:type scor:Skill ;
    rdfs:comment "The processes of coordinating a system of preparing goods for transport, warehousing, logistics, sale, and end use"@en  ;
    rdfs:label "Packaging"@en ;
    skos:notation "HS.0086"@en  ;
    rdfs:isDefinedBy scor: ;
    vs:term_status "testing" ;
    dct:modified "2015-11-05"^^xsd:date ;
 .

scor:PaymentProcessing
    rdf:type scor:Skill ;
    rdfs:comment "Working knowledge of the processes and policies required for contractual authorization of payments for sourced products and services"@en  ;
    rdfs:label "Payment Processing"@en ;
    skos:notation "HS.0087"@en  ;
    rdfs:isDefinedBy scor: ;
    vs:term_status "testing" ;
    dct:modified "2015-11-05"^^xsd:date ;
 .

scor:PhysicalCapability
    rdf:type scor:Skill ;
    rdfs:comment "The ability to complete a process through the use of dexterity, strength or other capacities"@en  ;
    rdfs:label "Physical Capability"@en ;
    skos:notation "HS.0088"@en  ;
    rdfs:isDefinedBy scor: ;
    vs:term_status "testing" ;
    dct:modified "2015-11-05"^^xsd:date ;
 .

scor:PhysicalDistributionSystems
    rdf:type scor:Skill ;
    rdfs:comment "The set of activities concerned with efficient movement of finished goods from the end of the production operation to the consumer"@en  ;
    rdfs:label "Physical Distribution Systems"@en ;
    skos:notation "HS.0089"@en  ;
    rdfs:isDefinedBy scor: ;
    vs:term_status "testing" ;
    dct:modified "2015-11-05"^^xsd:date ;
 .

scor:PickingProcess
    rdf:type scor:Skill ;
    rdfs:comment "The process of selecting and collecting SKUs and materials in a specified order and quantity with the objective of satisfying customers orders"@en  ;
    rdfs:label "Picking process / order batching"@en ;
    skos:notation "HS.0090"@en  ;
    rdfs:isDefinedBy scor: ;
    vs:term_status "testing" ;
    dct:modified "2015-11-05"^^xsd:date ;
 .

scor:PlanogramUsageStrategies
    rdf:type scor:Skill ;
    rdfs:comment "The process of using a planogram to diagram fixtures and products to illustrate how and where retail products should be displayed, usually on a store shelf in order to increase customer purchases"@en  ;
    rdfs:label "Planogram usage and strategies"@en ;
    skos:notation "HS.0091"@en  ;
    rdfs:isDefinedBy scor: ;
    vs:term_status "testing" ;
    dct:modified "2015-11-05"^^xsd:date ;
 .

scor:PricingManagement
    rdf:type scor:Skill ;
    rdfs:comment "The analysis and setting of prices (on a per unit or volume basis) to meet required characteristics, business rules and/or business performance requirements"@en  ;
    rdfs:label "Pricing Management"@en ;
    skos:notation "HS.0092"@en  ;
    rdfs:isDefinedBy scor: ;
    vs:term_status "testing" ;
    dct:modified "2015-11-05"^^xsd:date ;
 .

scor:Prioritization
    rdf:type scor:Skill ;
    rdfs:comment "The knowledge and ability to arrange process steps, jobs or orders in queue, or product receipts in the proper sequence in order to meet product/service production and deliveries as scheduled"@en  ;
    rdfs:label "Prioritization"@en ;
    skos:notation "HS.0093"@en  ;
    rdfs:isDefinedBy scor: ;
    vs:term_status "testing" ;
    dct:modified "2015-11-05"^^xsd:date ;
 .

scor:Procurement
    rdf:type scor:Skill ;
    rdfs:comment "Working knowledge of the process for acquiring goods and/or services at the best possible total cost of ownership, in the right quantity, quality, at the right time and in the right place, with all required documentation"@en  ;
    rdfs:label "Procurement"@en ;
    skos:notation "HS.0094"@en  ;
    rdfs:isDefinedBy scor: ;
    vs:term_status "testing" ;
    dct:modified "2015-11-05"^^xsd:date ;
 .

scor:ProductConfigurationValidation
    rdf:type scor:Skill ;
    rdfs:comment "The analysis of stated product and configuration specifications against required and feasible product's performance, functional, and physical requirements"@en  ;
    rdfs:label "Product and Configuration Validation"@en ;
    skos:notation "HS.0095"@en  ;
    rdfs:isDefinedBy scor: ;
    vs:term_status "testing" ;
    dct:modified "2015-11-05"^^xsd:date ;
 .

scor:ProductCheckoutProcess
    rdf:type scor:Skill ;
    rdfs:comment "The process of removing a product from inventory and exchanging funds for the value of the product in a retail supply chain"@en  ;
    rdfs:label "Product checkout process"@en ;
    skos:notation "HS.0096"@en  ;
    rdfs:isDefinedBy scor: ;
    vs:term_status "testing" ;
    dct:modified "2015-11-05"^^xsd:date ;
 .

scor:ProductDevelopment
    rdf:type scor:Skill ;
    rdfs:comment "Familiarity and awareness of the Product Development process and its key steps and the interaction with the Source activity"@en  ;
    rdfs:label "Product Development"@en ;
    skos:notation "HS.0097"@en  ;
    rdfs:isDefinedBy scor: ;
    vs:term_status "testing" ;
    dct:modified "2015-11-05"^^xsd:date ;
 .

scor:ProductInformationManagement
    rdf:type scor:Skill ;
    rdfs:comment "The use of software or other tools to capture and maintain information on products and/or services through their life cycle"@en  ;
    rdfs:label "Product Information Management"@en ;
    skos:notation "HS.0098"@en  ;
    rdfs:isDefinedBy scor: ;
    vs:term_status "testing" ;
    dct:modified "2015-11-05"^^xsd:date ;
 .

scor:Production
    rdf:type scor:Skill ;
    rdfs:comment "The process of using machines, tools, materials and labor to make things for use or sale"@en  ;
    rdfs:label "Production"@en ;
    skos:notation "HS.0099"@en  ;
    rdfs:isDefinedBy scor: ;
    vs:term_status "testing" ;
    dct:modified "2015-11-05"^^xsd:date ;
 .

scor:ProductionPlanning
    rdf:type scor:Skill ;
    rdfs:comment "Actions, tasks and responsibilities concerned with the planning, scheduling and releasing of production orders in order to satisfy demand while optimizing the available and planned resources/capacity"@en  ;
    rdfs:label "Production Planning"@en ;
    skos:notation "HS.0101"@en  ;
    rdfs:isDefinedBy scor: ;
    vs:term_status "testing" ;
    dct:modified "2015-11-05"^^xsd:date ;
 .


# Standart Practice Individuals
scor:ConsignmentInventory
    rdf:type scor:StandardPractice ;
    rdfs:comment "The organization of source processes where the ownership of materials transfers are based on a signal further down in the supply chain (for example Make or Deliver)."@en  ;
    rdfs:label "Consignment Inventory"@en ;
    skos:notation "BP.006"@en  ;
    rdfs:isDefinedBy scor: ;
    vs:term_status "testing" ;
    dct:modified "2015-11-05"^^xsd:date ;
 .

scor:SlowMovingInventoryMonitoring
    rdf:type scor:StandardPractice ;
    rdfs:comment "Slow-moving inventory is defined as the value of those SKUs whose stock level is higher than the total consumption within the last 12 months"@en  ;
    rdfs:label "Slow-moving Inventory Monitoring"@en ;
    skos:notation "BP.008"@en  ;
    rdfs:isDefinedBy scor: ;
    vs:term_status "testing" ;
    dct:modified "2015-11-05"^^xsd:date ;
 .

scor:Kanban
    rdf:type scor:StandardPractice ;
    rdfs:comment "A inventory replenishment technique where a material is replenished based on consumption"@en  ;
    rdfs:label "Kanban"@en ;
    skos:notation "BP.009"@en  ;
    rdfs:isDefinedBy scor: ;
    vs:term_status "testing" ;
    dct:modified "2015-11-05"^^xsd:date ;
 .

scor:MinMaxReplenishment
    rdf:type scor:StandardPractice ;
    rdfs:comment "A inventory replenishment practice where purchase requisitions or purchase orders are created when inventory for an item drops below the Minimum inventory level"@en  ;
    rdfs:label "Min-Max Replenishment"@en ;
    skos:notation "BP.010"@en  ;
    rdfs:isDefinedBy scor: ;
    vs:term_status "testing" ;
    dct:modified "2015-11-05"^^xsd:date ;
 .

scor:LotTracking
    rdf:type scor:StandardPractice ;
    rdfs:comment "The practice of storing information about the history and/or genealogy of a product or material"@en  ;
    rdfs:label "Lot Tracking"@en ;
    skos:notation "BP.012"@en  ;
    rdfs:isDefinedBy scor: ;
    vs:term_status "testing" ;
    dct:modified "2015-11-05"^^xsd:date ;
 .

scor:ItemRationalization
    rdf:type scor:StandardPractice ;
    rdfs:comment "Rationalization of inventory at the item/part/SKU number level"@en  ;
    rdfs:label "Item Rationalization"@en ;
    skos:notation "BP.013"@en  ;
    rdfs:isDefinedBy scor: ;
    vs:term_status "testing" ;
    dct:modified "2015-11-05"^^xsd:date ;
 .

scor:SafetyStockPlanning
    rdf:type scor:StandardPractice ;
    rdfs:comment "Meet desired customer service levels while maintaining a minimum amount of safety stock"@en  ;
    rdfs:label "Safety Stock Planning"@en ;
    skos:notation "BP.015"@en  ;
    rdfs:isDefinedBy scor: ;
    vs:term_status "testing" ;
    dct:modified "2015-11-05"^^xsd:date ;
 .

scor:DistributionPlanning
    rdf:type scor:StandardPractice ;
    rdfs:comment "Determine the best short-term strategy to meet demand and to replenish stocking locations"@en  ;
    rdfs:label "Distribution Planning"@en ;
    skos:notation "BP.017"@en  ;
    rdfs:isDefinedBy scor: ;
    vs:term_status "testing" ;
    dct:modified "2015-11-05"^^xsd:date ;
 .

scor:ABCInventoryClassificationSystem
    rdf:type scor:StandardPractice ;
    rdfs:comment "The ABC classification system is the Pareto analysis of a range of inventory items, into three or four inventory categories"@en  ;
    rdfs:label "ABC Inventory Classification System"@en ;
    skos:notation "BP.018"@en  ;
    rdfs:isDefinedBy scor: ;
    vs:term_status "testing" ;
    dct:modified "2015-11-05"^^xsd:date ;
 .

scor:DemandPlanning
    rdf:type scor:StandardPractice ;
    rdfs:comment "Demand Planning is the process used for developing an accurate and comprehensive material forecast"@en  ;
    rdfs:label "Demand Planning"@en ;
    skos:notation "BP.019"@en  ;
    rdfs:isDefinedBy scor: ;
    vs:term_status "testing" ;
    dct:modified "2015-11-05"^^xsd:date ;
 .

scor:SalesOperationsPlanning
    rdf:type scor:StandardPractice ;
    rdfs:comment "Mid to Long Term supply chain planning practice which seeks to compare the forecast sales plan to the company resources, and analyze where any imbalances to the plan might exist"@en  ;
    rdfs:label "Sales and Operations Planning"@en ;
    skos:notation "BP.021"@en  ;
    rdfs:isDefinedBy scor: ;
    vs:term_status "testing" ;
    dct:modified "2015-11-05"^^xsd:date ;
 .

scor:MRPI
    rdf:type scor:StandardPractice ;
    rdfs:comment "A 'plan' scheme of different inventory management practices has been adopted by a company in a mixed model manufacturing environment"@en  ;
    rdfs:label "MRP I"@en ;
    skos:notation "BP.022"@en  ;
    rdfs:isDefinedBy scor: ;
    vs:term_status "testing" ;
    dct:modified "2015-11-05"^^xsd:date ;
 .

scor:ImproveSOPprocess
    rdf:type scor:StandardPractice ;
    rdfs:comment "Establish disciplined monthly cross-functional process to increase accuracy of demand management, establish biz inventory policy, and agreement on demand and supply balancing"@en  ;
    rdfs:label "Improve S and OP process"@en ;
    skos:notation "BP.026"@en  ;
    rdfs:isDefinedBy scor: ;
    vs:term_status "testing" ;
    dct:modified "2015-11-05"^^xsd:date ;
 .

scor:StockKeepingUnit
    rdf:type scor:StandardPractice ;
    rdfs:comment "Inventory reduction practice to determine which SKUs that can be terminated t using SKU Cost of Sales Analysis"@en  ;
    rdfs:label "Stock keeping Unit (SKU) Rationalization/Cost of Sales Analysis"@en ;
    skos:notation "BP.031"@en  ;
    rdfs:isDefinedBy scor: ;
    vs:term_status "testing" ;
    dct:modified "2015-11-05"^^xsd:date ;
 .

scor:DelayInboundSupplierShipments
    rdf:type scor:StandardPractice ;
    rdfs:comment "Analyze and execute a delay in inbound supplier raw material shipments to reduce raw material costs at summer break, end-of-year or other scheduled plant closure"@en  ;
    rdfs:label "Delay Inbound Supplier Shipments"@en ;
    skos:notation "BP.045"@en  ;
    rdfs:isDefinedBy scor: ;
    vs:term_status "testing" ;
    dct:modified "2015-11-05"^^xsd:date ;
 .

scor:ExpediteOutboundCustomerShipments
    rdf:type scor:StandardPractice ;
    rdfs:comment "The practice of analyzing the cost of maintaining inventory vs. the cost of transportation for opportunities to optimize total cost"@en  ;
    rdfs:label "Expedite Outbound Customer Shipments"@en ;
    skos:notation "BP.046"@en  ;
    rdfs:isDefinedBy scor: ;
    vs:term_status "testing" ;
    dct:modified "2015-11-05"^^xsd:date ;
 .

scor:ReturnAuthorization
    rdf:type scor:StandardPractice ;
    rdfs:comment "The Return Authorization (Return Material Authorization/Return Merchandise Authorization/Goods Return Authorization) process provides the inputs into the reverse logistics plan"@en  ;
    rdfs:label "Return Authorization"@en ;
    skos:notation "BP.135"@en  ;
    rdfs:isDefinedBy scor: ;
    vs:term_status "testing" ;
    dct:modified "2015-11-05"^^xsd:date ;
 .

scor:OutsourcedReverseLogistics
    rdf:type scor:StandardPractice ;
    rdfs:comment "Rather than manage returns as part of a service organization or operations many companies turn to outsourced service providers including Contract Manufacturers, EMS providers and Third Party Logistics providers for returns management"@en  ;
    rdfs:label "Outsourced Reverse Logistics"@en ;
    skos:notation "BP.136"@en  ;
    rdfs:isDefinedBy scor: ;
    vs:term_status "testing" ;
    dct:modified "2015-11-05"^^xsd:date ;
 .

scor:PurchaseOrderManagement
    rdf:type scor:StandardPractice ;
    rdfs:comment "The practice of issuing a purchase order for a number of products which are required in the short to mid term"@en  ;
    rdfs:label "Purchase Order Management"@en ;
    skos:notation "BP.144"@en  ;
    rdfs:isDefinedBy scor: ;
    vs:term_status "testing" ;
    dct:modified "2015-11-05"^^xsd:date ;
 .

scor:BPCrossDocking
    rdf:type scor:StandardPractice ;
    rdfs:comment "the practice of unloading materials from an incoming vehicle and loading these materials directly onto outbound vehicles without putting away into the regular storage locations in a warehouse"@en  ;
    rdfs:label "Cross-Docking"@en ;
    skos:notation "BP.146"@en  ;
    rdfs:isDefinedBy scor: ;
    vs:term_status "testing" ;
    dct:modified "2015-11-05"^^xsd:date ;
 .

scor:WayDeliveryVerification
    rdf:type scor:StandardPractice ;
    rdfs:comment "The practice of checking received invoices from suppliers against the quantities received and against the associated Purchase Order, Contract or Vendor Schedule"@en  ;
    rdfs:label "3-Way Delivery Verification"@en ;
    skos:notation "BP.148"@en  ;
    rdfs:isDefinedBy scor: ;
    vs:term_status "testing" ;
    dct:modified "2015-11-05"^^xsd:date ;
 .

scor:RotableSparesPool
    rdf:type scor:StandardPractice ;
    rdfs:comment "An inventory of serviceable parts that can replace a customers broken part to increase their recovery time"@en  ;
    rdfs:label "Rotable Spares Pool"@en ;
    skos:notation "BP.168"@en  ;
    rdfs:isDefinedBy scor: ;
    vs:term_status "testing" ;
    dct:modified "2015-11-05"^^xsd:date ;
 .

scor:BeyondEconomicRepairManagement
    rdf:type scor:StandardPractice ;
    rdfs:comment "The practice of assessing items as they are removed for Maintenance, Repair and Overhaul to determine whether repair would cost more than buying a replacement part"@en  ;
    rdfs:label "Beyond Economic Repair (BER) Management"@en ;
    skos:notation "BP.169"@en  ;
    rdfs:isDefinedBy scor: ;
    vs:term_status "testing" ;
    dct:modified "2015-11-05"^^xsd:date ;
 .

# Emerging Practice Individuals


scor:DemandPlanningForecasting
    rdf:type scor:EmergingPractice ;
    rdfs:comment "Use state-of-the-art forecasting algorithms for product life-cycle planning and trade promotion planning."@en  ;
    rdfs:label "Demand Planning Forecasting"@en ;
    skos:notation "BP.014"@en ;
    rdfs:isDefinedBy scor: ;
    vs:term_status "testing" ;
    dct:modified "2015-11-05"^^xsd:date ;
 .

scor:SupplyNetworkPlanning
    rdf:type scor:EmergingPractice ;
    rdfs:comment "Simulate and implement comprehensive tactical planning and sourcing decisions based on a single, globally consistent model."@en  ;
    rdfs:label "Supply Network Planning"@en ;
    skos:notation "BP.016"@en  ;
    rdfs:isDefinedBy scor: ;
    vs:term_status "testing" ;
    dct:modified "2015-11-05"^^xsd:date ;
 .

scor:BPDemandManagement
    rdf:type scor:EmergingPractice ;
    rdfs:comment "Takes Demand Planning to the next level and integrates the plan up and down the supply chain as well as across the enterprise."@en ;
    rdfs:label "Demand Management (Emerging Practice)"@en ;
    skos:notation "BP.020"@en ;
    rdfs:isDefinedBy scor: ;
    vs:term_status "testing" ;
    dct:modified "2015-11-05"^^xsd:date ;
 .

scor:BusinessRuleManagement
    rdf:type scor:EmergingPractice ;
    rdfs:comment "Business rules are in a (human-readable) form that are used by, but not embedded in, supply chain systems"@en ;
    rdfs:label "Business Rule Management"@en ;
      skos:notation "BP.023"@en ;
    rdfs:isDefinedBy scor: ;
    vs:term_status "testing" ;
    dct:modified "2015-11-05"^^xsd:date ;
 .

scor:SupplyChainOptimization
    rdf:type scor:EmergingPractice ;
    rdfs:comment "A part of the enterprise strategic plan for leading edge companies"@en ;
    rdfs:label "Supply Chain Optimization"@en ;
    skos:notation "BP.024"@en  ;
    rdfs:isDefinedBy scor: ;
    vs:term_status "testing" ;
    dct:modified "2015-11-05"^^xsd:date ;
 .

scor:SelfServiceWarrantyClaimSubmittal
    rdf:type scor:EmergingPractice ;
    rdfs:comment "enables customers and service providers to submit warranty claims over the web, reducing internal validation and processing workload. "@en;
    rdfs:label "Self-Service Warranty Claim Submittal"@en ;
    skos:notation "BP.025"@en  ;
    rdfs:isDefinedBy scor: ;
    vs:term_status "testing" ;
    dct:modified "2015-11-05"^^xsd:date ;
 .

scor:BusinessRuleReview
    rdf:type scor:EmergingPractice ;
    rdfs:comment "Is performed by supply chain middle and upper level management of an organization."@en ;
    rdfs:label "Business Rule Review"@en ;
    skos:notation "BP.035"@en ;
    rdfs:isDefinedBy scor: ;
    vs:term_status "testing" ;
    dct:modified "2015-11-05"^^xsd:date ;
 .

scor:LeanPlanning
    rdf:type scor:EmergingPractice ;
    rdfs:comment "Creates real world project plans which robustly model the project from initiation to final delivery."@en  ;
    rdfs:label "Lean Planning"@en ;
    skos:notation "BP.049"@en  ;
    rdfs:isDefinedBy scor: ;
    vs:term_status "testing" ;
    dct:modified "2015-11-05"^^xsd:date ;
 .

scor:ReturnsReceivingRefurbishment
    rdf:type scor:EmergingPractice ;
    rdfs:comment "The practice of refurbishing materials during the receiving processes (i.e. Source processes) for returned materials."@en  ;
    rdfs:label "Returns Receiving Refurbishment"@en ;
    skos:notation "BP.073"@en  ;
    rdfs:isDefinedBy scor: ;
    vs:term_status "testing" ;
    dct:modified "2015-11-05"^^xsd:date ;
 .

scor:LoanerProgram
    rdf:type scor:EmergingPractice ;
    rdfs:comment "In order to minimize lost productivity, many companies offer a loaner program for their customers when they need to return a defective product."@en  ;
    rdfs:label "Loaner Program"@en ;
    skos:notation "BP.079"@en  ;
    rdfs:isDefinedBy scor: ;
    vs:term_status "testing" ;
    dct:modified "2015-11-05"^^xsd:date ;
 .

scor:MobileAccessOfInformation
    rdf:type scor:EmergingPractice ;
    rdfs:comment "Mobile access to information in supply chain means information on status metrics supply and demand are available in the internet smart phones and other similar mobile devices."@en  ;
    rdfs:label "Mobile Access of Information"@en ;
    skos:notation "BP.098"@en  ;
    rdfs:isDefinedBy scor: ;
    vs:term_status "testing" ;
    dct:modified "2015-11-05"^^xsd:date ;
 .

scor:ReturnPolicyConformanceIntegration
    rdf:type scor:EmergingPractice ;
    rdfs:comment "The practice of implementing standard procedures and enableing technology to ensure conformance to return policies."@en  ;
    rdfs:label "Return Policy Conformance Integration"@en ;
    skos:notation "BP.108"@en  ;
    rdfs:isDefinedBy scor: ;
    vs:term_status "testing" ;
    dct:modified "2015-11-05"^^xsd:date ;
 .

scor:CarcassPrepositioning
    rdf:type scor:EmergingPractice ;
    rdfs:comment "The practice of making disposition decisions for reparable parts/cores/carcasses early in the (Return Material Authorization) RMA process."@en ;
    rdfs:label "Carcass Prepositioning"@en ;
    skos:notation "BP.109"@en ;
    rdfs:isDefinedBy scor: ;
    vs:term_status "testing" ;
    dct:modified "2015-11-05"^^xsd:date ;
 .

scor:EmbedSpecializedServices
    rdf:type scor:EmergingPractice ;
    rdfs:comment "Add additional capability, processes and expertise by embedding specialized packaging, product completion and pack out services on-site from a 3rd party provider."@en  ;
    rdfs:label "Embed Specialized Services"@en ;
    skos:notation "BP.117"@en ;
    rdfs:isDefinedBy scor: ;
    vs:term_status "testing" ;
    dct:modified "2015-11-05"^^xsd:date ;
 .

scor:TransportationManagementOutsourcing
    rdf:type scor:EmergingPractice ;
    rdfs:comment "Outsourcing transportation creates an opportunity for small businesses to combine their transportation spend and get a lower overall tariff rate."@en  ;
    rdfs:label "Transportation Management Outsourcing"@en ;
    skos:notation "BP.118"@en  ;
    rdfs:isDefinedBy scor: ;
    vs:term_status "testing" ;
    dct:modified "2015-11-05"^^xsd:date ;
 .

scor:ThreeDPrintRapidProtoyping
    rdf:type scor:EmergingPractice ;
    rdfs:comment "3D printing is a phrase used to describe the process of creating three dimensional objects from digital file using a materials printer, in a manner similar to printing images on paper."@en  ;
    rdfs:label "3D Print Rapid Protoyping"@en ;
    skos:notation "BP.120"@en  ;
    rdfs:isDefinedBy scor: ;
    vs:term_status "testing" ;
    dct:modified "2015-11-05"^^xsd:date ;
 .

scor:DigitalPackagingOnDemand
    rdf:type scor:EmergingPractice ;
    rdfs:comment "The use of digital packaging printing to create custom product packaging unique to the customer and the product requirements."@en  ;
    rdfs:label "Digital Packaging on Demand"@en ;
    skos:notation "BP.121"@en ;
    rdfs:isDefinedBy scor: ;
    vs:term_status "testing" ;
    dct:modified "2015-11-05"^^xsd:date ;
 .

scor:CarcassDisassembly
    rdf:type scor:EmergingPractice ;
    rdfs:comment "Returned Maintenance, Repair, Operations (MRO) items are disassembled to the bill of material level and component parts are tested."@en ;
    rdfs:label "Carcass Disassembly"@en ;
    skos:notation "BP.137"@en ;
    rdfs:isDefinedBy scor: ;
    vs:term_status "testing" ;
    dct:modified "2015-11-05"^^xsd:date ;
 .

scor:BarCodingRFID
    rdf:type scor:EmergingPractice ;
    rdfs:comment "Bar coding is the practice of adding machine readable labels to packaging of goods, in order to increase reading speed and reducing reading errors."@en  ;
    rdfs:label "Bar Coding RFID"@en ;
    skos:notation "BP.153"@en  ;
    rdfs:isDefinedBy scor: ;
    vs:term_status "testing" ;
    dct:modified "2015-11-05"^^xsd:date ;
 .

scor:EnterpriseLevelSpendAnalysis
    rdf:type scor:EmergingPractice ;
    rdfs:comment "Spend analysis involved collection of data across procures to pay process in an enterprise and slicing and dicing these data into useful information."@en  ;
    rdfs:label "Enterprise Level Spend Analysis"@en ;
    skos:notation "BP.161"@en  ;
    rdfs:isDefinedBy scor: ;
    vs:term_status "testing" ;
    dct:modified "2015-11-05"^^xsd:date ;
 .

scor:LongTermSupplierAgreementPartnership
    rdf:type scor:EmergingPractice ;
    rdfs:comment "The Long Term Supplier Agreement/Partnership is a communication framework of buyer and supplier relationship."@en  ;
    rdfs:label "Long Term Supplier Agreement Partnership"@en ;
    skos:notation "BP.162"@en  ;
    rdfs:isDefinedBy scor: ;
    vs:term_status "testing" ;
    dct:modified "2015-11-05"^^xsd:date ;
 .

scor:MixedModeReverseMaterialIssue
    rdf:type scor:EmergingPractice ;
    rdfs:comment "Backflush is a concept where issuing of the material automatically happens once the finished product is ready."@en  ;
    rdfs:label "Mixed Mode Reverse Material Issue"@en ;
    skos:notation "BP.171"@en  ;
    rdfs:isDefinedBy scor: ;
    vs:term_status "testing" ;
    dct:modified "2015-11-05"^^xsd:date ;
 .

scor:ProductionSchedulingOptimizationUsingTech
    rdf:type scor:EmergingPractice ;
    rdfs:comment "Effective scheduling should not only include production related attributes (e.g. rated/demonstrated capacity asset loading sequencing changeover constraints etc.) but also other directly and indirectly related processes."@en  ;
    rdfs:label "Production Scheduling Optimization Using Tech"@en ;
    skos:notation "BP.172"@en  ;
    rdfs:isDefinedBy scor: ;
    vs:term_status "testing" ;
    dct:modified "2015-11-05"^^xsd:date ;
 .


# Best Practices individuals

scor:SCRiskManagement
    rdf:type scor:BestPractice ;
    rdfs:comment "the systematic identification, assessment and mitigation of potential disruptions in logistics networks"@en  ;
    rdfs:label "Supply Chain Risk Management"@en  ;
    skos:notation "BP.001"@en  ;
    rdfs:isDefinedBy scor: ;
    vs:term_status "testing" ;
    dct:modified "2015-11-05"^^xsd:date ;
 .

scor:RiskManagementStrategies
    rdf:type scor:BestPractice ;
    rdfs:comment "Risk management strategies are developed and communicated. Commonly used strategies are Risk Mitigation, Risk Avoidance, Risk Transfer and also Risk Acceptance"@en  ;
    rdfs:label "Risk Management Strategies"@en  ;
    skos:notation "BP.002"@en  ;
    rdfs:isDefinedBy scor: ;
    vs:term_status "testing" ;
    dct:modified "2015-11-05"^^xsd:date ;
 .

scor:SingleMinuteExchangeOfDie
    rdf:type scor:BestPractice ;
    rdfs:comment "The practice of reducing the time it takes to change a production line, equipment or machine from running one product to the next"@en  ;
    rdfs:label "Single-Minute Exchange of Die (SMED)"@en  ;
    skos:notation "BP.003"@en  ;
    rdfs:isDefinedBy scor: ;
    vs:term_status "testing" ;
    dct:modified "2015-11-05"^^xsd:date ;
 .

scor:NetworkPrioritizationForRiskIdentification
    rdf:type scor:BestPractice ;
    rdfs:comment "Network prioritization for risk identification is the process of prioritizing parts of a supply chain for risk analysis based on the overall risk potential in each portion of the supply chain"@en  ;
    rdfs:label "Network Prioritization for Risk Identification"@en  ;
    skos:notation "BP.004"@en  ;
    rdfs:isDefinedBy scor: ;
    vs:term_status "testing" ;
    dct:modified "2015-11-05"^^xsd:date ;
 .

scor:SelfInvoicing
    rdf:type scor:BestPractice ;
    rdfs:comment "The practice where a customer generates the invoices for the products or services it consumed from a supplier"@en  ;
    rdfs:label "Self-Invoicing"@en  ;
    skos:notation "BP.005"@en  ;
    rdfs:isDefinedBy scor: ;
    vs:term_status "testing" ;
    dct:modified "2015-11-05"^^xsd:date ;
 .

scor:BaselineInventoryMonitoring
    rdf:type scor:BestPractice ;
    rdfs:comment "To avoid overstock situations, we regularly review Baseline inventory levels. Baseline inventory is defined as the lowest stock level that a particular SKU actually had during the last 12 months."@en  ;
    rdfs:label "Baseline Inventory Monitoring"@en  ;
    skos:notation "BP.007"@en  ;
    rdfs:isDefinedBy scor: ;
    vs:term_status "testing" ;
    dct:modified "2015-11-05"^^xsd:date ;
 .

scor:ProductionLineSequencing
    rdf:type scor:BestPractice ;
    rdfs:comment "The practice where materials are ordered, shipped, received and/or staged in the same sequence as they will be consumed."@en  ;
    rdfs:label "Production Line Sequencing"@en  ;
    skos:notation "BP.011"@en  ;
    rdfs:isDefinedBy scor: ;
    vs:term_status "testing" ;
    dct:modified "2015-11-05"^^xsd:date ;
 .

scor:PullBasedInventoryReplenishment
    rdf:type scor:BestPractice ;
    rdfs:comment "Pull-based (Demand) replenishment is an approach that utilizes customer demand (`pull`) to replace and optimize inventory while reducing total net landed cost."@en  ;
    rdfs:label "Pull-Based Inventory Replenishment"@en  ;
    skos:notation "BP.027"@en  ;
    rdfs:isDefinedBy scor: ;
    vs:term_status "testing" ;
    dct:modified "2015-11-05"^^xsd:date ;
 .

scor:InventoryOptimization
    rdf:type scor:BestPractice ;
    rdfs:comment "Use of multi-echelon (simultaneous across all inventory stocking points in supply chain) stochastic (random variability) optimization."@en  ;
    rdfs:label "Inventory Optimization"@en  ;
    skos:notation "BP.028"@en  ;
    rdfs:isDefinedBy scor: ;
    vs:term_status "testing" ;
    dct:modified "2015-11-05"^^xsd:date ;
 .

scor:InventoryManagementBP029
    rdf:type scor:BestPractice ;
    rdfs:comment "Supply chains and supply networks both describe the flow and movement of materials & information, by linking organizations together to serve the end-customer."@en  ;
    rdfs:label "Inventory Management Using Supply Chain Network Optimization"@en  ;
    skos:notation "BP.029"@en  ;
    rdfs:isDefinedBy scor: ;
    vs:term_status "testing" ;
    dct:modified "2015-11-05"^^xsd:date ;
 .

scor:InventoryRecordAccuracy
    rdf:type scor:BestPractice ;
    rdfs:comment "Establish disciplined monthly process to ensure timely reporting of accurate inventory (physical inventory matches ERP inventory & identify sitting inventory not identified by a SKU) at the manufacturing and terminal locations."@en  ;
    rdfs:label "Inventory Record Accuracy"@en  ;
    skos:notation "BP.030"@en  ;
    rdfs:isDefinedBy scor: ;
    vs:term_status "testing" ;
    dct:modified "2015-11-05"^^xsd:date ;
 .

scor:ReduceSlowMovingInventory
    rdf:type scor:BestPractice ;
    rdfs:comment "Analyze and determine what inventory can be written off due to age, shelf-life, and/or lack of demand."@en  ;
    rdfs:label "Reduce / Write-off Slow Moving Inventory"@en  ;
    skos:notation "BP.032"@en  ;
    rdfs:isDefinedBy scor: ;
    vs:term_status "testing" ;
    dct:modified "2015-11-05"^^xsd:date ;
 .

scor:TraditionalDemandForecastingImprovement
    rdf:type scor:BestPractice ;
    rdfs:comment "Use of more sophisticated qualitative and quantitative forecasting processes and tools to improve customer demand forecast typically at SKU level."@en  ;
    rdfs:label "Traditional Demand Forecasting Improvement"@en  ;
    skos:notation "BP.033"@en  ;
    rdfs:isDefinedBy scor: ;
    vs:term_status "testing" ;
    dct:modified "2015-11-05"^^xsd:date ;
 .

scor:ExtendInventoryBP34
    rdf:type scor:BestPractice ;
    rdfs:comment "Collaborative inventory planning can be used as a way to extend supply chain planning with key customers."@en  ;
    rdfs:label "Extend Inventory Planning using Collaboration (Key Suppliers)"@en  ;
    skos:notation "BP.034"@en  ;
    rdfs:isDefinedBy scor: ;
    vs:term_status "testing" ;
    dct:modified "2015-11-05"^^xsd:date ;
 .

scor:ConsignmentInventoryWithSuppliers
    rdf:type scor:BestPractice ;
    rdfs:comment "Consignment inventory is a family of business models in which the buyer of a product provides certain information to a supplier of that product and the supplier takes full responsibility for maintaining an agreed of the material, usually at the buyer's consumption location (usually a store)."@en  ;
    rdfs:label "Consignment Inventory with Key Suppliers"@en  ;
    skos:notation "BP.036"@en  ;
    rdfs:isDefinedBy scor: ;
    vs:term_status "testing" ;
    dct:modified "2015-11-05"^^xsd:date ;
 .

scor:ManufacturingDirectDropShipment
    rdf:type scor:BestPractice ;
    rdfs:comment "The practice of shipping products and goods directly from the manufacturing plant to the customer (bypassing consolidation activities in warehouses and/or distribution centers)."@en  ;
    rdfs:label "Manufacturing Direct/Drop Shipment"@en  ;
    skos:notation "BP.037"@en  ;
    rdfs:isDefinedBy scor: ;
    vs:term_status "testing" ;
    dct:modified "2015-11-05"^^xsd:date ;
 .

scor:BatchSizeReduction
    rdf:type scor:BestPractice ;
    rdfs:comment "Use Lean principles to reduce size of manufacturing batch sizes to better match customer demand vs. asset utilization/quality issues."@en  ;
    rdfs:label "Batch Size Reduction"@en  ;
    skos:notation "BP.038"@en  ;
    rdfs:isDefinedBy scor: ;
    vs:term_status "testing" ;
    dct:modified "2015-11-05"^^xsd:date ;
 .

scor:RightSizeFrequencyOfProductionWheel
    rdf:type scor:BestPractice ;
    rdfs:comment "Use Lean principles to increase frequency/agility of production wheel, or production cycle in order to modify production planning and right-size finished goods and work-in-process inventory."@en  ;
    rdfs:label "Right Size Frequency of Production Wheel"@en  ;
    skos:notation "BP.039"@en  ;
    rdfs:isDefinedBy scor: ;
    vs:term_status "testing" ;
    dct:modified "2015-11-05"^^xsd:date ;
 .

scor:MTOOrderFulfillmentStrategy
    rdf:type scor:BestPractice ;
    rdfs:comment "Evaluate potential to change order fulfillment strategy from Make-To-Stock (MTS) to Make-To-Order (MTO) SKU by SKU to offset need to carry inventory due to infrequent demand or low demand."@en  ;
    rdfs:label "MTO Order Fulfillment Strategy"@en  ;
    skos:notation "BP.040"@en  ;
    rdfs:isDefinedBy scor: ;
    vs:term_status "testing" ;
    dct:modified "2015-11-05"^^xsd:date ;
 .

scor:TransportationOptimization
    rdf:type scor:BestPractice ;
    rdfs:comment "Evaluate potential to change inbound/outbound transportation mode to `faster` mode depending on freight terms (FOB, etc.) to accelerate transfer of inventory title to customer and/or better match demand/supply to optimize inventory balances."@en  ;
    rdfs:label "Transportation Optimization"@en  ;
    skos:notation "BP.041"@en  ;
    rdfs:isDefinedBy scor: ;
    vs:term_status "testing" ;
    dct:modified "2015-11-05"^^xsd:date ;
 .

scor:ReviewOfProcurementTermsConditions
    rdf:type scor:BestPractice ;
    rdfs:comment "Evaluate potential to change inbound/outbound transportation mode to `faster` mode depending on freight terms (FOB, etc.) to accelerate transfer of inventory title to customer and/or better match demand/supply to optimize inventory balances."@en  ;
    rdfs:label "Regular Review of Procurement Terms and Conditions"@en  ;
    skos:notation "BP.042"@en  ;
    rdfs:isDefinedBy scor: ;
    vs:term_status "testing" ;
    dct:modified "2015-11-05"^^xsd:date ;
 .

scor:ConsignmentInventoryReduction
    rdf:type scor:BestPractice ;
    rdfs:comment "Analyze potential to reduce consignment inventory commitments. These are typically included as part of the terms and conditions of customer contracts."@en  ;
    rdfs:label "Consignment Inventory Reduction"@en  ;
    skos:notation "BP.043"@en  ;
    rdfs:isDefinedBy scor: ;
    vs:term_status "testing" ;
    dct:modified "2015-11-05"^^xsd:date ;
 .

scor:InventoryFinancingEvaluation
    rdf:type scor:BestPractice ;
    rdfs:comment "Evaluate potential to use external finance company to `purchase inventory` while in-transit or in certain circumstances and sell back to the company prior to delivery to customer."@en  ;
    rdfs:label "Inventory Financing Evaluation"@en  ;
    skos:notation "BP.044"@en  ;
    rdfs:isDefinedBy scor: ;
    vs:term_status "testing" ;
    dct:modified "2015-11-05"^^xsd:date ;
 .

scor:FinishedGoodsInventoryPostponement
    rdf:type scor:BestPractice ;
    rdfs:comment "Provide process to determine and execute optimum placement and volume for Inventory in the Value Stream (Chain). Requires analysis of Value Stream and identification of opportunities for Demand Pooling of materials."@en  ;
    rdfs:label "Finished Goods Inventory Postponement"@en  ;
    skos:notation "BP.047"@en  ;
    rdfs:isDefinedBy scor: ;
    vs:term_status "testing" ;
    dct:modified "2015-11-05"^^xsd:date ;
 .

scor:InventoryIncentives
    rdf:type scor:BestPractice ;
    rdfs:comment "Balance cost/value of offering discounts for customers to move forward orders on specific finished good products in inventory."@en  ;
    rdfs:label "Inventory incentives / promotions for customers"@en  ;
    skos:notation "BP.048"@en  ;
    rdfs:isDefinedBy scor: ;
    vs:term_status "testing" ;
    dct:modified "2015-11-05"^^xsd:date ;
 .

scor:CustomerIncentives
    rdf:type scor:BestPractice ;
    rdfs:comment "Provide a one time improvement in finished good inventory; Requires analysis of value/cost trade-off to insure proper incentive."@en  ;
    rdfs:label "Customer Incentives/Promotions for Large Inventory Purchases"@en  ;
    skos:notation "BP.050"@en  ;
    rdfs:isDefinedBy scor: ;
    vs:term_status "testing" ;
    dct:modified "2015-11-05"^^xsd:date ;
 .

scor:EmbedInventoryManagementGoals
    rdf:type scor:BestPractice ;
    rdfs:comment "Develop method to embed and track specific inventory management goals for the business for all functions within the business due to cross-functional issues associated with inventory vs. service level."@en  ;
    rdfs:label "Embed Inventory Management Goals"@en  ;
    skos:notation "BP.051"@en  ;
    rdfs:isDefinedBy scor: ;
    vs:term_status "testing" ;
    dct:modified "2015-11-05"^^xsd:date ;
 .

scor:DesignForLogisticsManagement
    rdf:type scor:BestPractice ;
    rdfs:comment "Change new product development process to embed reuse and/or risk assessment around inventory management (e.g., include check off from supply chain of potential inventory management impact of proposed new product development). This could include mandatory end of lifecycle for another product, Commercial`s agreement to potential inventory/working capital exposure, etc."@en  ;
    rdfs:label "Design for Logistics (DFL) Management"@en  ;
    skos:notation "BP.052"@en  ;
    rdfs:isDefinedBy scor: ;
    vs:term_status "testing" ;
    dct:modified "2015-11-05"^^xsd:date ;
 .

scor:ManufacturingReliabilityImprovement
    rdf:type scor:BestPractice ;
    rdfs:comment "The practice includes use of reliability tools and implementation of work process roles within manufacturing to address manufacturing reliability."@en  ;
    rdfs:label "Manufacturing Reliability Improvement"@en  ;
    skos:notation "BP.053"@en  ;
    rdfs:isDefinedBy scor: ;
    vs:term_status "testing" ;
    dct:modified "2015-11-05"^^xsd:date ;
 .

scor:ManufacturingQualityImprovementsBP054
    rdf:type scor:BestPractice ;
    rdfs:comment "This consists of efforts to address manufacturing quality & improving manufacturing cost/capacity and service factor."@en  ;
    rdfs:label "Manufacturing Quality Improvements for Return Reduction"@en  ;
    skos:notation "BP.054"@en  ;
    rdfs:isDefinedBy scor: ;
    vs:term_status "testing" ;
    dct:modified "2015-11-05"^^xsd:date ;
 .

scor:FreightCarrierDeliveryBP55
    rdf:type scor:BestPractice ;
    rdfs:comment "The practice of formal freight carrier performance reviews to reduce the risk of landed cost budget variances."@en  ;
    rdfs:label "Freight Carrier Delivery Performance Evaluation"@en  ;
    skos:notation "BP.055"@en  ;
    rdfs:isDefinedBy scor: ;
    vs:term_status "testing" ;
    dct:modified "2015-11-05"^^xsd:date ;
 .

scor:SupplierRawMaterialBP56
    rdf:type scor:BestPractice ;
    rdfs:comment "Provide analysis of potential value that could be gained from raw material inventory reduction (in addition to traditional manufacturing quality/capacity and service factors)."@en  ;
    rdfs:label "Supplier Raw Material Quality Improvement"@en  ;
    skos:notation "BP.056"@en  ;
    rdfs:isDefinedBy scor: ;
    vs:term_status "testing" ;
    dct:modified "2015-11-05"^^xsd:date ;
 .

scor:InventoryManagementTraining
    rdf:type scor:BestPractice ;
    rdfs:comment "Develop a training curriculum and monitor key employee participation/completion in the areas of inventory management (particularly with schedulers, planners, SC managers) as well as exposure to  emerging best practices/technology (e.g., inventory optimization.)."@en  ;
    rdfs:label "Inventory Management Training"@en  ;
    skos:notation "BP.058"@en  ;
    rdfs:isDefinedBy scor: ;
    vs:term_status "testing" ;
    dct:modified "2015-11-05"^^xsd:date ;
 .

scor:EmployeeIncentivesInventoryBP59
    rdf:type scor:BestPractice ;
    rdfs:comment "Effective inventory management is the result of outstanding inventory control and inventory management."@en  ;
    rdfs:label "Employee Incentives for Effective Inventory Management"@en  ;
    skos:notation "BP.059"@en  ;
    rdfs:isDefinedBy scor: ;
    vs:term_status "testing" ;
    dct:modified "2015-11-05"^^xsd:date ;
 .

scor:OrderLeadTimeCorrectiveAction
    rdf:type scor:BestPractice ;
    rdfs:comment "Attaining acceptable delivery performance is the most significant manufacturing challenge faced by many organizations."@en  ;
    rdfs:label "Order Lead Time Corrective Action"@en  ;
    skos:notation "BP.060"@en  ;
    rdfs:isDefinedBy scor: ;
    vs:term_status "testing" ;
    dct:modified "2015-11-05"^^xsd:date ;
 .

scor:ReduceNonStrategicInventoryLevel
    rdf:type scor:BestPractice ;
    rdfs:comment "Unsold inventory is not `money in the bank`. A company should identify idle assets by analyzing production records, reviewing stock status reports to isolate inventory that is slow moving or out of balance, and sell/reduce the nonstrategic inventory."@en  ;
    rdfs:label "Reduce Non-Strategic Inventory Level"@en  ;
    skos:notation "BP.061"@en  ;
    rdfs:isDefinedBy scor: ;
    vs:term_status "testing" ;
    dct:modified "2015-11-05"^^xsd:date ;
 .

scor:MasterDataAccuracy
    rdf:type scor:BestPractice ;
    rdfs:comment "Re-validate existing Master Data (order lead times, replenishment times, transit times, etc.) to ensure it matches current operational capabilities and performance."@en  ;
    rdfs:label "Master Data Accuracy"@en  ;
    skos:notation "BP.061"@en  ;
    rdfs:isDefinedBy scor: ;
    vs:term_status "testing" ;
    dct:modified "2015-11-05"^^xsd:date ;
 .

scor:OptimizeSourcingDecisionsBP63
    rdf:type scor:BestPractice ;
    rdfs:comment "Assess potential to change sourcing decisions to local source point (likely the optimal source point) to reduce overall replenishment lead time."@en  ;
    rdfs:label "Optimize Sourcing Decisions to Local Source Point"@en  ;
    skos:notation "BP.063"@en  ;
    rdfs:isDefinedBy scor: ;
    vs:term_status "testing" ;
    dct:modified "2015-11-05"^^xsd:date ;
 .

scor:SafetyStockReduction
    rdf:type scor:BestPractice ;
    rdfs:comment "Pursue a more aggressive Reorder Point / safety stock target replenishment stance that places more risk on the chance of a stock out."@en  ;
    rdfs:label "Safety Stock Reduction"@en  ;
    skos:notation "BP.064"@en  ;
    rdfs:isDefinedBy scor: ;
    vs:term_status "testing" ;
    dct:modified "2015-11-05"^^xsd:date ;
 .

scor:SeasonalPackagingChange
    rdf:type scor:BestPractice ;
    rdfs:comment "What constitutes seasonal varies from organization to organization. From a requirements determination perspective however seasonal items may be classified as items that have less than six months of demand in the preceding 12 months."@en  ;
    rdfs:label "Seasonal Packaging Reduction/Removal"@en  ;
    skos:notation "BP.065"@en  ;
    rdfs:isDefinedBy scor: ;
    vs:term_status "testing" ;
    dct:modified "2015-11-05"^^xsd:date ;
 .

scor:ReduceReturnsInventoryBP66
    rdf:type scor:BestPractice ;
    rdfs:comment "Evaluate and establish a business returns policy (buyer`s remorse, defectives, warranty, overstock, Root Cause Investigation to determine & eliminate return cause, etc.) including determining its impact to overall inventory management."@en  ;
    rdfs:label "Returns Policy to Reduce Returns Inventory"@en  ;
    skos:notation "BP.066"@en  ;
    rdfs:isDefinedBy scor: ;
    vs:term_status "testing" ;
    dct:modified "2015-11-05"^^xsd:date ;
 .

scor:ReturnsInventoryReduction
    rdf:type scor:BestPractice ;
    rdfs:comment "Develop a process for efficiently receiving, processing and disposition of returned products."@en  ;
    rdfs:label "Returns Inventory Reduction"@en  ;
    skos:notation "BP.067"@en  ;
    rdfs:isDefinedBy scor: ;
    vs:term_status "testing" ;
    dct:modified "2015-11-05"^^xsd:date ;
 .

scor:SupplierDeliveryPerformanceAnalysis
    rdf:type scor:BestPractice ;
    rdfs:comment "Track and analyze the on time delivery performance for suppliers.."@en  ;
    rdfs:label "Supplier Delivery Performance Analysis"@en  ;
    skos:notation "BP.068"@en  ;
    rdfs:isDefinedBy scor: ;
    vs:term_status "testing" ;
    dct:modified "2015-11-05"^^xsd:date ;
 .

scor:RawMaterialsReceivingProcess
    rdf:type scor:BestPractice ;
    rdfs:comment "Develop process for efficiently receiving and processing raw materials from suppliers to minimize receipt of raw materials."@en  ;
    rdfs:label "Raw Materials Receiving Process"@en  ;
    skos:notation "BP.069"@en  ;
    rdfs:isDefinedBy scor: ;
    vs:term_status "testing" ;
    dct:modified "2015-11-05"^^xsd:date ;
 .

scor:PlanningInventoryTraining
    rdf:type scor:BestPractice ;
    rdfs:comment "Improve employee knowledge of inventory control to increase level of performance in inventory management."@en  ;
    rdfs:label "Planning/scheduling inventory training"@en  ;
    skos:notation "BP.070"@en  ;
    rdfs:isDefinedBy scor: ;
    vs:term_status "testing" ;
    dct:modified "2015-11-05"^^xsd:date ;
 .

scor:CostsInventoryStockingBP71
    rdf:type scor:BestPractice ;
    rdfs:comment "Balance the trade-off between logistics cost reduction and increased capital costs."@en  ;
    rdfs:label "Freight Costs and Inventory Stocking Optimization"@en  ;
    skos:notation "BP.071"@en  ;
    rdfs:isDefinedBy scor: ;
    vs:term_status "testing" ;
    dct:modified "2015-11-05"^^xsd:date ;
 .

scor:InboundRMAEnabledProcessing
    rdf:type scor:BestPractice ;
    rdfs:comment "This practice of requiring and enforcing a return shipment is accompanied by a company-issued Return Material (or Merchandise) Authorization (or Agreement) (RMA)."@en  ;
    rdfs:label "Inbound RMA-enabled Processing"@en  ;
    skos:notation "BP.072"@en  ;
    rdfs:isDefinedBy scor: ;
    vs:term_status "testing" ;
    dct:modified "2015-11-05"^^xsd:date ;
 .

scor:ProcessMetricsAlignment
    rdf:type scor:BestPractice ;
    rdfs:comment "Metric alignment refers to the organized and deliberate development of metrics across an organization. The process starts with organizational/business or supply chain metrics then decomposes to organizational processes at level-2, level-3, and further if desired."@en  ;
    rdfs:label "Process/Metrics Alignment"@en  ;
    skos:notation "BP.074"@en  ;
    rdfs:isDefinedBy scor: ;
    vs:term_status "testing" ;
    dct:modified "2015-11-05"^^xsd:date ;
 .

