# baseURI: http://eis.iai.uni-bonn.de/openscorvoc#
# imports: http://purl.org/dc/elements/1.1/
# imports: http://www.w3.org/2004/02/skos/core

@prefix :        <http://www.semanticweb.org/owl/owlapi/turtle#> .
@prefix daq:     <http://purl.org/eis/vocab/daq#> .
@prefix dc:      <http://purl.org/dc/elements/1.1/> .
@prefix gr:      <http://purl.org/goodrelations/v1#> .
@prefix owl:     <http://www.w3.org/2002/07/owl#> .
@prefix rdf:     <http://www.w3.org/1999/02/22-rdf-syntax-ns#> .
@prefix rdfs:    <http://www.w3.org/2000/01/rdf-schema#> .
@prefix scor:    <http://eis.iai.uni-bonn.de/openscorvoc#> .
@prefix skos:    <http://www.w3.org/2004/02/skos/core#> .
@prefix xml:     <http://www.w3.org/XML/1998/namespace> .
@prefix xsd:     <http://www.w3.org/2001/XMLSchema#> .

<http://eis.iai.uni-bonn.de/openscorvoc#>
      rdf:type owl:Ontology ;
      rdfs:comment "Supply Chain Operation Reference Vocabulary has the purpose to represent the information about the Supply Chain in order to use this in a Linked Data environement"@en ;
      rdfs:label "Supply Chain Operation Reference Vocabulary"^^xsd:string ;
      dc:date "2014-10-05T12:52:16"^^xsd:dateTime ;
      owl:imports <http://www.w3.org/2004/02/skos/core> , dc: .

scor:Process
      rdf:type owl:Class ;
      rdfs:comment "A process is a unique activity performed to meet predefined outcomes"@en ;
      rdfs:label "Process" .
	  
# Level 1 Processes

scor:Plan
      rdf:type owl:Class ;
      rdfs:comment "Describes the planning activities associated with operating a supply chain. This includes gathering customer requirements, collecting information on available resources, and balancing requirements and resources to determine planned capabilities and resource gaps. This is followed by identifying the actions required to correct any gaps."@en ;
      rdfs:label "Plan" ;
      rdfs:subClassOf scor:Process ;
      scor:hasProcessID "P" ;
      skos:altLabel "sP" .
	  
scor:Source
      rdf:type owl:Class ;
      rdfs:comment "Order, deliver, receipt and transfer of raw material items, subassemblies, product and/or services"@en ;
      rdfs:label "Source" ;
      rdfs:subClassOf scor:Process ;
      scor:hasProcessID "S" ;
      skos:altLabel "sS" .	

scor:Make
      rdf:type owl:Class ;
      rdfs:comment "Adds value to products through mixing, separating, forming, machining, and chemical processes"@en ;
      rdfs:label "Make" ;
      rdfs:subClassOf scor:Process ;
      scor:hasProcessID "M" ;
      skos:altLabel "sM" .	

scor:Deliver
      rdf:type owl:Class ;
      rdfs:comment "Performs customer-facing order management and order fulfillment activities"@en ;
      rdfs:label "Deliver" ;
      rdfs:subClassOf scor:Process ;
      scor:hasProcessID "D" ;
      skos:altLabel "sD" .	

scor:Return
      rdf:type owl:Class ;
      rdfs:comment "Moves material from a customer back through the supply chain to address defects in product, ordering, or manufacturing, or to perform upkeep activities"@en ;
      rdfs:label "Return" ;
      rdfs:subClassOf scor:Process ;
      scor:hasProcessID "R" ;
      skos:altLabel "sR" .	  

scor:Enable
      rdf:type owl:Class ;
      rdfs:comment "Establishing, maintaining and monitoring information, relationships, resources, assets, business rules, compliance and contracts required to operate the supply chain"@en ;
      rdfs:label "Enable" ;
      rdfs:subClassOf scor:Process ;
      scor:hasProcessID "E" ;
      skos:altLabel "sE" .
	  
# Level 2 Processes 

# Plan 	  

scor:PlanSupplyChain
      rdf:type owl:Class ;
      rdfs:comment "The development and establishment of courses of action over specified time periods that represent a projected appropriation of supply chain resources to meet supply chain requirements for the longest time fence constraints of supply resources"@en ;
      rdfs:label "Plan Supply Chain" ;
      rdfs:subClassOf scor:Plan ;
      skos:altLabel "sP1" .

scor:PlanSource
      rdf:type owl:Class ;
      rdfs:comment "The development and establishment of courses of action over specified time periods that represent a projected appropriation of material resources to meet supply chain requirements"@en ;
      rdfs:label "Plan Source" ;
      rdfs:subClassOf scor:Plan ;
      skos:altLabel "sP2" .

scor:PlanMake
      rdf:type owl:Class ;
      rdfs:comment "The development and establishment of courses of action over specified time periods that represent a projected appropriation of production resources to meet production requirements"@en ;
      rdfs:label "Plan Make" ;
      rdfs:subClassOf scor:Plan ;
      skos:altLabel "sP3" .
	  
scor:PlanDeliver
      rdf:type owl:Class ;
      rdfs:comment "The development and establishment of courses of action over specified time periods that represent a projected appropriation of delivery resources to meet delivery requirements"@en ;
      rdfs:label "Plan Deliver" ;
      rdfs:subClassOf scor:Plan ;
      skos:altLabel "sP4" .

scor:PlanReturn
      rdf:type owl:Class ;
      rdfs:comment "establish and adjust courses of action or tasks over specified time periods that represent a projected appropriation of return resources and assets to meet anticipated as well as unanticipated return requirements"@en ;
      rdfs:label "Plan Return" ;
      rdfs:subClassOf scor:Plan ;
      skos:altLabel "sP5" .

# Source 	  

scor:SourceStockedProduct
      rdf:type owl:Class ;
      rdfs:comment "The process of ordering, receiving and transferring raw material items, sub-assemblies, product and or services based on aggregated demand requirements." @en;
      rdfs:label "Source Stocked Product" ;
      rdfs:subClassOf scor:Source ;
      skos:altLabel "sS1" .	 

scor:SourceMakeToOrderProduct
      rdf:type owl:Class ;
      rdfs:comment "The processes of ordering and receiving product or material that is ordered (and may be configured) only when required by a specific customer order." @en ;
      rdfs:label "Source Make-to-Order Product" ;
      rdfs:subClassOf scor:Source ;
      skos:altLabel "sS2" .	  
	  
scor:SourceEngineerToOrderProduct
      rdf:type owl:Class ;
      rdfs:comment "The processes of identifying and selecting sources of supply, negotiating, validating, scheduling, ordering and receiving parts, assemblies or specialized products or services that are designed, ordered and/or built based on the requirements or specifications of a specific customer order." @en ;
      rdfs:label "Source Engineer-to-Order Product" ;
      rdfs:subClassOf scor:Source ;
      skos:altLabel "sS3" .
	  
# Make

scor:MakeToStock
      rdf:type owl:Class ;
      rdfs:comment "The process of manufacturing in a make-to-stock environment adds value to products through mixing, separating, forming, machining, and chemical processes." @en ;
      rdfs:label "Make-to-Stock" ;
      rdfs:subClassOf scor:Make ;
      skos:altLabel "sM1" .

scor:MakeToOrder
      rdf:type owl:Class ;
      rdfs:comment "The process of manufacturing in a make-to-order environment adds value to products through mixing, separating, forming, machining, and chemical processes for a specific customer order."@en ;
      rdfs:label "Make-to-Order" ;
      rdfs:subClassOf scor:Make ;
      skos:altLabel "sM2" .

scor:EngineerToOrder
      rdf:type owl:Class ;
      rdfs:comment "The process of developing, designing, validating, and ultimately using a manufacturing process to produce products or services based on the requirements of a specific customer." @en;
      rdfs:label "Engineer-to-Order" ;
      rdfs:subClassOf scor:Make ;
      skos:altLabel "sM3" .	  

# Deliver

scor:DeliverStockedProduct
      rdf:type owl:Class ;
      rdfs:comment "Delivers product that is sourced or made based on aggregated customer orders, projected orders/demand and inventory re-ordering parameters" @en ;
      rdfs:label "Deliver Stocked Product" ;
      rdfs:subClassOf scor:Deliver ;
      scor:hasProcessID "sD1" ;
      skos:altLabel "sD1" .	  

scor:DeliverMakeToOrderProduct
      rdf:type owl:Class ;
      rdfs:comment "Delivers product that is sourced, configured, manufactured, and/or assembled from standard raw materials, parts, ingredients or sub-assemblies, in response to a specific firm customer order" @en ;
      rdfs:label "Deliver Make-to-Order Product" ;
      rdfs:subClassOf scor:Deliver ;
      scor:hasProcessID "sD2" ;
      skos:altLabel "sD2" .	  
	  
scor:DeliverEngineerToOrderProduct
      rdf:type owl:Class ;
      rdfs:comment "Obtaining, responding to, and allocating resources for a customer order that has unique requirements or specifications and delivering a product that is partially or fully designed, redesigned, manufactured, and/or assembled from a bill of materials or recipe that includes one or more custom parts or ingredients" @en ;
      rdfs:label "Deliver Engineer-to-Order Product" ;
      rdfs:subClassOf scor:Deliver ;
      scor:hasProcessID "sD3" ;
      skos:altLabel "sD3" .

scor:DeliverRetailProduct
      rdf:type owl:Class ;
      rdfs:comment "To acquire, merchandise, and sell finished goods at a retail store" @en ;
      rdfs:label "Deliver Retail Product" ;
      rdfs:subClassOf scor:Deliver ;
      skos:altLabel "sD4" .
	  
# Return

scor:DeliverReturnDefectiveProduct
      rdf:type owl:Class ;
      rdfs:comment "The receipt and disposition determination of defective products as defined by the warranty claims, product recall, non-conforming product and/or other similar policies including appropriate replacement" @en ;
      rdfs:label "Deliver Return Defective Product" ;
      rdfs:subClassOf scor:Return ;
      skos:altLabel "sDR1" .

scor:DeliverReturnMROProduct
      rdf:type owl:Class ;
      rdfs:comment "The receipt of Maintenance, Repair and Overhaul (MRO) products or company assets for the purpose of servicing, repairing or upgrading it, as defined by Maintenance Plans or the occurrence or anticipation of risk of failure" @en ;
      rdfs:label "Deliver Return MRO Product" ;
      rdfs:subClassOf scor:Return ;
      skos:altLabel "sDR2" .	  
	  
scor:DeliverReturnExcessProduct
      rdf:type owl:Class ;
      rdfs:comment "The receipt of excess or aging inventory or obsolete products as defined by the terms and conditions of a customer/supplier contract" @en ;
      rdfs:label "Deliver Return Excess Product" ;
      rdfs:subClassOf scor:Return ;
      skos:altLabel "sDR3" .

scor:ReturnMROProduct
      rdf:type owl:Class ;
      rdfs:comment "The return of Maintenance, Repair and Overhaul (MRO) products or company assets for the purpose of servicing, repairing or upgrading it, as defined by Maintenance Plans or the occurrence or anticipation of risk of failure"@en ;
      rdfs:label "Return MRO Product" ;
      rdfs:subClassOf scor:Return ;
      skos:altLabel "sSR2" .
	  
scor:SourceReturnDefectiveProduct
      rdf:type owl:Class ;
      rdfs:comment "The return and disposition determination of defective products as defined by the warranty claims, product recall, non-conforming product and/or other similar policies including appropriate replacement"@en ;
      rdfs:label "Source Return Defective Product" ;
      rdfs:subClassOf scor:Return ;
      skos:altLabel "sSR1" .

scor:SourceReturnExcessProduct
      rdf:type owl:Class ;
      rdfs:comment "The return of excess or aging inventory or obsolete products as defined by the terms and conditions of a customer/supplier contract"@en ;
      rdfs:label "Source Return Excess Product" ;
      rdfs:subClassOf scor:Return ;
      skos:altLabel "sSR3" .	  
	  
# Enable 

scor:ManageSupplyChainBusinessRules
      rdf:type owl:Class ;
      rdfs:comment "Establishing, documenting, communicating and publishing supply chain business rules" @en ;
      rdfs:label "Manage Supply Chain Business Rules" ;
      rdfs:subClassOf scor:Enable ;
      skos:altLabel "sE1" .	 

scor:ManagePerformance
      rdf:type owl:Class ;
      rdfs:comment "Reporting performance, identifying gaps in performance, performing root cause analysis, and developing and launching corrective actions to close gaps in perfromance" @en ;
      rdfs:label "Manage Performance" ;
      rdfs:subClassOf scor:Enable ;
      skos:altLabel "sE2" .
	  
scor:ManageDataInformation
      rdf:type owl:Class ;
      rdfs:comment "Collecting, maintaining and publishing data and information required to plan, operate, measure and manage the supply chain" @en ;
      rdfs:label "Manage Data and Information" ;
      rdfs:subClassOf scor:Enable ;
      skos:altLabel "sE3" .
	  
scor:ManageSupplyChainHumanResources
      rdf:type owl:Class ;
      rdfs:comment "Developing, governing and maintaining an organization of permanent, temporary and outsourced staff, with the right qualifications, in support of the business objects and supply chain goals" @en ;
      rdfs:label "Manage Supply Chain Human Resources" ;
      rdfs:subClassOf scor:Enable ;
      skos:altLabel "sE4" .	  
	  
scor:ManageSupplyChainAssets
      rdf:type owl:Class ;
      rdfs:comment "Scheduling, maintaining and dispositioning of supply chain assets that operate supply chain processes" @en ;
      rdfs:label "Manage Supply Chain Assets" ;
      rdfs:subClassOf scor:Enable ;
      skos:altLabel "sE5" .	  

scor:ManageSupplyChainContracts
      rdf:type owl:Class ;
      rdfs:comment "The management and communication of contractual agreements in support of business objectives and supply chain goals" @en ;
      rdfs:label "Manage Supply Chain Contracts" ;
      rdfs:subClassOf scor:Enable ;
      skos:altLabel "sE6" .

scor:ManageSupplyChainNetworks
      rdf:type owl:Class ;
      rdfs:comment "Developing, governing and maintaining a network of supply chain assets" @en ;
      rdfs:label "Manage Supply Chain Networks" ;
      rdfs:subClassOf scor:Enable ;
      skos:altLabel "sE7" .	  
	  
scor:ManageRegulatoryCompliance
      rdf:type owl:Class ;
      rdfs:comment "Identifying, collecting, assessing and integrating regulatory compliance requirements in standard supply chain processes, policies and business rules" @en ;
      rdfs:label "Manage Regulatory Compliance" ;
      rdfs:subClassOf scor:Enable ;
      skos:altLabel "sE8" .
	  
scor:ManageSupplyChainRisk
      rdf:type owl:Class ;
      rdfs:comment "Identification and assessment of potential disruptions (risks) in the supply chain and developing a plan to mitigate these threats to operating the supply chain" @en ;
      rdfs:label "Manage Supply Chain Risk" ;
      rdfs:subClassOf scor:Enable ;
      skos:altLabel "sE9" .	  

# End of Level 2 Processes 

# Level 3 Processes 

# Plan SC

scor:IdentifyPrioritizeAggregateSCRequirements
      rdf:type owl:Class ;
      rdfs:comment "The process of identifying, aggregating, and prioritizing, all sources of demand for the integrated supply chain of a product or service at the appropriate level, horizon and interval."@en ;
      rdfs:label "Identify, Prioritize Aggregate Supply Chain Requirements" ;
      rdfs:subClassOf scor:PlanSupplyChain ;
      skos:altLabel "sP1.1" .

scor:IdentifyPrioritizeAggregateSCResources
      rdf:type owl:Class ;
      rdfs:comment "The process of identifying, prioritizing, and aggregating, as a whole with constituent parts, all sources of supply that are required and add value in the supply chain of a product or service at the appropriate level, horizon and interval."@en ;
      rdfs:label "Identify, Prioritize Aggregate Supply Chain Resources" ;
      rdfs:subClassOf scor:PlanSupplyChain ;
      skos:altLabel "sP1.2" .
	  
scor:BalanceSCResourcesWithSCRequirements
      rdf:type owl:Class ;
      rdfs:comment "The process of identifying and measuring the gaps and imbalances between demand and resources in order to determine how to best resolve the variances through marketing, pricing, packaging, warehousing, outsource plans or some other action that will optimize service, flexibility, costs, assets, (or other supply chain inconsistencies) in an iterative and collaborative environment."@en ;
      rdfs:label "Balance Supply Chain Resources with SC Requirements" ;
      rdfs:subClassOf scor:PlanSupplyChain ;
      skos:altLabel "sP1.3" .
	  
scor:EstablishCommunicateSCPlans
      rdf:type owl:Class ;
      rdfs:comment "The establishment and communication of courses of action over the appropriate time-defined (long-term, annual, monthly, weekly) planning horizon and interval, representing a projected appropriation of supply-chain resources to meet supply chain requirements." @en ;
      rdfs:label "Establish and Communicate Supply Chain Plans" ;
      rdfs:subClassOf scor:PlanSupplyChain ;
      skos:altLabel "sP1.4" .	

# Plan Source

scor:IdentifyPrioritizeAggregateProductRequirements
      rdf:type owl:Class ;
      rdfs:comment "The process of identifying, prioritizing, and considering, as a whole with constituent parts, all sources of demand for a product or service in the supply chain." @en ;
      rdfs:label "Identify, Prioritize and Aggregate Product Requirements" ;
      rdfs:subClassOf scor:PlanSource ;
      skos:altLabel "sP2.1" .	

scor:IdentifyAssessAggregateProductResources
      rdf:type owl:Class ;
      rdfs:comment "The process of identifying, evaluating, and considering, as a whole with constituent parts, all material and other resources used to add value in the supply chain for a product or services." @en ;
      rdfs:label "Identify, Assess and Aggregate Product Resources" ;
      rdfs:subClassOf scor:PlanSource ;
      skos:altLabel "sP2.2" .		

scor:BalanceProductResourcesWithProductRequirements
      rdf:type owl:Class ;
      rdfs:comment "The process of developing a time-phased course of action that commits resources to meet requirements." @en ;
      rdfs:label "Balance Product Resources with Product Requirements" ;
      rdfs:subClassOf scor:PlanSource ;
      skos:altLabel "sP2.3" .

scor:EstablishSourcingPlans
      rdf:type owl:Class ;
      rdfs:comment "The establishment of courses of action over specified time periods that represent a projected appropriation of supply resources to meet sourcing plan requirements." @en ;
      rdfs:label "Establish Sourcing Plans" ;
      rdfs:subClassOf scor:PlanSource ;
      skos:altLabel "sP2.4" .		

# Plan Make
	  
scor:IdentifyPrioritizeAggregateProductionRequirements
      rdf:type owl:Class ;
      rdfs:comment "The process of identifying, prioritizing, and considering as a whole with constituent parts, all sources of demand in the creation of a product or service." @en ;
      rdfs:label "Identify, Prioritize and Aggregate Production Requirements" ;
      rdfs:subClassOf scor:PlanMake ;
      skos:altLabel "sP3.1" .
	  
scor:IdentifyAssessAggregateProductionResources
      rdf:type owl:Class ;
      rdfs:comment "The process of identifying, evaluating, and considering, as a whole with constituent parts, all things that add value in the creation of a product or performance of a service." @en ;
      rdfs:label "Identify, Assess and Aggregate Production Resources" ;
      rdfs:subClassOf scor:PlanMake ;
      skos:altLabel "sP3.2" .	
	  
scor:BalanceProductionResourcesWithProductionRequirements
      rdf:type owl:Class ;
      rdfs:comment "The process of developing a time-phased course of action that commits creation and operation resources to meet creation and operation requirements." @en ;
      rdfs:label "Balance Production Resources with Production Requirements" ;
      rdfs:subClassOf scor:PlanMake ;
      skos:altLabel "sP3.3" .	  
	  
scor:EstablishProductionPlans
      rdf:type owl:Class ;
      rdfs:comment "The establishment of courses of action over specified time periods that represent a projected appropriation of supply resources to meet production and operating plan requirements." @en ;
      rdfs:label "Establish Production Plans" ;
      rdfs:subClassOf scor:PlanMake ;
      skos:altLabel "sP3.4" .

# Plan Deliver

scor:IdentifyPrioritizeAggregateDeliveryRequirements
      rdf:type owl:Class ;
      rdfs:comment "The process of identifying, prioritizing, and considering, as a whole with constituent parts, all sources of demand in the delivery of a product or service." @en ;
      rdfs:label "Identify, Prioritize and Aggregate Delivery Requirements" ;
      rdfs:subClassOf scor:PlanDeliver ;
      skos:altLabel "sP4.1" .
	  
scor:IdentifyAssessAggregateDeliveryResources
      rdf:type owl:Class ;
      rdfs:comment "The process of identifying, evaluating, and considering, as a whole with constituent parts, all things that add value in the delivery of a product or service." @en ;
      rdfs:label "Identify, Assess and Aggregate Delivery Resources" ;
      rdfs:subClassOf scor:PlanDeliver ;
      skos:altLabel "sP4.2" .
	  
scor:BalanceDeliveryResourcesCapabilitiesWithDeliveryRequirements
      rdf:type owl:Class ;
      rdfs:comment "The process of developing a time-phased course of action that commits delivery resources to meet delivery requirements." @en ;
      rdfs:label "Balance Delivery Resources and Capabilities with Delivery Requirements" ;
      rdfs:subClassOf scor:PlanDeliver ;
      skos:altLabel "sP4.3" .
	  
scor:EstablishDeliveryPlans
      rdf:type owl:Class ;
      rdfs:comment "The establishment of courses of action over specified time periods that represent a projected appropriation of delivery resources to meet delivery requirements." @en ;
      rdfs:label "Establish Delivery Plans" ;
      rdfs:subClassOf scor:PlanDeliver ;
      skos:altLabel "sP4.4" .	

# Plan Return

scor:AssessAggregateReturnRequirements
      rdf:type owl:Class ;
      rdfs:comment "The process of identifying, evaluating, and considering, as a whole with constituent parts, all sources of demand for the return of a product." @en ;
      rdfs:label "Assess and Aggregate Return Requirements" ;
      rdfs:subClassOf scor:PlanReturn ;
      skos:altLabel "sP5.1" .	

scor:IdentifyAssessAggregateReturnResources
      rdf:type owl:Class ;
      rdfs:comment "The process of identifying, evaluating, and consideration for all resources that add value to, execute, or constrain the processes for the return of a product.." @en ;
      rdfs:label "Identify, Assess and Aggregate Return Resources" ;
      rdfs:subClassOf scor:PlanReturn ;
      skos:altLabel "sP5.2" .	  
	
scor:BalanceReturnResourcesWithReturnRequirements
      rdf:type owl:Class ;
      rdfs:comment "The process of developing courses of action that make feasible the commitment the appropriate return resources and or assets to satisfy return requirements." @en ;
      rdfs:label "Balance Return Resources with Return Requirements" ;
      rdfs:subClassOf scor:PlanReturn ;
      skos:altLabel "sP5.3" .	
	  
scor:EstablishCommunicateReturnPlans
      rdf:type owl:Class ;
      rdfs:comment "The establishment and communication of courses of action over specified time periods that represent a projected appropriation of required return resources and or assets to meet return process requirements." @en ;
      rdfs:label "Establish and Communicate Return Plans" ;
      rdfs:subClassOf scor:PlanReturn ;
      skos:altLabel "sP5.4" .		  

# Source Stoked Product

scor:ScheduleProductDeliveries
      rdf:type owl:Class ;
      rdfs:comment "Scheduling and managing the execution of the individual deliveries of product against an existing contract or purchase order." @en ;
      rdfs:label "Schedule Product Deliveries" ;
      rdfs:subClassOf scor:SourceStockedProduct ;
      skos:altLabel "sS1.1" .	  
	  
scor:ReceiveProduct
      rdf:type owl:Class ;
      rdfs:comment "The process and associated activities of receiving product to contract requirements." @en ;
      rdfs:label "Receive Product" ;
      rdfs:subClassOf scor:SourceStockedProduct ;
      skos:altLabel "sS1.2" .	
	  
scor:VerifyProduct
      rdf:type owl:Class ;
      rdfs:comment "The process and associated activities of receiving product to contract requirements." @en ;
      rdfs:label "Verify Product" ;
      rdfs:subClassOf scor:SourceStockedProduct ;
      skos:altLabel "sS1.3" .	  

scor:TransferProduct
      rdf:type owl:Class ;
      rdfs:comment "The transfer of accepted product to the appropriate stocking location within the supply chain." @en ;
      rdfs:label "Transfer Product" ;
      rdfs:subClassOf scor:SourceStockedProduct ;
      skos:altLabel "sS1.4" .
	  
scor:AuthorizeSupplierPayment
      rdf:type owl:Class ;
      rdfs:comment "The process of authorizing payments and paying suppliers for product or services." @en ;
      rdfs:label "Authorize Supplier Payment" ;
      rdfs:subClassOf scor:SourceStockedProduct ;
      skos:altLabel "sS1.5" .	

# Source MakeToOrderProduct

scor:ScheduleProductDeliveries
      rdf:type owl:Class ;
      rdfs:comment "Scheduling and managing the execution of the individual deliveries of product against the contract." @en ;
      rdfs:label "Schedule Product Deliveries" ;
      rdfs:subClassOf scor:SourceMakeToOrderProduct ;
      skos:altLabel "sS2.1" .
	  
scor:SourceMakeToOrderReceiveProduct
      rdf:type owl:Class ;
      rdfs:comment "The process and associated activities of receiving product to contract requirements." @en ;
      rdfs:label "Receive Product" ;
      rdfs:subClassOf scor:SourceMakeToOrderProduct ;
      skos:altLabel "sS2.2" .
	  
scor:SourceMakeToOrderVerifyProduct
      rdf:type owl:Class ;
      rdfs:comment "The process and actions required determining product conformance to requirements and criteria." @en ;
      rdfs:label "Verify Product" ;
      rdfs:subClassOf scor:SourceMakeToOrderProduct ;
      skos:altLabel "sS2.3" .
	  
scor:SourceMakeToOrderTransferProduct
      rdf:type owl:Class ;
      rdfs:comment "The transfer of accepted product to the appropriate stocking location within the supply chain." @en ;
      rdfs:label "Transfer Product" ;
      rdfs:subClassOf scor:SourceMakeToOrderProduct ;
      skos:altLabel "sS2.4" .
	  
scor:SourceMakeToOrderAuthorizeSupplierPayment
      rdf:type owl:Class ;
      rdfs:comment "The process of authorizing payments and paying suppliers for product or services." @en ;
      rdfs:label "Supplier Payment" ;
      rdfs:subClassOf scor:SourceMakeToOrderProduct ;
      skos:altLabel "sS2.4" .

# SourceEngineerToOrderProduct	
  
scor:IdentifySourcesOfSupply
      rdf:type owl:Class ;
      rdfs:comment "The identification and qualification of potential suppliers capable of designing and delivering product that will meet all of the required product specifications." @en ;
      rdfs:label "Identify Sources of Supply" ;
      rdfs:subClassOf scor:SourceEngineerToOrderProduct ;
      skos:altLabel "sS3.1" .	 

scor:SelectFinalSupplierNegotiate
      rdf:type owl:Class ;
      rdfs:comment "The identification of the final supplier(s) based on the evaluation of RFQs, supplier qualifications and the generation of a contract defining the costs and terms and conditions of product availability." @en ;
      rdfs:label "Select Final Supplier and Negotiate" ;
      rdfs:subClassOf scor:SourceEngineerToOrderProduct ;
      skos:altLabel "sS3.2" .

scor:ScheduleProductDeliveries
      rdf:type owl:Class ;
      rdfs:comment "Scheduling and managing the execution of the individual deliveries of product against the contract." @en ;
      rdfs:label "Schedule Product Deliveries" ;
      rdfs:subClassOf scor:SourceEngineerToOrderProduct ;
      skos:altLabel "sS3.3" .
	  
scor:SourceEngineerToOrderReceiveProduct
      rdf:type owl:Class ;
      rdfs:comment "The process and associated activities of receiving product to contract requirements." @en ;
      rdfs:label "Receive Product" ;
      rdfs:subClassOf scor:SourceEngineerToOrderProduct ;
      skos:altLabel "sS3.4" .
	  
scor:SourceEngineerToOrderVerifyProduct
      rdf:type owl:Class ;
      rdfs:comment "The process and actions required determining product conformance to requirements and criteria." @en ;
      rdfs:label "Verify Product" ;
      rdfs:subClassOf scor:SourceEngineerToOrderProduct ;
      skos:altLabel "sS3.5" .	
	  
scor:SourceEngineerToOrderTransferProduct
      rdf:type owl:Class ;
      rdfs:comment "The transfer of accepted product to the appropriate stocking location within the supply chain." @en ;
      rdfs:label "Transfer Product" ;
      rdfs:subClassOf scor:SourceEngineerToOrderProduct ;
      skos:altLabel "sS3.6" .
	  
scor:SourceEngineerToOrderAuthorizeSupplierPayment
      rdf:type owl:Class ;
      rdfs:comment "The process of authorizing payments and paying suppliers for product or services. This process includes invoice collection, invoice matching and the issuance of checks." @en ;
      rdfs:label "Authorize Supplier Payment" ;
      rdfs:subClassOf scor:SourceEngineerToOrderProduct ;
      skos:altLabel "sS3.7" .	  
	
# Make MakeToStock	

scor:ScheduleProductionActivities
      rdf:type owl:Class ;
      rdfs:comment "Given plans for the production of specific parts, products, or formulations in specified quantities and planned availability of required sourced products, the scheduling of the operations to be performed in accordance with these plans." @en ;
      rdfs:label "Schedule Production Activities" ;
      rdfs:subClassOf scor:MakeToStock ;
      skos:altLabel "sM1.1" .	
	  
scor:IssueMaterial
      rdf:type owl:Class ;
      rdfs:comment "The selection and physical movement of sourced/in-process product (e.g., raw materials, fabricated components, subassemblies, required ingredients or intermediate formulations) from a stocking location (e.g., stockroom, a location on the production floor, a supplier) to a specific point of use location." @en ;
      rdfs:label "Issue Material" ;
      rdfs:subClassOf scor:MakeToStock ;
      skos:altLabel "sM1.2" .	

scor:ProduceTest
      rdf:type owl:Class ;
      rdfs:comment "The series of activities performed upon sourced/in-process product to convert it from the raw or semi-finished state to a state of completion and greater value." @en ;
      rdfs:label "Produce and Test" ;
      rdfs:subClassOf scor:MakeToStock ;
      skos:altLabel "sM1.3" .	 

scor:Package
      rdf:type owl:Class ;
      rdfs:comment "The series of activities that containerize completed products for storage or sale to end-users." @en ;
      rdfs:label "Package" ;
      rdfs:subClassOf scor:MakeToStock ;
      skos:altLabel "sM1.4" .

scor:StageProduct
      rdf:type owl:Class ;
      rdfs:comment "The movement of packaged products into a temporary holding location to await movement to a finished goods location." @en ;
      rdfs:label "Stage Product" ;
      rdfs:subClassOf scor:MakeToStock ;
      skos:altLabel "sM1.5" .	 

scor:ReleaseProductToDeliver
      rdf:type owl:Class ;
      rdfs:comment "Activities associated with post-production documentation, testing, or certification required prior to delivery of finished product to customer." @en ;
      rdfs:label "Release Product to Deliver" ;
      rdfs:subClassOf scor:MakeToStock ;
      skos:altLabel "sM1.6" .	

scor:WasteDisposal
      rdf:type owl:Class ;
      rdfs:comment "Activities associated with collecting and managing waste produced during the produce and test process including scrap material and non-conforming product." @en ;
      rdfs:label "Waste Disposal" ;
      rdfs:subClassOf scor:MakeToStock ;
      skos:altLabel "sM1.7" .

# Make MakeToOrder	  
	  
scor:MakeToOrderScheduleProductionActivities
      rdf:type owl:Class ;
      rdfs:comment "Given plans for the production of specific parts, products, or formulations in specific quantities and planned availability of required sourced products, the scheduling of the operations to be preformed in accordance with these plans." @en ;
      rdfs:label "Schedule Production Activities" ;
      rdfs:subClassOf scor:MakeToOrder ;
      skos:altLabel "sM2.1" .
	  
scor:IssueSourcedInProcessProduct
      rdf:type owl:Class ;
      rdfs:comment "The selection and physical movement of sourced/in-process products (e.g., raw materials, fabricated components, subassemblies, required ingredients or intermediate formulations) from a stocking location (e.g., stockroom, a location on the production floor, a supplier) to a specific point of use location." @en ;
      rdfs:label "Issue Sourced In-Process Product" ;
      rdfs:subClassOf scor:MakeToOrder ;
      skos:altLabel "sM2.2" .
	  
scor:MakeToOrderProduceTest
      rdf:type owl:Class ;
      rdfs:comment "The series of activities performed upon sourced/in-process product to convert it from the raw or semi-finished state to a state of completion and greater value." @en ;
      rdfs:label "Produce and Test" ;
      rdfs:subClassOf scor:MakeToOrder ;
      skos:altLabel "sM2.3" .
	  
scor:MakeToOrderPackage
      rdf:type owl:Class ;
      rdfs:comment "The series of activities that containerize completed products for storage or sale to end-users." @en ;
      rdfs:label "Package" ;
      rdfs:subClassOf scor:MakeToOrder ;
      skos:altLabel "sM2.4" .	
	  
scor:StageFinishedProduct
      rdf:type owl:Class ;
      rdfs:comment "The movement of packaged products into a temporary holding location to await movement to a finished goods location." @en ;
      rdfs:label "Stage Finished Product" ;
      rdfs:subClassOf scor:MakeToOrder ;
      skos:altLabel "sM2.5" .	

scor:ReleaseFinishedProductToDeliver
      rdf:type owl:Class ;
      rdfs:comment "Activities associated with post-production documentation, testing, or certification required prior to delivery of finished product to customer." @en ;
      rdfs:label "Release Finished Product to Deliver" ;
      rdfs:subClassOf scor:MakeToOrder ;
      skos:altLabel "sM2.6" .	  
	  
scor:MakeToOrderWasteDisposal
      rdf:type owl:Class ;
      rdfs:comment "Activities associated with collecting and managing waste produced during the produce and test process including scrap material and non-conforming product." @en ;
      rdfs:label "Waste Disposal" ;
      rdfs:subClassOf scor:MakeToOrder ;
      skos:altLabel "sM2.7" .
	  
# Make Engineer to Order	  

scor:FinalizeProductionEngineering
      rdf:type owl:Class ;
      rdfs:comment "Engineering activities required after acceptance of order, but before product can be produced. May include generation and delivery of final drawings, specifications, formulas, part programs, etc." @en ;
      rdfs:label "Finalize Production Engineering" ;
      rdfs:subClassOf scor:EngineerToOrder ;
      skos:altLabel "sM3.1" .
	  
scor:EngineerToOrderScheduleProductionActivities
      rdf:type owl:Class ;
      rdfs:comment "Given plans for the production of specific parts, products, or formulations in specified quantities and planned availability of required sourced products, the scheduling of the operations to be performed in accordance with these plans" @en ;
      rdfs:label "Schedule Production Activities" ;
      rdfs:subClassOf scor:EngineerToOrder ;
      skos:altLabel "sM3.2" .	 
	  
scor:EngineerToOrderSourcedInProcessProduct
      rdf:type owl:Class ;
      rdfs:comment "The selection and physical movement of sourced/in-process products (e.g., raw materials, fabricated components, subassemblies, required ingredients or intermediate formulations) from a stocking location (e.g., stockroom, a location on the production floor, a supplier) to a specific point of use location" @en ;
      rdfs:label "Issue Sourced In-Process Product" ;
      rdfs:subClassOf scor:EngineerToOrder ;
      skos:altLabel "sM3.3" .	

scor:EngineerToOrderProduceTest
      rdf:type owl:Class ;
      rdfs:comment "The series of activities performed upon sourced/in-process product to convert it from the raw or semi-finished state to a state of completion and greater value" @en ;
      rdfs:label "Produce and Test" ;
      rdfs:subClassOf scor:EngineerToOrder ;
      skos:altLabel "sM3.4" .	
	  
scor:EngineerToOrderPackage
      rdf:type owl:Class ;
      rdfs:comment "The series of activities that containerize completed products for storage or sale to end-users." @en ;
      rdfs:label "Package" ;
      rdfs:subClassOf scor:EngineerToOrder ;
      skos:altLabel "sM3.5" .
	  
scor:EngineerToOrderStageFinishedProduct
      rdf:type owl:Class ;
      rdfs:comment "The movement of packaged products into a temporary holding location to await movement to a finished goods location." @en ;
      rdfs:label "Stage Finished Product" ;
      rdfs:subClassOf scor:EngineerToOrder ;
      skos:altLabel "sM3.6" .	

scor:EngineerToOrderReleaseProductToDeliver
      rdf:type owl:Class ;
      rdfs:comment "Activities associated with post-production documentation, testing, or certification required prior to delivery of finished product to customer." @en ;
      rdfs:label "Release Product to Deliver" ;
      rdfs:subClassOf scor:EngineerToOrder ;
      skos:altLabel "sM3.7" .	  
	  
scor:EngineerToOrderWasteDisposal
      rdf:type owl:Class ;
      rdfs:comment "Activities associated with collecting and managing waste produced during the produce and test process including scrap material and non-conforming product." @en ;
      rdfs:label "Waste Disposal" ;
      rdfs:subClassOf scor:EngineerToOrder ;
      skos:altLabel "sM3.8" .	  
  
# End of Level 3 Processes 
	  
# Metrics

scor:Agility
      rdf:type owl:Class ;
      rdfs:comment "The Agility attribute describes the ability to respond to external influences; the ability to and speed of change."@en ;
      rdfs:label "Agility" ;
      rdfs:subClassOf scor:PerformanceAttribute .

scor:Assets
      rdf:type owl:Class ;
      rdfs:comment "The Assets attribute describes the ability to efficiently utilize assets."@en ;
      rdfs:label "Assets" ;
      rdfs:subClassOf scor:PerformanceAttribute .

scor:AdditionalRequiredDocumentationAccuracy
      rdf:type owl:Class ;
      rdfs:subClassOf scor:DocumentationAccuracy ;
      scor:isCalculatedBy "[Total Perfect Orders] / [Total Number of Orders] x 100%" .	  
	  
scor:CashToCashCycleTime
      rdf:type owl:Class ;
      rdfs:comment "The time it takes for an investment made to flow back into a company after it has been spent for raw materials"@en ;
      rdfs:label "CashToCashCycleTime" ;
      rdfs:subClassOf scor:KeyPerformanceIndicator ;
      skos:altLabel "AM.1.1" .

scor:ComplianceDocumentationAccuracy
      rdf:type owl:Class ;
      rdfs:subClassOf scor:DocumentationAccuracy ;
      scor:isCalculatedBy "[Total Perfect Orders] / [Total Number of Orders] x 100%" .

scor:Cost
      rdf:type owl:Class ;
      rdfs:comment "The Cost attribute describes the cost of operating the process."@en ;
      rdfs:label "Cost" ;
      rdfs:subClassOf scor:PerformanceAttribute .

scor:CustomerCommitDateAchievementTimeCustomerReceiving
      rdf:type owl:Class ;
      rdfs:subClassOf scor:DeliveryPerformanceToCustomerCommitDate ;
      scor:isCalculatedBy "[Total Perfect Orders] / [Total Number of Orders] x 100%" .

scor:DeliveryItemAccuracy
      rdf:type owl:Class ;
      rdfs:subClassOf scor:PercentOfOrdersDeliveredInFull ;
      scor:isCalculatedBy "[Total Perfect Orders] / [Total Number of Orders] x 100%" .

scor:DeliveryLocationAccuracy
      rdf:type owl:Class ;
      rdfs:subClassOf scor:DeliveryPerformanceToCustomerCommitDate ;
      scor:isCalculatedBy "[Total Perfect Orders] / [Total Number of Orders] x 100%" .

scor:DeliveryPerformanceToCustomerCommitDate
      rdf:type owl:Class ;
      rdfs:subClassOf scor:PerfectOrderFulfillment ;
      scor:isCalculatedBy "[Total Perfect Orders] / [Total Number of Orders] x 100%" .

scor:DeliveryQuantityAccuracy
      rdf:type owl:Class ;
      rdfs:subClassOf scor:PercentOfOrdersDeliveredInFull ;
      scor:isCalculatedBy "[Total Perfect Orders] / [Total Number of Orders] x 100%" .

scor:DocumentationAccuracy
      rdf:type owl:Class ;
      rdfs:subClassOf scor:PerfectOrderFulfillment ;
      scor:isCalculatedBy "[Total Perfect Orders] / [Total Number of Orders] x 100%" .

scor:DownsideAdaptability
      rdf:type owl:Class ;
      rdfs:comment "Downside  Adaptability" ;
      rdfs:label "DownsideAdaptability" ;
      rdfs:subClassOf scor:KeyPerformanceIndicator ;
      skos:altLabel "AG.1.3" .

scor:KeyPerformanceIndicator
      rdf:type owl:Class ;
      rdfs:comment "Diagnostics for the overall health of the supply chain. Benchmarking Key Performance Indicators helps establishing realistic targets to support the strategic directions"@en ;
      rdfs:label "KeyPerformanceIndicator" ;
      rdfs:subClassOf daq:Metric .

scor:OrderDeliveredDamageFreeConformance
      rdf:type owl:Class ;
      rdfs:subClassOf scor:PerfectCondition ;
      scor:isCalculatedBy "[Total Perfect Orders] / [Total Number of Orders] x 100%" .

scor:OrderDeliveredDefectFreeConformance
      rdf:type owl:Class ;
      rdfs:subClassOf scor:PerfectCondition ;
      scor:isCalculatedBy "[Total Perfect Orders] / [Total Number of Orders] x 100%" .

scor:OrderFulfillmentCycleTime
      rdf:type owl:Class ;
      rdfs:comment "Order Fulfillment Cycle Time" ;
      rdfs:label "OrderFulfillmentCycleTime" ;
      rdfs:subClassOf scor:KeyPerformanceIndicator ;
      skos:altLabel "RS.1.1" .

scor:OverallValueAtRisk
      rdf:type owl:Class ;
      rdfs:comment "Overall Value-at-Risk" ;
      rdfs:label "OverallValueAtRisk" ;
      rdfs:subClassOf scor:KeyPerformanceIndicator ;
      skos:altLabel "AG.1.4" .

scor:PaymentDocumenationAccuracy
      rdf:type owl:Class ;
      rdfs:subClassOf scor:DocumentationAccuracy ;
      scor:isCalculatedBy "[Total Perfect Orders] / [Total Number of Orders] x 100%" .

scor:PercentOfFaultnessInstallations
      rdf:type owl:Class ;
      rdfs:subClassOf scor:PerfectCondition ;
      scor:isCalculatedBy "[Total Perfect Orders] / [Total Number of Orders] x 100%" .

scor:PercentOfOrdersDeliveredInFull
      rdf:type owl:Class ;
      rdfs:subClassOf scor:PerfectOrderFulfillment ;
      scor:isCalculatedBy "[Total Perfect Orders] / [Total Number of Orders] x 100%" .

scor:PercentOrdersLinesReceivedDamageFree
      rdf:type owl:Class ;
      rdfs:subClassOf scor:PerfectCondition ;
      scor:isCalculatedBy "[Total Perfect Orders] / [Total Number of Orders] x 100%" .

scor:PerfectCondition
      rdf:type owl:Class ;
      rdfs:subClassOf scor:PerfectOrderFulfillment ;
      scor:isCalculatedBy "[Total Perfect Orders] / [Total Number of Orders] x 100%" .

scor:PerfectOrderFulfillment
      rdf:type owl:Class ;
      rdfs:comment "Delivered complete, on time according the client's specifications of time. Documentation complete. Faultlessly installed"@en ;
      rdfs:label "PerfectOrderFulfillment" ;
      rdfs:subClassOf scor:Reliability , scor:KeyPerformanceIndicator ;
      scor:isCalculatedBy "[Total Perfect Orders] / [Total Number of Orders] x 100%" ;
      skos:altLabel "RL.1.1" .

scor:PerformanceAttribute
      rdf:type owl:Class ;
      rdfs:comment "A performance attribute is a grouping or categorization of metrics used to express a specific strategy"@en ;
      rdfs:label "PerformanceAttribute" .

scor:Reliability
      rdf:type owl:Class ;
      rdfs:comment "The Reliability attribute addresses the ability to perform tasks as required. Reliability focuses on the predictability of the outcome of a process."@en;
      rdfs:label "Reliability" ;
      rdfs:subClassOf scor:PerformanceAttribute .

scor:Responsiveness
      rdf:type owl:Class ;
      rdfs:comment "The Responsiveness attribute describes the speed at which tasks are performed. Responsiveness addresses repeated speed of doing business."@en ;
      rdfs:label "Responsiveness" ;
      rdfs:subClassOf scor:PerformanceAttribute .

scor:ReturnOnFixedAssets
      rdf:type owl:Class ;
      rdfs:comment "Measures the return an organization receives on its invested capital in supply chain fixed assets. This includes the fixed assets used in Plan, Source, Make,Deliver, and Return"@en ;
      rdfs:label "ReturnOnFixedAssets" ;
      rdfs:subClassOf scor:KeyPerformanceIndicator ;
      skos:altLabel "AM.1.2." .

scor:ReturnOnWorkingCapital
      rdf:type owl:Class ;
      rdfs:comment "Assesses the magnitude of investment relative to a company's working capital position versus the revenue generated from a supply chain."@en ;
      rdfs:label "ReturnOnWorkingCapital" ;
      rdfs:subClassOf scor:KeyPerformanceIndicator ;
      skos:altLabel "AM.1.3." .

scor:ShippingDocumenationAccuracy
      rdf:type owl:Class ;
      rdfs:subClassOf scor:DocumentationAccuracy ;
      scor:isCalculatedBy "[Total Perfect Orders] / [Total Number of Orders] x 100%" .

scor:TotalCostToServe
      rdf:type owl:Class ;
      rdfs:comment "The sum of the Supply Chain Cost to deliver products and services to customers"@en ;
      rdfs:label "TotalCostToServe" ;
      rdfs:subClassOf scor:KeyPerformanceIndicator ;
      skos:altLabel "CO.1.001" .

scor:UpsideAdaptability
      rdf:type owl:Class ;
      rdfs:comment "Upside Adaptability" ;
      rdfs:label "UpsideAdaptability" ;
      rdfs:subClassOf scor:KeyPerformanceIndicator ;
      skos:altLabel "AG.1.2" .

scor:UpsideFlexibility
      rdf:type owl:Class ;
      rdfs:comment "Upside Flexibility" ;
      rdfs:label "UpsideFlexibility" ;
      rdfs:subClassOf scor:KeyPerformanceIndicator ;
      skos:altLabel "AG.1.1" .

scor:WarrantyReturns
      rdf:type owl:Class ;
      rdfs:subClassOf scor:PerfectCondition ;
      scor:isCalculatedBy "[Total Perfect Orders] / [Total Number of Orders] x 100%" .

scor:hasMetric
      rdf:type owl:ObjectProperty ;
      rdfs:domain scor:Process ;
      rdfs:range daq:Metric .

scor:hasMetricID
      rdf:type owl:AnnotationProperty ;
      rdfs:comment "" ;
      rdfs:domain daq:Metric ;
      rdfs:label "has metric ID" ;
      rdfs:range xsd:string .

scor:hasProcessID
      rdf:type owl:AnnotationProperty ;
      rdfs:comment "Represents a unique identifier of a process within the SCOR model"@en ;
      rdfs:label "has process ID" ;
      rdfs:range xsd:string .

scor:hasProcessStepList
      rdf:type owl:DatatypeProperty , owl:ObjectProperty ;
      rdfs:comment "Represents a unique identifier of a process within the SCOR model"@en ;
      rdfs:domain scor:Process ;
      rdfs:label "has process step list" ;
      rdfs:range xsd:string .

scor:isCalculatedBy
      rdf:type owl:AnnotationProperty ;
      rdfs:label "is calculated by" ;
      rdfs:range xsd:string .

scor:measure
      rdf:type owl:ObjectProperty ;
      rdfs:domain scor:KeyPerformanceIndicator ;
      rdfs:range scor:PerformanceAttribute .

daq:Metric
      rdf:type owl:Class ;
      rdfs:comment "A metric is a standard for measurement of the performance of a process." @en;
      rdfs:label "Metric" .

scor:AuthorizeSupplierPaymentCycleTime
      rdf:type owl:Class ;
      rdfs:subClassOf scor:SourceCycleTime ;
      skos:prefLabel "RS.3.8"^^xsd:string .

scor:DownsideDeliverAdaptability
      rdf:type owl:Class ;
      rdfs:comment "Downside Deliver Adaptability = The reduction in delivered quantities sustainable at 30 days prior to delivery with no inventory or cost penalties." @en ;
      rdfs:subClassOf scor:DownsideSCAdaptability ;
	  rdfs:label "Downside Deliver Adaptability";
      skos:prefLabel "AG.2.13"^^xsd:string .

scor:DownsideMakeAdaptability
      rdf:type owl:Class ;
      rdfs:comment "The production reduction sustainable at 30 days prior to delivery with no inventory or cost penalties."@en ;
      rdfs:subClassOf scor:DownsideSCAdaptability ;
	  rdfs:label "Downside Make Adaptability";
      skos:prefLabel "AG.2.12"^^xsd:string .

scor:DownsideSCAdaptability
      rdf:type owl:Class ;
      rdfs:comment "The reduction in quantities ordered sustainable at 30 days prior to delivery with no inventory or cost penalties."@en ;
      rdfs:subClassOf scor:Agility ;
	  rdfs:label "Downside Supply Chain Adaptability";
      skos:prefLabel "AG.1.3"^^xsd:string .

scor:DownsideSourceAdaptability
      rdf:type owl:Class ;
      rdfs:comment "The raw material quantity reduction sustainable at 30 days prior to delivery with no inventory or cost penalties." @en ;
      rdfs:subClassOf scor:DownsideSCAdaptability ;
	  rdfs:label "Downside Source Adaptability";
      skos:prefLabel "AG.2.11"^^xsd:string .

scor:OrderFullfilmentCycleTime
      rdf:type owl:Class ;
      rdfs:comment "The average actual cycle consistently achieved to fulfill customers orders" @en;
      rdfs:subClassOf scor:Responsiveness ;
	  rdfs:label "Order Fullfilment Cycle Time";
      skos:prefLabel "RS.1.1"^^xsd:string .
	  
scor:SourceCycleTime
      rdf:type owl:Class ;
      rdfs:comment "The average time associated with Source Processes. (Processes: sS1, sS2, sS3)" @en ;
      rdfs:subClassOf scor:OrderFullfilmentCycleTime ;
	  rdfs:label "Source Cycle Time";
      skos:prefLabel "RS.2.1"^^xsd:string .

scor:OverallValueAtRisk
      rdf:type owl:Class ;
      rdfs:comment "Risk management in organizations traditionally resides within the finance function, due to its inherent focus on financial impact on the organization." @en ;
      rdfs:subClassOf scor:Agility ;
      skos:prefLabel "AG.1.4"^^xsd:string .

scor:SupplierCustomerProductRiskRating
      rdf:type owl:Class ;
      rdfs:comment "The numerical risk rating for supplier, customer or product. Normalized and used for comparison purposes." @en ;
      rdfs:label "Supplier's/Customer's/Products's Risk Rating"^^xsd:string ;
      rdfs:subClassOf scor:DownsideSCAdaptability ;
      skos:prefLabel "AG.2.14"^^xsd:string .

scor:UpsideDeliverAdaptability
      rdf:type owl:Class ;
      rdfs:comment "The maximum sustainable percentage increase in quantities delivered that can be achieved in 30 days with the assumption of unconstrained finished good availability."@en ;
	  rdfs:label "Upside Deliver Adaptability"^^xsd:string ;
      rdfs:subClassOf scor:UpsideSCAdaptability ;
      skos:prefLabel "AG.2.8"^^xsd:string .

scor:UpsideDeliverFlexibility
      rdf:type owl:Class ;
	  rdfs:label "Upside Deliver Flexibility"^^xsd:string ;
      rdfs:subClassOf scor:UpsideSCFlexibility ;
      skos:prefLabel "AG.2.3"^^xsd:string .

scor:UpsideDeliverReturnAdaptability
      rdf:type owl:Class ;
      rdfs:comment "The maximum sustainable percentage increase in returns of finished goods from customers that can be achieved in 30 days."@en ;
	  rdfs:label "Upside Deliver Return Adaptability"^^xsd:string ;
      rdfs:subClassOf scor:UpsideSCAdaptability ;
      skos:prefLabel "AG.2.10"^^xsd:string .

scor:UpsideDeliverReturnFlexibility
      rdf:type owl:Class ;
	  rdfs:label "Upside Deliver Return Flexibility"^^xsd:string ;
      rdfs:subClassOf scor:UpsideSCFlexibility ;
      skos:prefLabel "AG.2.5"^^xsd:string .

scor:UpsideMakeAdaptability
      rdf:type owl:Class ;
	  rdfs:label "Upside Make Adaptability"^^xsd:string ;
      rdfs:comment "The maximum sustainable percentage increase in production that can be achieved in 30 days with the assumption of no raw material constraints." ;
      rdfs:subClassOf scor:UpsideSCAdaptability ;
      skos:prefLabel "AG.2.7"^^xsd:string .

scor:UpsideMakeFlexibility
      rdf:type owl:Class ;
	  rdfs:label "Upside Make Flexibility"^^xsd:string ;
      rdfs:comment "The number of days required to achieve an unplanned sustainable 20% increase in production with the assumption of no raw material constraints."@en ;
      rdfs:subClassOf scor:UpsideSCFlexibility ;
      skos:prefLabel "AG.2.2"^^xsd:string .

scor:UpsideSCAdaptability
      rdf:type owl:Class ;
	  rdfs:label "Upside Supply Chain Adaptability"^^xsd:string ;
      rdfs:comment "The maximum sustainable percentage increase in quantity delivered that can be achieved in 30 days."@en ;
      rdfs:subClassOf scor:Agility ;
      skos:prefLabel "AG.1.2"^^xsd:string .

scor:UpsideSCFlexibility
      rdf:type owl:Class ;
	  rdfs:label "Upside Supply Chain Flexibility"^^xsd:string ;
      rdfs:comment "The number of days required to achieve an unplanned sustainable 20% increase in quantities delivered."@en ;
      rdfs:subClassOf scor:Agility ;
      skos:prefLabel "AG.1.1"^^xsd:string .

scor:UpsideSourceAdaptability
      rdf:type owl:Class ;
      rdfs:comment "The maximum sustainable percentage increase in raw material quantities that can be acquired/received in 30 days."@en ;
	  rdfs:label "Upside Source Adaptability"^^xsd:string ;
      rdfs:subClassOf scor:UpsideSCAdaptability ;
      skos:prefLabel "AG.2.6"^^xsd:string .

scor:UpsideSourceFlexibility
      rdf:type owl:Class ;
      rdfs:comment "The number of days required to achieve an unplanned sustainable 20% increase in quantity of raw  materials."@en ;
      rdfs:subClassOf scor:UpsideSCFlexibility ;
	  rdfs:label "Upside Source Flexibility"^^xsd:string ;
      skos:prefLabel "AG.2.1"^^xsd:string .

scor:UpsideSourceReturnAdaptability
      rdf:type owl:Class ;
      rdfs:comment "The maximum sustainable percentage increase in returns of raw materials to suppliers that can be achieved in 30 days."@en ;
	  rdfs:label "Upside Source Return Adaptability"^^xsd:string ;
      rdfs:subClassOf scor:UpsideSCAdaptability ;
      skos:prefLabel "AG.2.9"^^xsd:string .

scor:UpsideSourceReturnFlexibility
      rdf:type owl:Class ;
      rdfs:comment "The number of days required to achieve an unplanned sustainable 20% increase in the return of raw materials to suppliers."@en ;
	  rdfs:label "Upside Source Return Flexibility"^^xsd:string ;
      rdfs:subClassOf scor:UpsideSCFlexibility ;
      skos:prefLabel "AG.2.4"^^xsd:string .

scor:Scope
      rdf:type owl:Class ;
      rdfs:comment "Types of focus measure for performance attributes."@en ;
      rdfs:label "Scope" .
	  
scor:Customer
      rdf:type owl:Class ;
      rdfs:comment "Customer focus for performance attributes"@en ;
      rdfs:label "Customer" ;
      rdfs:subClassOf scor:Scope .
	  
scor:Internal
      rdf:type owl:Class ;
      rdfs:comment "Internal focus for performance attributes"@en ;
      rdfs:label "Internal" ;
      rdfs:subClassOf scor:Scope .
	  
scor:Supplier
      rdf:type owl:Class ;
      rdfs:comment "Supplier focus for performance attributes"@en ;
      rdfs:label "Supplier" ;
      rdfs:subClassOf scor:Scope .

dc:Plan1
      rdf:type owl:NamedIndividual , scor:Plan ;
      scor:hasMetric daq:Metric1 .

daq:Metric1
      rdf:type owl:NamedIndividual , daq:Metric ;
      scor:hasMetricID "CO.2.001"^^xsd:string .
	  
skos:altLabel
      rdf:type owl:AnnotationProperty .
